All important proof rules for Refine PiCore

PiCore_Sim.thy
@@ -31,10 +31,6 @@ fixes
                   ('s\<^sub>c \<times> 's\<^sub>a) set, 'prog\<^sub>c \<Rightarrow> 'prog\<^sub>a option, ('s\<^sub>c \<times> 's\<^sub>a) set,
                   'Env\<^sub>a, ('s\<^sub>a,'prog\<^sub>a) pconf, ('s\<^sub>a \<times> 's\<^sub>a) set, ('s\<^sub>a \<times> 's\<^sub>a) set] \<Rightarrow> bool" 
   ("'(_,_,_,_')/ \<preceq>\<^sub>p \<^sub>'(\<^sub>_\<^sub>;\<^sub>_\<^sub>;\<^sub>_\<^sub>') /'(_,_,_,_')" [81,81,81,81,81,81,81,81,81,81,81] 100)
-  and prog_sim_pre :: "['Env\<^sub>c, 'prog\<^sub>c, ('s\<^sub>c \<times> 's\<^sub>c) set, ('s\<^sub>c \<times> 's\<^sub>c) set, 
-                  ('s\<^sub>c \<times> 's\<^sub>a) set, 'prog\<^sub>c \<Rightarrow> 'prog\<^sub>a option, ('s\<^sub>c \<times> 's\<^sub>a) set, ('s\<^sub>c \<times> 's\<^sub>a) set,
-                  'Env\<^sub>a, 'prog\<^sub>a, ('s\<^sub>a \<times> 's\<^sub>a) set, ('s\<^sub>a \<times> 's\<^sub>a) set] \<Rightarrow> bool" 
-  ("'(_,_,_,_')/ \<preceq>\<^sub>p \<^sub>'(\<^sub>_\<^sub>;\<^sub>_\<^sub>;\<^sub>_\<^sub>\<rhd>\<^sub>_\<^sub>')  /'(_,_,_,_')" [81,81,81,81,81,81,81,81,81,81,81,81] 100)
 assumes
   prog_sim_validity: "(\<Gamma>\<^sub>c, (P\<^sub>c, s\<^sub>c), R\<^sub>c, G\<^sub>c) \<preceq>\<^sub>p \<^sub>(\<^sub>\<alpha>\<^sub>;\<^sub>\<zeta>\<^sub>;\<^sub>\<gamma>\<^sub>) (\<Gamma>\<^sub>a, (P\<^sub>a, s\<^sub>a), R\<^sub>a, G\<^sub>a) \<Longrightarrow>
                             (s\<^sub>c, s\<^sub>a) \<in> \<alpha> \<and>
@@ -48,16 +44,12 @@ assumes
                             (\<Gamma>\<^sub>c, (P\<^sub>c', s\<^sub>c'), R\<^sub>c, G\<^sub>c) \<preceq>\<^sub>p \<^sub>(\<^sub>\<alpha>\<^sub>;\<^sub>\<zeta>\<^sub>;\<^sub>\<gamma>\<^sub>) (\<Gamma>\<^sub>a, (P\<^sub>a', s\<^sub>a'), R\<^sub>a, G\<^sub>a)))) \<and>
                       
                             (P\<^sub>c = fin_com\<^sub>c \<longrightarrow> P\<^sub>a = fin_com\<^sub>a \<and> (s\<^sub>c, s\<^sub>a) \<in> \<gamma> \<and> \<gamma> \<subseteq> \<alpha>) \<and> 
+              
+                            (P\<^sub>c \<noteq> fin_com\<^sub>c \<longrightarrow> P\<^sub>a \<noteq> fin_com\<^sub>a) \<and>
 
-                            (\<forall>s\<^sub>c' s\<^sub>a'. ((s\<^sub>c, s\<^sub>c'), (s\<^sub>a, s\<^sub>a')) \<in> ((R\<^sub>c, R\<^sub>a \<union> Id)\<^sub>\<alpha>) \<longrightarrow> 
-                            (\<Gamma>\<^sub>c, (P\<^sub>c, s\<^sub>c'), R\<^sub>c, G\<^sub>c) \<preceq>\<^sub>p \<^sub>(\<^sub>\<alpha>\<^sub>;\<^sub>\<zeta>\<^sub>;\<^sub>\<gamma>\<^sub>) (\<Gamma>\<^sub>a, (P\<^sub>a, s\<^sub>a'), R\<^sub>a, G\<^sub>a))" and
-  prog_sim_pre_validity: " \<lbrakk>(\<Gamma>\<^sub>c, P\<^sub>c, R\<^sub>c, G\<^sub>c) \<preceq>\<^sub>p \<^sub>(\<^sub>\<alpha>\<^sub>;\<^sub>\<zeta>\<^sub>;\<^sub>\<xi>\<^sub>\<rhd>\<^sub>\<gamma>\<^sub>)  (\<Gamma>\<^sub>a, P\<^sub>a, R\<^sub>a, G\<^sub>a); (s\<^sub>c, s\<^sub>a) \<in> \<xi>\<rbrakk> \<Longrightarrow>  
-                           (\<Gamma>\<^sub>c, (P\<^sub>c, s\<^sub>c), R\<^sub>c, G\<^sub>c) \<preceq>\<^sub>p \<^sub>(\<^sub>\<alpha>\<^sub>;\<^sub>\<zeta>\<^sub>;\<^sub>\<gamma>\<^sub>) (\<Gamma>\<^sub>a, (P\<^sub>a, s\<^sub>a), R\<^sub>a, G\<^sub>a)"
+                            (\<forall>s\<^sub>c' s\<^sub>a'. ((s\<^sub>c, s\<^sub>c'),(s\<^sub>a, s\<^sub>a')) \<in> ((R\<^sub>c \<union> Id, R\<^sub>a \<union> Id)\<^sub>\<alpha>) \<longrightarrow> 
+                            (\<Gamma>\<^sub>c, (P\<^sub>c, s\<^sub>c'), R\<^sub>c, G\<^sub>c) \<preceq>\<^sub>p \<^sub>(\<^sub>\<alpha>\<^sub>;\<^sub>\<zeta>\<^sub>;\<^sub>\<gamma>\<^sub>) (\<Gamma>\<^sub>a, (P\<^sub>a, s\<^sub>a'), R\<^sub>a, G\<^sub>a))" 
 begin
-
-
-lemma prog_sim_pre_implies_inv : "(\<Gamma>\<^sub>c,P\<^sub>c,R\<^sub>c,G\<^sub>c) \<preceq>\<^sub>p \<^sub>(\<^sub>\<alpha>\<^sub>;\<^sub>\<zeta>\<^sub>;\<^sub>\<xi>\<^sub>\<rhd>\<^sub>\<gamma>\<^sub>)  (\<Gamma>\<^sub>a,P\<^sub>a,R\<^sub>a,G\<^sub>a) \<Longrightarrow> \<xi> \<subseteq> \<alpha>"
-  by (meson prog_sim_pre_validity prog_sim_validity subrelI)
 
 abbreviation ptran\<^sub>c' :: "'Env\<^sub>c \<Rightarrow> ('s\<^sub>c,'prog\<^sub>c) pconf \<Rightarrow> ('s\<^sub>c,'prog\<^sub>c) pconf \<Rightarrow> bool" ("_ \<turnstile>\<^sub>c _ -c\<rightarrow> _" [81,81] 80)
   where "ptran\<^sub>c' \<equiv> Event\<^sub>c.ptran'"
@@ -98,185 +90,415 @@ abbreviation pestran\<^sub>a :: "'Env\<^sub>a \<Rightarrow> ('l\<^sub>a,'k,'s\<^
                         ('l\<^sub>a,'k,'s\<^sub>a,'prog\<^sub>a) pesconf \<Rightarrow> bool" ("_ \<turnstile>\<^sub>a _ -pes-_\<rightarrow> _" [70,70] 60)
   where "pestran\<^sub>a \<equiv> Event\<^sub>a.pestran"
 
-coinductive e_sim :: "['Env\<^sub>c, ('l\<^sub>c,'k,'s\<^sub>c,'prog\<^sub>c) econf, ('s\<^sub>c \<times> 's\<^sub>c) set, ('s\<^sub>c \<times> 's\<^sub>c) set, 
-                  ('s\<^sub>c \<times> 's\<^sub>a) set, 'prog\<^sub>c \<Rightarrow> 'prog\<^sub>a option, ('s\<^sub>c \<times> 's\<^sub>a) set,
+coinductive e_sim :: "['Env\<^sub>c, ('l\<^sub>c,'k,'s\<^sub>c,'prog\<^sub>c) econf, ('s\<^sub>c \<times> 's\<^sub>c) set, ('s\<^sub>c \<times> 's\<^sub>c) set, 'k,
+                  ('s\<^sub>c \<times> 's\<^sub>a) set,
+                  ('l\<^sub>c,'k,'s\<^sub>c,'prog\<^sub>c) event \<Rightarrow> ('l\<^sub>a,'k,'s\<^sub>a,'prog\<^sub>a) event, 
+                  ('l\<^sub>c,'k,'s\<^sub>c,'prog\<^sub>c) event \<Rightarrow> 'prog\<^sub>c \<Rightarrow> 'prog\<^sub>a option, 
+                  ('s\<^sub>c \<times> 's\<^sub>a) set,
                   'Env\<^sub>a, ('l\<^sub>a,'k,'s\<^sub>a,'prog\<^sub>a) econf, ('s\<^sub>a \<times> 's\<^sub>a) set, ('s\<^sub>a \<times> 's\<^sub>a) set] \<Rightarrow> bool" 
-  ("'(_,_,_,_')/ \<preceq>\<^sub>e \<^sub>'(\<^sub>_\<^sub>;\<^sub>_\<^sub>;\<^sub>_\<^sub>') /'(_,_,_,_')" [81,81,81,81,81,81,81,81,81,81,81] 100)
+  ("'(_,_,_,_')/ \<preceq>\<^sub>e\<^sub>@\<^sub>_ \<^sub>'(\<^sub>_\<^sub>;\<^sub>_\<^sub>;\<^sub>_\<^sub>;\<^sub>_\<^sub>') /'(_,_,_,_')" [81,81,81,81,81,81,81,81,81,81,81,81] 100)
   where rgsim : "\<lbrakk>(s\<^sub>c, s\<^sub>a) \<in> \<alpha>; 
                   
-                  (\<forall>ec e\<^sub>c' x\<^sub>c' k. (\<Gamma>\<^sub>c \<turnstile>\<^sub>c (e\<^sub>c, s\<^sub>c, x\<^sub>c) -et-((EvtEnt ec)\<sharp>k)\<rightarrow> (e\<^sub>c', s\<^sub>c, x\<^sub>c')) \<longrightarrow> (\<exists>ea e\<^sub>a' x\<^sub>a'.
-                   (\<Gamma>\<^sub>a \<turnstile>\<^sub>a (e\<^sub>a, s\<^sub>a, x\<^sub>a) -et-((EvtEnt ea)\<sharp>k)\<rightarrow> (e\<^sub>a', s\<^sub>a, x\<^sub>a')) \<and>
-                   (\<Gamma>\<^sub>c, (e\<^sub>c', s\<^sub>c, x\<^sub>c'), R\<^sub>c, G\<^sub>c) \<preceq>\<^sub>e \<^sub>(\<^sub>\<alpha>\<^sub>;\<^sub>\<zeta>\<^sub>;\<^sub>\<gamma>\<^sub>) (\<Gamma>\<^sub>a, (e\<^sub>a', s\<^sub>a, x\<^sub>a'), R\<^sub>a, G\<^sub>a))) ;
+                  \<forall>ec e\<^sub>c' x\<^sub>c'. (\<Gamma>\<^sub>c \<turnstile>\<^sub>c (e\<^sub>c, s\<^sub>c, x\<^sub>c) -et-((EvtEnt ec)\<sharp>k)\<rightarrow> (e\<^sub>c', s\<^sub>c, x\<^sub>c')) \<longrightarrow> (\<exists>e\<^sub>a' x\<^sub>a'.
+                   (\<Gamma>\<^sub>a \<turnstile>\<^sub>a (e\<^sub>a, s\<^sub>a, x\<^sub>a) -et-((EvtEnt (\<eta> ec))\<sharp>k)\<rightarrow> (e\<^sub>a', s\<^sub>a, x\<^sub>a')) \<and>
+                   (\<Gamma>\<^sub>c, (e\<^sub>c', s\<^sub>c, x\<^sub>c'), R\<^sub>c, G\<^sub>c) \<preceq>\<^sub>e\<^sub>@\<^sub>k \<^sub>(\<^sub>\<alpha>\<^sub>;\<^sub>\<eta>\<^sub>;\<^sub>\<zeta>\<^sub>;\<^sub>\<gamma>\<^sub>) (\<Gamma>\<^sub>a, (e\<^sub>a', s\<^sub>a, x\<^sub>a'), R\<^sub>a, G\<^sub>a)) ;
 
-                   (\<forall>Pc e\<^sub>c' s\<^sub>c' k. (\<Gamma>\<^sub>c \<turnstile>\<^sub>c (e\<^sub>c, s\<^sub>c, x\<^sub>c) -et-((Cmd Pc)\<sharp>k)\<rightarrow> (e\<^sub>c', s\<^sub>c', x\<^sub>c)) \<and> \<zeta> Pc = None \<longrightarrow> 
-                   (s\<^sub>c, s\<^sub>c') \<in> G\<^sub>c \<and> (\<Gamma>\<^sub>c, (e\<^sub>c', s\<^sub>c', x\<^sub>c), R\<^sub>c, G\<^sub>c) \<preceq>\<^sub>e \<^sub>(\<^sub>\<alpha>\<^sub>;\<^sub>\<zeta>\<^sub>;\<^sub>\<gamma>\<^sub>) (\<Gamma>\<^sub>a, (e\<^sub>a, s\<^sub>a, x\<^sub>a), R\<^sub>a, G\<^sub>a)) ;
+                   \<forall>Pc e\<^sub>c' s\<^sub>c'. (\<Gamma>\<^sub>c \<turnstile>\<^sub>c (e\<^sub>c, s\<^sub>c, x\<^sub>c) -et-((Cmd Pc)\<sharp>k)\<rightarrow> (e\<^sub>c', s\<^sub>c', x\<^sub>c)) \<and> \<zeta> (x\<^sub>c k) Pc = None \<longrightarrow> 
+                   (s\<^sub>c, s\<^sub>c') \<in> G\<^sub>c \<and> (\<Gamma>\<^sub>c, (e\<^sub>c', s\<^sub>c', x\<^sub>c), R\<^sub>c, G\<^sub>c) \<preceq>\<^sub>e\<^sub>@\<^sub>k \<^sub>(\<^sub>\<alpha>\<^sub>;\<^sub>\<eta>\<^sub>;\<^sub>\<zeta>\<^sub>;\<^sub>\<gamma>\<^sub>) (\<Gamma>\<^sub>a, (e\<^sub>a, s\<^sub>a, x\<^sub>a), R\<^sub>a, G\<^sub>a) ;
 
-                  (\<forall>Pc e\<^sub>c' s\<^sub>c' k Pa. (\<Gamma>\<^sub>c \<turnstile>\<^sub>c (e\<^sub>c, s\<^sub>c, x\<^sub>c) -et-((Cmd Pc)\<sharp>k)\<rightarrow> (e\<^sub>c', s\<^sub>c', x\<^sub>c)) \<and> \<zeta> Pc = Some Pa \<longrightarrow> 
-                   (\<exists>e\<^sub>a' s\<^sub>a'. 
-                   (\<Gamma>\<^sub>a \<turnstile>\<^sub>a (e\<^sub>a, s\<^sub>a, x\<^sub>a) -et-((Cmd Pa)\<sharp>k)\<rightarrow> (e\<^sub>a', s\<^sub>a', x\<^sub>a)) \<and> (s\<^sub>c, s\<^sub>c') \<in> G\<^sub>c \<and> (s\<^sub>a, s\<^sub>a') \<in> G\<^sub>a \<and> 
-                   (\<Gamma>\<^sub>c, (e\<^sub>c', s\<^sub>c', x\<^sub>c), R\<^sub>c, G\<^sub>c) \<preceq>\<^sub>e \<^sub>(\<^sub>\<alpha>\<^sub>;\<^sub>\<zeta>\<^sub>;\<^sub>\<gamma>\<^sub>) (\<Gamma>\<^sub>a, (e\<^sub>a', s\<^sub>a', x\<^sub>a), R\<^sub>a, G\<^sub>a))) ;
+                  \<forall>Pc e\<^sub>c' s\<^sub>c' Pa. (\<Gamma>\<^sub>c \<turnstile>\<^sub>c (e\<^sub>c, s\<^sub>c, x\<^sub>c) -et-((Cmd Pc)\<sharp>k)\<rightarrow> (e\<^sub>c', s\<^sub>c', x\<^sub>c)) \<and> \<zeta> (x\<^sub>c k) Pc = Some Pa \<longrightarrow> 
+                  \<eta> (x\<^sub>c k) = x\<^sub>a k \<and> (\<exists>e\<^sub>a' s\<^sub>a'. 
+                  (\<Gamma>\<^sub>a \<turnstile>\<^sub>a (e\<^sub>a, s\<^sub>a, x\<^sub>a) -et-((Cmd Pa)\<sharp>k)\<rightarrow> (e\<^sub>a', s\<^sub>a', x\<^sub>a)) \<and> (s\<^sub>c, s\<^sub>c') \<in> G\<^sub>c \<and> (s\<^sub>a, s\<^sub>a') \<in> G\<^sub>a \<and> 
+                  (\<Gamma>\<^sub>c, (e\<^sub>c', s\<^sub>c', x\<^sub>c), R\<^sub>c, G\<^sub>c) \<preceq>\<^sub>e\<^sub>@\<^sub>k \<^sub>(\<^sub>\<alpha>\<^sub>;\<^sub>\<eta>\<^sub>;\<^sub>\<zeta>\<^sub>;\<^sub>\<gamma>\<^sub>) (\<Gamma>\<^sub>a, (e\<^sub>a', s\<^sub>a', x\<^sub>a), R\<^sub>a, G\<^sub>a)) ;
 
 
-                   (e\<^sub>c = AnonyEvent fin_com\<^sub>c \<longrightarrow> e\<^sub>a = AnonyEvent fin_com\<^sub>a \<and> (s\<^sub>c, s\<^sub>a) \<in> \<gamma> \<and> \<gamma> \<subseteq> \<alpha>) ; 
+                   e\<^sub>c = AnonyEvent fin_com\<^sub>c \<longrightarrow> e\<^sub>a = AnonyEvent fin_com\<^sub>a \<and> (s\<^sub>c, s\<^sub>a) \<in> \<gamma> \<and> \<gamma> \<subseteq> \<alpha>;
 
-                   (\<forall>s\<^sub>c' s\<^sub>a' x\<^sub>c' x\<^sub>a'. ((s\<^sub>c, s\<^sub>c'), (s\<^sub>a, s\<^sub>a')) \<in> ((R\<^sub>c, R\<^sub>a \<union> Id)\<^sub>\<alpha>) \<longrightarrow> 
-                     (\<Gamma>\<^sub>c, (e\<^sub>c, s\<^sub>c', x\<^sub>c'), R\<^sub>c, G\<^sub>c) \<preceq>\<^sub>e \<^sub>(\<^sub>\<alpha>\<^sub>;\<^sub>\<zeta>\<^sub>;\<^sub>\<gamma>\<^sub>) (\<Gamma>\<^sub>a, (e\<^sub>a, s\<^sub>a', x\<^sub>a'), R\<^sub>a, G\<^sub>a))      
-                  \<rbrakk> \<Longrightarrow> (\<Gamma>\<^sub>c, (e\<^sub>c, s\<^sub>c, x\<^sub>c), R\<^sub>c, G\<^sub>c) \<preceq>\<^sub>e \<^sub>(\<^sub>\<alpha>\<^sub>;\<^sub>\<zeta>\<^sub>;\<^sub>\<gamma>\<^sub>) (\<Gamma>\<^sub>a, (e\<^sub>a, s\<^sub>a, x\<^sub>a), R\<^sub>a, G\<^sub>a)"
+                   e\<^sub>c \<noteq> AnonyEvent fin_com\<^sub>c \<longrightarrow> e\<^sub>a \<noteq> AnonyEvent fin_com\<^sub>a;
 
-definition e_sim_pre :: "['Env\<^sub>c, ('l\<^sub>c,'k,'s\<^sub>c,'prog\<^sub>c) event, ('s\<^sub>c \<times> 's\<^sub>c) set, ('s\<^sub>c \<times> 's\<^sub>c) set, 
-                  ('s\<^sub>c \<times> 's\<^sub>a) set, 'prog\<^sub>c \<Rightarrow> 'prog\<^sub>a option, ('s\<^sub>c \<times> 's\<^sub>a) set, ('s\<^sub>c \<times> 's\<^sub>a) set,
-                  'Env\<^sub>a, ('l\<^sub>a,'k,'s\<^sub>a,'prog\<^sub>a) event, ('s\<^sub>a \<times> 's\<^sub>a) set, ('s\<^sub>a \<times> 's\<^sub>a) set] \<Rightarrow> bool" 
-  ("'(_,_,_,_')/ \<preceq>\<^sub>e \<^sub>'(\<^sub>_\<^sub>;\<^sub>_\<^sub>;\<^sub>_\<^sub>\<rhd>\<^sub>_\<^sub>') /'(_,_,_,_')" [81,81,81,81,81,81,81,81,81,81,81] 100)
-  where "(\<Gamma>\<^sub>c, e\<^sub>c, R\<^sub>c, G\<^sub>c) \<preceq>\<^sub>e \<^sub>(\<^sub>\<alpha>\<^sub>;\<^sub>\<zeta>\<^sub>;\<^sub>\<xi>\<^sub>\<rhd>\<^sub>\<gamma>\<^sub>)  (\<Gamma>\<^sub>a, e\<^sub>a, R\<^sub>a, G\<^sub>a) = (\<forall>s\<^sub>c s\<^sub>a x\<^sub>c x\<^sub>a. (s\<^sub>c, s\<^sub>a) \<in> \<xi> \<longrightarrow> 
-         (\<Gamma>\<^sub>c, (e\<^sub>c, s\<^sub>c, x\<^sub>c), R\<^sub>c, G\<^sub>c) \<preceq>\<^sub>e \<^sub>(\<^sub>\<alpha>\<^sub>;\<^sub>\<zeta>\<^sub>;\<^sub>\<gamma>\<^sub>) (\<Gamma>\<^sub>a, (e\<^sub>a, s\<^sub>a, x\<^sub>a), R\<^sub>a, G\<^sub>a))"
+                   \<forall>s\<^sub>c' s\<^sub>a' x\<^sub>c' x\<^sub>a'. ((s\<^sub>c, s\<^sub>c'),(s\<^sub>a, s\<^sub>a')) \<in> ((R\<^sub>c \<union> Id, R\<^sub>a \<union> Id)\<^sub>\<alpha>) \<longrightarrow>(x\<^sub>c' k = x\<^sub>c k \<and> x\<^sub>a' k = x\<^sub>a k)
+                    \<longrightarrow> (\<Gamma>\<^sub>c, (e\<^sub>c, s\<^sub>c', x\<^sub>c'), R\<^sub>c, G\<^sub>c) \<preceq>\<^sub>e\<^sub>@\<^sub>k \<^sub>(\<^sub>\<alpha>\<^sub>;\<^sub>\<eta>\<^sub>;\<^sub>\<zeta>\<^sub>;\<^sub>\<gamma>\<^sub>) (\<Gamma>\<^sub>a, (e\<^sub>a, s\<^sub>a', x\<^sub>a'), R\<^sub>a, G\<^sub>a)      
+                  \<rbrakk> \<Longrightarrow> (\<Gamma>\<^sub>c, (e\<^sub>c, s\<^sub>c, x\<^sub>c), R\<^sub>c, G\<^sub>c) \<preceq>\<^sub>e\<^sub>@\<^sub>k \<^sub>(\<^sub>\<alpha>\<^sub>;\<^sub>\<eta>\<^sub>;\<^sub>\<zeta>\<^sub>;\<^sub>\<gamma>\<^sub>) (\<Gamma>\<^sub>a, (e\<^sub>a, s\<^sub>a, x\<^sub>a), R\<^sub>a, G\<^sub>a)"
 
-lemma e_sim_init :"(\<Gamma>\<^sub>c,(e\<^sub>c, s\<^sub>c, x\<^sub>c),R\<^sub>c,G\<^sub>c) \<preceq>\<^sub>e \<^sub>(\<^sub>\<alpha>\<^sub>;\<^sub>\<zeta>\<^sub>;\<^sub>\<gamma>\<^sub>) (\<Gamma>\<^sub>a,(e\<^sub>a, s\<^sub>a, x\<^sub>a),R\<^sub>a,G\<^sub>a) \<Longrightarrow> (s\<^sub>c, s\<^sub>a) \<in> \<alpha>"
+lemma e_sim_init :"(\<Gamma>\<^sub>c,(e\<^sub>c, s\<^sub>c, x\<^sub>c),R\<^sub>c,G\<^sub>c) \<preceq>\<^sub>e\<^sub>@\<^sub>k \<^sub>(\<^sub>\<alpha>\<^sub>;\<^sub>\<eta>\<^sub>;\<^sub>\<zeta>\<^sub>;\<^sub>\<gamma>\<^sub>) (\<Gamma>\<^sub>a,(e\<^sub>a, s\<^sub>a, x\<^sub>a),R\<^sub>a,G\<^sub>a) \<Longrightarrow> (s\<^sub>c, s\<^sub>a) \<in> \<alpha>"
   by (erule e_sim.cases, simp_all)
 
-lemma e_sim_pre_implies_inv : "(\<Gamma>\<^sub>c, e\<^sub>c, R\<^sub>c, G\<^sub>c) \<preceq>\<^sub>e \<^sub>(\<^sub>\<alpha>\<^sub>;\<^sub>\<zeta>\<^sub>;\<^sub>\<xi>\<^sub>\<rhd>\<^sub>\<gamma>\<^sub>)  (\<Gamma>\<^sub>a, e\<^sub>a, R\<^sub>a, G\<^sub>a) \<Longrightarrow> \<xi> \<subseteq> \<alpha>"
-  by (meson e_sim_pre_def PiCore_Sim_axioms e_sim_init subrelI)
 
-lemma AnonyEvt_Sound_help1: "\<lbrakk>(\<Gamma>\<^sub>c,(P\<^sub>c, s\<^sub>c),R\<^sub>c,G\<^sub>c) \<preceq>\<^sub>p \<^sub>(\<^sub>\<alpha>\<^sub>;\<^sub>\<zeta>\<^sub>;\<^sub>\<gamma>\<^sub>) (\<Gamma>\<^sub>a,(P\<^sub>a, s\<^sub>a),R\<^sub>a,G\<^sub>a); 
+lemma AnonyEvt_Sound_lemma1: "\<lbrakk>(\<Gamma>\<^sub>c,(P\<^sub>c, s\<^sub>c),R\<^sub>c,G\<^sub>c) \<preceq>\<^sub>p \<^sub>(\<^sub>\<alpha>\<^sub>;\<^sub>\<zeta>\<^sub>;\<^sub>\<gamma>\<^sub>) (\<Gamma>\<^sub>a,(P\<^sub>a, s\<^sub>a),R\<^sub>a,G\<^sub>a); 
       \<Gamma>\<^sub>c \<turnstile>\<^sub>c (AnonyEvent P\<^sub>c, s\<^sub>c, x\<^sub>c) -et-Cmd Pc\<sharp>k\<rightarrow> (e\<^sub>c', s\<^sub>c', x\<^sub>c); \<zeta> Pc = None\<rbrakk> 
       \<Longrightarrow> (s\<^sub>c, s\<^sub>c') \<in> G\<^sub>c \<and> (\<exists>P\<^sub>c'. e\<^sub>c' = AnonyEvent P\<^sub>c' \<and> (\<Gamma>\<^sub>c,(P\<^sub>c', s\<^sub>c'),R\<^sub>c,G\<^sub>c) \<preceq>\<^sub>p \<^sub>(\<^sub>\<alpha>\<^sub>;\<^sub>\<zeta>\<^sub>;\<^sub>\<gamma>\<^sub>) (\<Gamma>\<^sub>a,(P\<^sub>a, s\<^sub>a),R\<^sub>a,G\<^sub>a))"
 proof-
   assume a0: "(\<Gamma>\<^sub>c,(P\<^sub>c, s\<^sub>c),R\<^sub>c,G\<^sub>c) \<preceq>\<^sub>p \<^sub>(\<^sub>\<alpha>\<^sub>;\<^sub>\<zeta>\<^sub>;\<^sub>\<gamma>\<^sub>) (\<Gamma>\<^sub>a,(P\<^sub>a, s\<^sub>a),R\<^sub>a,G\<^sub>a)"
      and a1: "\<Gamma>\<^sub>c \<turnstile>\<^sub>c (AnonyEvent P\<^sub>c, s\<^sub>c, x\<^sub>c) -et-Cmd Pc\<sharp>k\<rightarrow> (e\<^sub>c', s\<^sub>c', x\<^sub>c)"
      and a2: "\<zeta> Pc = None"
-  from a1 have "(Pc = P\<^sub>c) \<and> (\<exists>P\<^sub>c'. \<Gamma>\<^sub>c \<turnstile>\<^sub>c (P\<^sub>c, s\<^sub>c) -c\<rightarrow> (P\<^sub>c', s\<^sub>c') \<and> e\<^sub>c' = AnonyEvent P\<^sub>c')"
+  from a1 have "(Pc = P\<^sub>c) \<and> (\<exists>P\<^sub>c'. (\<Gamma>\<^sub>c \<turnstile>\<^sub>c (P\<^sub>c, s\<^sub>c) -c\<rightarrow> (P\<^sub>c', s\<^sub>c')) \<and> e\<^sub>c' = AnonyEvent P\<^sub>c')"
     apply (rule Event\<^sub>c.etran.cases, simp_all)
     by (metis act.inject(1) actk.ext_inject get_actk_def)
-  then obtain P\<^sub>c' where a3: "Pc = P\<^sub>c \<and> \<Gamma>\<^sub>c \<turnstile>\<^sub>c (P\<^sub>c, s\<^sub>c) -c\<rightarrow> (P\<^sub>c', s\<^sub>c') \<and> e\<^sub>c' = AnonyEvent P\<^sub>c'" by auto
+  then obtain P\<^sub>c' where a3: "Pc = P\<^sub>c \<and> (\<Gamma>\<^sub>c \<turnstile>\<^sub>c (P\<^sub>c, s\<^sub>c) -c\<rightarrow> (P\<^sub>c', s\<^sub>c')) \<and> e\<^sub>c' = AnonyEvent P\<^sub>c'" by auto
   with a0 a2 have "(s\<^sub>c, s\<^sub>c') \<in> G\<^sub>c \<and> (\<Gamma>\<^sub>c, (P\<^sub>c', s\<^sub>c'), R\<^sub>c, G\<^sub>c) \<preceq>\<^sub>p \<^sub>(\<^sub>\<alpha>\<^sub>;\<^sub>\<zeta>\<^sub>;\<^sub>\<gamma>\<^sub>) (\<Gamma>\<^sub>a, (P\<^sub>a, s\<^sub>a), R\<^sub>a, G\<^sub>a)"
     by (meson Event\<^sub>c.ptran'_def prog_sim_validity)
   then show ?thesis
     by (simp add: a3)
 qed
 
-lemma AnonyEvt_Sound_help2: "\<lbrakk>(\<Gamma>\<^sub>c,(P\<^sub>c, s\<^sub>c),R\<^sub>c,G\<^sub>c) \<preceq>\<^sub>p \<^sub>(\<^sub>\<alpha>\<^sub>;\<^sub>\<zeta>\<^sub>;\<^sub>\<gamma>\<^sub>) (\<Gamma>\<^sub>a,(P\<^sub>a, s\<^sub>a),R\<^sub>a,G\<^sub>a); 
+lemma AnonyEvt_Sound_lemma2: "\<lbrakk>(\<Gamma>\<^sub>c,(P\<^sub>c, s\<^sub>c),R\<^sub>c,G\<^sub>c) \<preceq>\<^sub>p \<^sub>(\<^sub>\<alpha>\<^sub>;\<^sub>\<zeta>\<^sub>;\<^sub>\<gamma>\<^sub>) (\<Gamma>\<^sub>a,(P\<^sub>a, s\<^sub>a),R\<^sub>a,G\<^sub>a); 
       \<Gamma>\<^sub>c \<turnstile>\<^sub>c (AnonyEvent P\<^sub>c, s\<^sub>c, x\<^sub>c) -et-Cmd Pc\<sharp>k\<rightarrow> (e\<^sub>c', s\<^sub>c', x\<^sub>c); \<zeta> Pc = Some Pa\<rbrakk> 
-      \<Longrightarrow> \<exists>e\<^sub>a' s\<^sub>a'. \<Gamma>\<^sub>a \<turnstile>\<^sub>a (AnonyEvent P\<^sub>a, s\<^sub>a, x\<^sub>a) -et-Cmd Pa\<sharp>k\<rightarrow> (e\<^sub>a', s\<^sub>a', x\<^sub>a) \<and>
+      \<Longrightarrow> \<exists>e\<^sub>a' s\<^sub>a'. (\<Gamma>\<^sub>a \<turnstile>\<^sub>a (AnonyEvent P\<^sub>a, s\<^sub>a, x\<^sub>a) -et-Cmd Pa\<sharp>k\<rightarrow> (e\<^sub>a', s\<^sub>a', x\<^sub>a)) \<and>
           (s\<^sub>c, s\<^sub>c') \<in> G\<^sub>c \<and> (s\<^sub>a, s\<^sub>a') \<in> G\<^sub>a \<and> (\<exists>P\<^sub>c. e\<^sub>c' = AnonyEvent P\<^sub>c \<and> (\<exists>P\<^sub>a'. e\<^sub>a' = AnonyEvent P\<^sub>a'
           \<and> (\<Gamma>\<^sub>c,(P\<^sub>c, s\<^sub>c'),R\<^sub>c,G\<^sub>c) \<preceq>\<^sub>p \<^sub>(\<^sub>\<alpha>\<^sub>;\<^sub>\<zeta>\<^sub>;\<^sub>\<gamma>\<^sub>) (\<Gamma>\<^sub>a,(P\<^sub>a', s\<^sub>a'),R\<^sub>a,G\<^sub>a)))"
 proof-
   assume a0: "(\<Gamma>\<^sub>c,(P\<^sub>c, s\<^sub>c),R\<^sub>c,G\<^sub>c) \<preceq>\<^sub>p \<^sub>(\<^sub>\<alpha>\<^sub>;\<^sub>\<zeta>\<^sub>;\<^sub>\<gamma>\<^sub>) (\<Gamma>\<^sub>a,(P\<^sub>a, s\<^sub>a),R\<^sub>a,G\<^sub>a)"
      and a1: "\<Gamma>\<^sub>c \<turnstile>\<^sub>c (AnonyEvent P\<^sub>c, s\<^sub>c, x\<^sub>c) -et-Cmd Pc\<sharp>k\<rightarrow> (e\<^sub>c', s\<^sub>c', x\<^sub>c)"
      and a2: "\<zeta> Pc = Some Pa"  
-  from a1 have "Pc = P\<^sub>c \<and> (\<exists>P\<^sub>c'. \<Gamma>\<^sub>c \<turnstile>\<^sub>c (P\<^sub>c, s\<^sub>c) -c\<rightarrow> (P\<^sub>c', s\<^sub>c') \<and> e\<^sub>c' = AnonyEvent P\<^sub>c')"
+  from a1 have "Pc = P\<^sub>c \<and> (\<exists>P\<^sub>c'. (\<Gamma>\<^sub>c \<turnstile>\<^sub>c (P\<^sub>c, s\<^sub>c) -c\<rightarrow> (P\<^sub>c', s\<^sub>c')) \<and> e\<^sub>c' = AnonyEvent P\<^sub>c')"
     apply (rule Event\<^sub>c.etran.cases, simp_all)
     by (metis act.inject(1) actk.ext_inject get_actk_def)
-  then obtain P\<^sub>c' where a3: "Pc = P\<^sub>c \<and> \<Gamma>\<^sub>c \<turnstile>\<^sub>c (P\<^sub>c, s\<^sub>c) -c\<rightarrow> (P\<^sub>c', s\<^sub>c') \<and> e\<^sub>c' = AnonyEvent P\<^sub>c'" by auto
-  with a0 have "\<zeta> P\<^sub>c = Some P\<^sub>a \<and> (\<exists>P\<^sub>a' s\<^sub>a'. \<Gamma>\<^sub>a \<turnstile>\<^sub>a (P\<^sub>a, s\<^sub>a) -c\<rightarrow> (P\<^sub>a', s\<^sub>a')
+  then obtain P\<^sub>c' where a3: "Pc = P\<^sub>c \<and> (\<Gamma>\<^sub>c \<turnstile>\<^sub>c (P\<^sub>c, s\<^sub>c) -c\<rightarrow> (P\<^sub>c', s\<^sub>c')) \<and> e\<^sub>c' = AnonyEvent P\<^sub>c'" by auto
+  with a0 have "\<zeta> P\<^sub>c = Some P\<^sub>a \<and> (\<exists>P\<^sub>a' s\<^sub>a'. (\<Gamma>\<^sub>a \<turnstile>\<^sub>a (P\<^sub>a, s\<^sub>a) -c\<rightarrow> (P\<^sub>a', s\<^sub>a'))
   \<and> (s\<^sub>c, s\<^sub>c') \<in> G\<^sub>c \<and> (s\<^sub>a, s\<^sub>a') \<in> G\<^sub>a \<and> (\<Gamma>\<^sub>c, (P\<^sub>c', s\<^sub>c'), R\<^sub>c, G\<^sub>c) \<preceq>\<^sub>p \<^sub>(\<^sub>\<alpha>\<^sub>;\<^sub>\<zeta>\<^sub>;\<^sub>\<gamma>\<^sub>) (\<Gamma>\<^sub>a, (P\<^sub>a', s\<^sub>a'), R\<^sub>a, G\<^sub>a))"
     by (smt (verit, best) Event\<^sub>a.ptran'_def Event\<^sub>c.ptran'_def a2 option.distinct(1) prog_sim_validity)
-  then obtain P\<^sub>a' s\<^sub>a' where a4: "\<zeta> P\<^sub>c = Some P\<^sub>a \<and> \<Gamma>\<^sub>a \<turnstile>\<^sub>a (P\<^sub>a, s\<^sub>a) -c\<rightarrow> (P\<^sub>a', s\<^sub>a')\<and> (s\<^sub>c, s\<^sub>c') \<in> G\<^sub>c 
+  then obtain P\<^sub>a' s\<^sub>a' where a4: "\<zeta> P\<^sub>c = Some P\<^sub>a \<and> (\<Gamma>\<^sub>a \<turnstile>\<^sub>a (P\<^sub>a, s\<^sub>a) -c\<rightarrow> (P\<^sub>a', s\<^sub>a')) \<and> (s\<^sub>c, s\<^sub>c') \<in> G\<^sub>c 
   \<and> (s\<^sub>a, s\<^sub>a') \<in> G\<^sub>a \<and> (\<Gamma>\<^sub>c, (P\<^sub>c', s\<^sub>c'), R\<^sub>c, G\<^sub>c) \<preceq>\<^sub>p \<^sub>(\<^sub>\<alpha>\<^sub>;\<^sub>\<zeta>\<^sub>;\<^sub>\<gamma>\<^sub>) (\<Gamma>\<^sub>a, (P\<^sub>a', s\<^sub>a'), R\<^sub>a, G\<^sub>a)" by auto
   with a2 a3 show ?thesis by (metis Event\<^sub>a.AnonyEvent option.inject)
 qed
 
-lemma AnonyEvt_Sound_lemma : "(\<Gamma>\<^sub>c, (P\<^sub>c, s\<^sub>c), R\<^sub>c, G\<^sub>c) \<preceq>\<^sub>p \<^sub>(\<^sub>\<alpha>\<^sub>;\<^sub>\<zeta>\<^sub>;\<^sub>\<gamma>\<^sub>) (\<Gamma>\<^sub>a, (P\<^sub>a, s\<^sub>a), R\<^sub>a, G\<^sub>a)  \<Longrightarrow>
-       (\<Gamma>\<^sub>c, (AnonyEvent P\<^sub>c, s\<^sub>c, x\<^sub>c), R\<^sub>c, G\<^sub>c) \<preceq>\<^sub>e \<^sub>(\<^sub>\<alpha>\<^sub>;\<^sub>\<zeta>\<^sub>;\<^sub>\<gamma>\<^sub>) (\<Gamma>\<^sub>a, (AnonyEvent P\<^sub>a, s\<^sub>a, x\<^sub>a), R\<^sub>a, G\<^sub>a)"
+
+lemma AnonyEvt_Rule : "\<lbrakk>(\<Gamma>\<^sub>c, (P\<^sub>c, s\<^sub>c), R\<^sub>c, G\<^sub>c) \<preceq>\<^sub>p \<^sub>(\<^sub>\<alpha>\<^sub>;\<^sub>\<sigma>\<^sub>;\<^sub>\<gamma>\<^sub>) (\<Gamma>\<^sub>a, (P\<^sub>a, s\<^sub>a), R\<^sub>a, G\<^sub>a); \<sigma> = \<zeta> (x\<^sub>c k); \<eta> (x\<^sub>c k) = x\<^sub>a k\<rbrakk>  \<Longrightarrow> 
+       (\<Gamma>\<^sub>c, (AnonyEvent P\<^sub>c, s\<^sub>c, x\<^sub>c), R\<^sub>c, G\<^sub>c) \<preceq>\<^sub>e\<^sub>@\<^sub>k \<^sub>(\<^sub>\<alpha>\<^sub>;\<^sub>\<eta>\<^sub>;\<^sub>\<zeta>\<^sub>;\<^sub>\<gamma>\<^sub>) (\<Gamma>\<^sub>a, (AnonyEvent P\<^sub>a, s\<^sub>a, x\<^sub>a), R\<^sub>a, G\<^sub>a)"
   apply (coinduction arbitrary: P\<^sub>c s\<^sub>c x\<^sub>c P\<^sub>a s\<^sub>a x\<^sub>a, clarsimp)
   apply (rule conjI)
   using prog_sim_validity apply blast
   apply (rule conjI)
    apply (metis Event\<^sub>c.EvtSeq1 Event\<^sub>c.EvtSeq2 Event\<^sub>c.ent_spec1 Event\<^sub>c.evtent_is_basicevt event.distinct(1))
   apply (rule conjI, clarsimp)
-  apply (simp add: AnonyEvt_Sound_help1)
+  apply (simp add: AnonyEvt_Sound_lemma1)
   apply (rule conjI, clarsimp)
-  using AnonyEvt_Sound_help2 apply fastforce
+  using AnonyEvt_Sound_lemma2 apply fastforce
   apply (rule conjI)
   using prog_sim_validity apply blast
   using prog_sim_validity by blast
 
-theorem AnonyEvent_rule : "(\<Gamma>\<^sub>c, P\<^sub>c, R\<^sub>c, G\<^sub>c) \<preceq>\<^sub>p \<^sub>(\<^sub>\<alpha>\<^sub>;\<^sub>\<zeta>\<^sub>;\<^sub>\<xi>\<^sub>\<rhd>\<^sub>\<gamma>\<^sub>)  (\<Gamma>\<^sub>a, P\<^sub>a, R\<^sub>a, G\<^sub>a) \<Longrightarrow>  
-                            (\<Gamma>\<^sub>c, AnonyEvent P\<^sub>c, R\<^sub>c, G\<^sub>c) \<preceq>\<^sub>e \<^sub>(\<^sub>\<alpha>\<^sub>;\<^sub>\<zeta>\<^sub>;\<^sub>\<xi>\<^sub>\<rhd>\<^sub>\<gamma>\<^sub>)  (\<Gamma>\<^sub>a, AnonyEvent P\<^sub>a, R\<^sub>a, G\<^sub>a)"
-  by (simp add: AnonyEvt_Sound_lemma e_sim_pre_def prog_sim_pre_validity)
-
-lemma BasicEvent_Sound_lemma : "\<lbrakk>(\<Gamma>\<^sub>c,P\<^sub>c,R\<^sub>c,G\<^sub>c) \<preceq>\<^sub>p \<^sub>(\<^sub>\<alpha>\<^sub>;\<^sub>\<zeta>\<^sub>;\<^sub>\<eta>\<^sub>\<rhd>\<^sub>\<gamma>\<^sub>)  (\<Gamma>\<^sub>a,P\<^sub>a,R\<^sub>a,G\<^sub>a); \<xi> \<subseteq> g\<^sub>c \<rightleftharpoons>\<^sub>r g\<^sub>a; (s\<^sub>c, s\<^sub>a) \<in> \<xi>;
-       \<eta> = \<xi> \<inter> (g\<^sub>c\<and>\<^sub>rg\<^sub>a); \<Gamma>\<^sub>c \<turnstile>\<^sub>c (BasicEvent (l\<^sub>c, g\<^sub>c, P\<^sub>c), s\<^sub>c, x\<^sub>c) -et-EvtEnt ec\<sharp>k\<rightarrow> (e\<^sub>c', s\<^sub>c, x\<^sub>c'); P\<^sub>a \<noteq> fin_com\<^sub>a \<rbrakk> \<Longrightarrow> 
-       \<exists>ea e\<^sub>a' x\<^sub>a'. (\<Gamma>\<^sub>a \<turnstile>\<^sub>a (BasicEvent (l\<^sub>a, g\<^sub>a, P\<^sub>a), s\<^sub>a, x\<^sub>a) -et-EvtEnt ea\<sharp>k\<rightarrow> (e\<^sub>a', s\<^sub>a, x\<^sub>a')) \<and>
-       (\<Gamma>\<^sub>c,(e\<^sub>c', s\<^sub>c, x\<^sub>c'),R\<^sub>c,G\<^sub>c) \<preceq>\<^sub>e \<^sub>(\<^sub>\<alpha>\<^sub>;\<^sub>\<zeta>\<^sub>;\<^sub>\<gamma>\<^sub>) (\<Gamma>\<^sub>a,(e\<^sub>a', s\<^sub>a, x\<^sub>a'),R\<^sub>a,G\<^sub>a)"
-proof-
-  assume a0: "(\<Gamma>\<^sub>c,P\<^sub>c,R\<^sub>c,G\<^sub>c) \<preceq>\<^sub>p \<^sub>(\<^sub>\<alpha>\<^sub>;\<^sub>\<zeta>\<^sub>;\<^sub>\<eta>\<^sub>\<rhd>\<^sub>\<gamma>\<^sub>)  (\<Gamma>\<^sub>a,P\<^sub>a,R\<^sub>a,G\<^sub>a)"
-     and a1: "\<xi> \<subseteq> g\<^sub>c \<rightleftharpoons>\<^sub>r g\<^sub>a"
-     and a2: "(s\<^sub>c, s\<^sub>a) \<in> \<xi>"
-     and a3: "\<eta> = \<xi> \<inter> (g\<^sub>c\<and>\<^sub>rg\<^sub>a)"
-     and a4: "\<Gamma>\<^sub>c \<turnstile>\<^sub>c (BasicEvent (l\<^sub>c, g\<^sub>c, P\<^sub>c), s\<^sub>c, x\<^sub>c) -et-EvtEnt ec\<sharp>k\<rightarrow> (e\<^sub>c', s\<^sub>c, x\<^sub>c')"
-     and a5: "P\<^sub>a \<noteq> fin_com\<^sub>a"
-  from a4 have a6: "s\<^sub>c \<in> g\<^sub>c \<and> e\<^sub>c' = AnonyEvent P\<^sub>c " 
-    apply (rule Event\<^sub>c.etran.cases, simp_all)
-    using guard_def body_def by (metis fstI sndI)
-  with a1 a2 have a7 : "s\<^sub>a \<in> g\<^sub>a" 
-    by (smt (verit, ccfv_SIG) CollectD case_prodE fst_conv rel_guard_eq_def snd_conv subsetD)
-  with a5 have a8: "\<Gamma>\<^sub>a \<turnstile>\<^sub>a (BasicEvent (l\<^sub>a, g\<^sub>a, P\<^sub>a), s\<^sub>a, x\<^sub>a) -et-EvtEnt (BasicEvent (l\<^sub>a, g\<^sub>a, P\<^sub>a))\<sharp>k\<rightarrow> 
-                   (AnonyEvent P\<^sub>a, s\<^sub>a, x\<^sub>a(k := BasicEvent (l\<^sub>a, g\<^sub>a, P\<^sub>a)))"
-    by (rule_tac Event\<^sub>a.EventEntry, simp_all add: body_def guard_def)
-  from a2 a3 a6 a7 have "(s\<^sub>c, s\<^sub>a) \<in> \<eta>"
-    by (simp add: rel_guard_and_def)
-  with a0 have "(\<Gamma>\<^sub>c, (P\<^sub>c, s\<^sub>c), R\<^sub>c, G\<^sub>c) \<preceq>\<^sub>p \<^sub>(\<^sub>\<alpha>\<^sub>;\<^sub>\<zeta>\<^sub>;\<^sub>\<gamma>\<^sub>)  (\<Gamma>\<^sub>a, (P\<^sub>a, s\<^sub>a), R\<^sub>a, G\<^sub>a)"
-    by (rule_tac \<xi> = \<eta> in prog_sim_pre_validity, simp_all)
-  then have "(\<Gamma>\<^sub>c, (AnonyEvent P\<^sub>c, s\<^sub>c, x\<^sub>c'), R\<^sub>c, G\<^sub>c) \<preceq>\<^sub>e \<^sub>(\<^sub>\<alpha>\<^sub>;\<^sub>\<zeta>\<^sub>;\<^sub>\<gamma>\<^sub>)  (\<Gamma>\<^sub>a, (AnonyEvent P\<^sub>a, s\<^sub>a, x\<^sub>a(k := BasicEvent (l\<^sub>a, g\<^sub>a, P\<^sub>a))), R\<^sub>a, G\<^sub>a)"
-    by (simp add: AnonyEvt_Sound_lemma)
-  then show ?thesis
-    using a6 a8 by blast
-qed
-
-theorem BasicEvent_rule : "\<lbrakk>(\<Gamma>\<^sub>c, P\<^sub>c, R\<^sub>c, G\<^sub>c) \<preceq>\<^sub>p \<^sub>(\<^sub>\<alpha>\<^sub>;\<^sub>\<zeta>\<^sub>;\<^sub>\<eta>\<^sub>\<rhd>\<^sub>\<gamma>\<^sub>)  (\<Gamma>\<^sub>a, P\<^sub>a, R\<^sub>a, G\<^sub>a); \<xi> \<subseteq> g\<^sub>c \<rightleftharpoons>\<^sub>r g\<^sub>a; P\<^sub>a \<noteq> fin_com\<^sub>a; 
-      \<eta> = \<xi> \<inter> (g\<^sub>c \<and>\<^sub>r g\<^sub>a); Stable \<eta> ((R\<^sub>c, R\<^sub>a \<union> Id)\<^sub>\<alpha>); Stable \<xi> ((R\<^sub>c, R\<^sub>a \<union> Id)\<^sub>\<alpha>); \<xi> \<subseteq> \<alpha> \<rbrakk> \<Longrightarrow>
-      (\<Gamma>\<^sub>c, BasicEvent (l\<^sub>c, g\<^sub>c, P\<^sub>c), R\<^sub>c, G\<^sub>c) \<preceq>\<^sub>e \<^sub>(\<^sub>\<alpha>\<^sub>;\<^sub>\<zeta>\<^sub>;\<^sub>\<xi>\<^sub>\<rhd>\<^sub>\<gamma>\<^sub>)  (\<Gamma>\<^sub>a, BasicEvent (l\<^sub>a, g\<^sub>a, P\<^sub>a), R\<^sub>a, G\<^sub>a)"
-  apply (simp add: e_sim_pre_def, clarify)
-  apply (coinduction arbitrary: P\<^sub>c P\<^sub>a, clarsimp)
+theorem BasicEvt_Rule: "\<lbrakk>\<xi> \<subseteq> g\<^sub>c \<rightleftharpoons>\<^sub>r g\<^sub>a; \<xi> \<subseteq> \<alpha>; Stable \<xi> ((R\<^sub>c \<union> Id, R\<^sub>a \<union> Id)\<^sub>\<alpha>); (s\<^sub>c, s\<^sub>a) \<in> \<xi>;
+    \<eta> (BasicEvent (l\<^sub>c, g\<^sub>c, P\<^sub>c)) = BasicEvent (l\<^sub>a, g\<^sub>a, P\<^sub>a); \<sigma> = \<zeta> (BasicEvent (l\<^sub>c, g\<^sub>c, P\<^sub>c));
+    \<forall>s\<^sub>c s\<^sub>a. (s\<^sub>c, s\<^sub>a) \<in> \<xi> \<inter> (g\<^sub>c \<and>\<^sub>r g\<^sub>a) \<longrightarrow> (\<Gamma>\<^sub>c, (P\<^sub>c, s\<^sub>c), R\<^sub>c, G\<^sub>c) \<preceq>\<^sub>p \<^sub>(\<^sub>\<alpha>\<^sub>;\<^sub>\<sigma>\<^sub>;\<^sub>\<gamma>\<^sub>) (\<Gamma>\<^sub>a, (P\<^sub>a, s\<^sub>a), R\<^sub>a, G\<^sub>a) \<rbrakk> \<Longrightarrow>
+    (\<Gamma>\<^sub>c, (BasicEvent (l\<^sub>c, g\<^sub>c, P\<^sub>c), s\<^sub>c, x\<^sub>c), R\<^sub>c, G\<^sub>c) \<preceq>\<^sub>e\<^sub>@\<^sub>k \<^sub>(\<^sub>\<alpha>\<^sub>;\<^sub>\<eta>\<^sub>;\<^sub>\<zeta>\<^sub>;\<^sub>\<gamma>\<^sub>)
+    (\<Gamma>\<^sub>a, (BasicEvent (l\<^sub>a, g\<^sub>a, P\<^sub>a),s\<^sub>a, x\<^sub>a), R\<^sub>a, G\<^sub>a)"
+  apply (coinduction arbitrary: P\<^sub>c s\<^sub>c x\<^sub>c P\<^sub>a s\<^sub>a x\<^sub>a, simp)
   apply (rule conjI)
    apply blast
   apply (rule conjI, clarsimp)
-   apply (meson BasicEvent_Sound_lemma)
-  apply (rule conjI, clarsimp)
-   apply (meson Event\<^sub>c.noevtent_notran0 act.distinct(1))
-  apply (rule conjI, clarsimp)
+   apply (erule Event\<^sub>c.etran.cases, simp_all, simp add: body_def get_actk_def guard_def)
+   apply auto[1]
+   apply (rule_tac x = "AnonyEvent P\<^sub>a" and y = "x\<^sub>a(k := BasicEvent (l\<^sub>a, g\<^sub>a, P\<^sub>a))" in ex2I)
+   apply (drule_tac a = s\<^sub>c and b = s\<^sub>a in all2_impD, simp add: rel_guard_and_def rel_guard_eq_def)
+    apply blast
+   apply (rule conjI)
+    apply (smt (verit, ccfv_SIG) CollectD Event\<^sub>a.basicevt_tran case_prod_conv get_actk_def 
+          prog_sim_validity rel_guard_eq_def subsetD)
+   apply (rule AnonyEvt_Rule, simp_all)
+  apply (rule conjI)
+   apply (metis Event\<^sub>c.noevtent_notran0 act.simps(4))
+  apply (rule conjI)
    apply (meson Event\<^sub>c.noevtent_notran0 act.distinct(1))
   by (meson Stable_def)
 
 coinductive es_sim :: "['Env\<^sub>c, ('l\<^sub>c,'k,'s\<^sub>c,'prog\<^sub>c) esconf, ('s\<^sub>c \<times> 's\<^sub>c) set, ('s\<^sub>c \<times> 's\<^sub>c) set, 
-                  ('s\<^sub>c \<times> 's\<^sub>a) set, 
+                  'k, ('s\<^sub>c \<times> 's\<^sub>a) set, 
                   ('l\<^sub>c,'k,'s\<^sub>c,'prog\<^sub>c) event \<Rightarrow> ('l\<^sub>a,'k,'s\<^sub>a,'prog\<^sub>a) event, 
                   ('l\<^sub>c,'k,'s\<^sub>c,'prog\<^sub>c) event \<Rightarrow> 'prog\<^sub>c \<Rightarrow> 'prog\<^sub>a option,
                   'Env\<^sub>a, ('l\<^sub>a,'k,'s\<^sub>a,'prog\<^sub>a) esconf, ('s\<^sub>a \<times> 's\<^sub>a) set, ('s\<^sub>a \<times> 's\<^sub>a) set] \<Rightarrow> bool" 
-  ("'(_,_,_,_')/ \<preceq>\<^sub>e\<^sub>s \<^sub>'(\<^sub>_\<^sub>;\<^sub>_\<^sub>;\<^sub>_\<^sub>') /'(_,_,_,_')" [81,81,81,81,81,81,81,81,81,81,81] 100)
-  where rgsim : "\<lbrakk>(s\<^sub>c, s\<^sub>a) \<in> \<alpha>; 
-                  
-                  (\<forall>k. 
+  ("'(_,_,_,_')/ \<preceq>\<^sub>e\<^sub>s\<^sub>@\<^sub>_ \<^sub>'(\<^sub>_\<^sub>;\<^sub>_\<^sub>;\<^sub>_\<^sub>') /'(_,_,_,_')" [81,81,81,81,81,81,81,81,81,81,81,81] 100)
+  where rgsim : "\<lbrakk>(s\<^sub>c, s\<^sub>a) \<in> \<alpha>;
+                       
+                  \<forall>e\<^sub>c es\<^sub>c' x\<^sub>c'. (\<Gamma>\<^sub>c \<turnstile>\<^sub>c (es\<^sub>c, s\<^sub>c, x\<^sub>c) -es-((EvtEnt e\<^sub>c)\<sharp>k)\<rightarrow> (es\<^sub>c', s\<^sub>c, x\<^sub>c')) \<longrightarrow>(\<exists> es\<^sub>a' x\<^sub>a'. 
+                  (\<Gamma>\<^sub>a \<turnstile>\<^sub>a (es\<^sub>a, s\<^sub>a, x\<^sub>a) -es-((EvtEnt (\<eta> e\<^sub>c))\<sharp>k)\<rightarrow> (es\<^sub>a', s\<^sub>a, x\<^sub>a')) \<and> 
+                  (\<Gamma>\<^sub>c, (es\<^sub>c', s\<^sub>c, x\<^sub>c'), R\<^sub>c, G\<^sub>c) \<preceq>\<^sub>e\<^sub>s\<^sub>@\<^sub>k \<^sub>(\<^sub>\<alpha>\<^sub>;\<^sub>\<eta>\<^sub>;\<^sub>\<zeta>\<^sub>) (\<Gamma>\<^sub>a, (es\<^sub>a', s\<^sub>a, x\<^sub>a'), R\<^sub>a, G\<^sub>a));
 
+                  \<forall>Pc es\<^sub>c' s\<^sub>c'. (\<Gamma>\<^sub>c \<turnstile>\<^sub>c (es\<^sub>c, s\<^sub>c, x\<^sub>c) -es-((Cmd Pc)\<sharp>k)\<rightarrow> (es\<^sub>c', s\<^sub>c', x\<^sub>c)) \<and> \<zeta> (x\<^sub>c k) Pc = None \<longrightarrow>
+                  (s\<^sub>c, s\<^sub>c') \<in> G\<^sub>c \<and> (\<Gamma>\<^sub>c, (es\<^sub>c', s\<^sub>c', x\<^sub>c), R\<^sub>c, G\<^sub>c) \<preceq>\<^sub>e\<^sub>s\<^sub>@\<^sub>k \<^sub>(\<^sub>\<alpha>\<^sub>;\<^sub>\<eta>\<^sub>;\<^sub>\<zeta>\<^sub>) (\<Gamma>\<^sub>a, (es\<^sub>a, s\<^sub>a, x\<^sub>a), R\<^sub>a, G\<^sub>a);
 
-                  (\<forall>e\<^sub>c es\<^sub>c' x\<^sub>c'. (\<Gamma>\<^sub>c \<turnstile>\<^sub>c (es\<^sub>c, s\<^sub>c, x\<^sub>c) -es-((EvtEnt e\<^sub>c)\<sharp>k)\<rightarrow> (es\<^sub>c', s\<^sub>c, x\<^sub>c')) \<longrightarrow>(\<exists> es\<^sub>a' x\<^sub>a'. 
-                   (\<Gamma>\<^sub>a \<turnstile>\<^sub>a (es\<^sub>a, s\<^sub>a, x\<^sub>a) -es-((EvtEnt (\<eta> e\<^sub>c))\<sharp>k)\<rightarrow> (es\<^sub>a', s\<^sub>a, x\<^sub>a')) \<and> 
-                    (\<Gamma>\<^sub>c, (es\<^sub>c', s\<^sub>c, x\<^sub>c'), R\<^sub>c, G\<^sub>c) \<preceq>\<^sub>e\<^sub>s \<^sub>(\<^sub>\<alpha>\<^sub>;\<^sub>\<eta>\<^sub>;\<^sub>\<kappa>\<^sub>) (\<Gamma>\<^sub>a, (es\<^sub>a', s\<^sub>a, x\<^sub>a'), R\<^sub>a, G\<^sub>a))) \<and>
-
-                  (\<forall>Pc es\<^sub>c' s\<^sub>c'. (\<Gamma>\<^sub>c \<turnstile>\<^sub>c (es\<^sub>c, s\<^sub>c, x\<^sub>c) -es-((Cmd Pc)\<sharp>k)\<rightarrow> (es\<^sub>c', s\<^sub>c', x\<^sub>c)) \<and> \<kappa> (x\<^sub>c k) Pc = None \<longrightarrow>
-                  (s\<^sub>c, s\<^sub>c') \<in> G\<^sub>c \<and> (\<Gamma>\<^sub>c, (es\<^sub>c', s\<^sub>c', x\<^sub>c), R\<^sub>c, G\<^sub>c) \<preceq>\<^sub>e\<^sub>s \<^sub>(\<^sub>\<alpha>\<^sub>;\<^sub>\<eta>\<^sub>;\<^sub>\<kappa>\<^sub>) (\<Gamma>\<^sub>a, (es\<^sub>a, s\<^sub>a, x\<^sub>a), R\<^sub>a, G\<^sub>a)) \<and>
-                  
-                  (\<forall>Pc es\<^sub>c' s\<^sub>c' Pa. (\<Gamma>\<^sub>c \<turnstile>\<^sub>c (es\<^sub>c, s\<^sub>c, x\<^sub>c) -es-((Cmd Pc)\<sharp>k)\<rightarrow> (es\<^sub>c', s\<^sub>c', x\<^sub>c)) \<and> \<kappa> (x\<^sub>c k) Pc = Some Pa \<longrightarrow>
+                  \<forall>Pc es\<^sub>c' s\<^sub>c' Pa. (\<Gamma>\<^sub>c \<turnstile>\<^sub>c (es\<^sub>c, s\<^sub>c, x\<^sub>c) -es-((Cmd Pc)\<sharp>k)\<rightarrow> (es\<^sub>c', s\<^sub>c', x\<^sub>c)) \<and> \<zeta> (x\<^sub>c k) Pc = Some Pa \<longrightarrow>
                   \<eta> (x\<^sub>c k) = x\<^sub>a k \<and>
                   (\<exists>es\<^sub>a' s\<^sub>a'. (\<Gamma>\<^sub>a \<turnstile>\<^sub>a (es\<^sub>a, s\<^sub>a, x\<^sub>a) -es-((Cmd Pa)\<sharp>k)\<rightarrow> (es\<^sub>a', s\<^sub>a', x\<^sub>a)) \<and> (s\<^sub>c, s\<^sub>c') \<in> G\<^sub>c \<and> (s\<^sub>a, s\<^sub>a') \<in> G\<^sub>a
-                  \<and> (\<Gamma>\<^sub>c, (es\<^sub>c', s\<^sub>c', x\<^sub>c), R\<^sub>c, G\<^sub>c) \<preceq>\<^sub>e\<^sub>s \<^sub>(\<^sub>\<alpha>\<^sub>;\<^sub>\<eta>\<^sub>;\<^sub>\<kappa>\<^sub>) (\<Gamma>\<^sub>a, (es\<^sub>a', s\<^sub>a', x\<^sub>a), R\<^sub>a, G\<^sub>a))) \<and>
-      
-                  (\<forall>s\<^sub>c' s\<^sub>a' x\<^sub>c' x\<^sub>a'. ((s\<^sub>c, s\<^sub>c') \<in> R\<^sub>c \<union> Id \<and> (s\<^sub>a, s\<^sub>a') \<in>  R\<^sub>a \<union> Id) \<longrightarrow>( x\<^sub>c' k = x\<^sub>c k \<and> x\<^sub>a' k = x\<^sub>a k)
-                   \<longrightarrow>  (\<Gamma>\<^sub>c, (es\<^sub>c, s\<^sub>c', x\<^sub>c'), R\<^sub>c, G\<^sub>c) \<preceq>\<^sub>e\<^sub>s \<^sub>(\<^sub>\<alpha>\<^sub>;\<^sub>\<eta>\<^sub>;\<^sub>\<kappa>\<^sub>) (\<Gamma>\<^sub>a, (es\<^sub>a, s\<^sub>a', x\<^sub>a'), R\<^sub>a, G\<^sub>a))
+                  \<and> (\<Gamma>\<^sub>c, (es\<^sub>c', s\<^sub>c', x\<^sub>c), R\<^sub>c, G\<^sub>c) \<preceq>\<^sub>e\<^sub>s\<^sub>@\<^sub>k \<^sub>(\<^sub>\<alpha>\<^sub>;\<^sub>\<eta>\<^sub>;\<^sub>\<zeta>\<^sub>) (\<Gamma>\<^sub>a, (es\<^sub>a', s\<^sub>a', x\<^sub>a), R\<^sub>a, G\<^sub>a));
 
-                  )       
-                  \<rbrakk> \<Longrightarrow> (\<Gamma>\<^sub>c, (es\<^sub>c, s\<^sub>c, x\<^sub>c), R\<^sub>c, G\<^sub>c) \<preceq>\<^sub>e\<^sub>s \<^sub>(\<^sub>\<alpha>\<^sub>;\<^sub>\<eta>\<^sub>;\<^sub>\<kappa>\<^sub>) (\<Gamma>\<^sub>a, (es\<^sub>a, s\<^sub>a, x\<^sub>a), R\<^sub>a, G\<^sub>a)"
+                 \<forall>s\<^sub>c' s\<^sub>a' x\<^sub>c' x\<^sub>a'. ((s\<^sub>c, s\<^sub>c'),(s\<^sub>a, s\<^sub>a')) \<in> ((R\<^sub>c \<union> Id, R\<^sub>a \<union> Id)\<^sub>\<alpha>) \<longrightarrow>(x\<^sub>c' k = x\<^sub>c k \<and> x\<^sub>a' k = x\<^sub>a k)
+                   \<longrightarrow> (\<Gamma>\<^sub>c, (es\<^sub>c, s\<^sub>c', x\<^sub>c'), R\<^sub>c, G\<^sub>c) \<preceq>\<^sub>e\<^sub>s\<^sub>@\<^sub>k \<^sub>(\<^sub>\<alpha>\<^sub>;\<^sub>\<eta>\<^sub>;\<^sub>\<zeta>\<^sub>) (\<Gamma>\<^sub>a, (es\<^sub>a, s\<^sub>a', x\<^sub>a'), R\<^sub>a, G\<^sub>a)\<rbrakk> 
+        \<Longrightarrow> (\<Gamma>\<^sub>c, (es\<^sub>c, s\<^sub>c, x\<^sub>c), R\<^sub>c, G\<^sub>c) \<preceq>\<^sub>e\<^sub>s\<^sub>@\<^sub>k \<^sub>(\<^sub>\<alpha>\<^sub>;\<^sub>\<eta>\<^sub>;\<^sub>\<zeta>\<^sub>) (\<Gamma>\<^sub>a, (es\<^sub>a, s\<^sub>a, x\<^sub>a), R\<^sub>a, G\<^sub>a)"
 
-definition es_sim_pre :: "['Env\<^sub>c, ('l\<^sub>c,'k,'s\<^sub>c,'prog\<^sub>c) esys, ('s\<^sub>c \<times> 's\<^sub>c) set, ('s\<^sub>c \<times> 's\<^sub>c) set, 
-                  ('s\<^sub>c \<times> 's\<^sub>a) set, ('s\<^sub>c \<times> 's\<^sub>a) set, 
+lemma es_sim_init :"(\<Gamma>\<^sub>c, (es\<^sub>c, s\<^sub>c, x\<^sub>c), R\<^sub>c, G\<^sub>c) \<preceq>\<^sub>e\<^sub>s\<^sub>@\<^sub>k \<^sub>(\<^sub>\<alpha>\<^sub>;\<^sub>\<eta>\<^sub>;\<^sub>\<zeta>\<^sub>) (\<Gamma>\<^sub>a, (es\<^sub>a, s\<^sub>a, x\<^sub>a), R\<^sub>a, G\<^sub>a) \<Longrightarrow> (s\<^sub>c, s\<^sub>a) \<in> \<alpha>"
+  by (erule es_sim.cases, simp_all)
+
+lemma EvtSys_Sound_help1: "\<lbrakk>\<Gamma>\<^sub>c \<turnstile>\<^sub>c (e\<^sub>c, s\<^sub>c, x\<^sub>c) -et-EvtEnt ec\<sharp>k\<rightarrow> (e\<^sub>c', s\<^sub>c, x\<^sub>c'); 
+       (\<Gamma>\<^sub>c,(e\<^sub>c, s\<^sub>c, x\<^sub>c),R\<^sub>c,G\<^sub>c) \<preceq>\<^sub>e\<^sub>@\<^sub>k \<^sub>(\<^sub>\<alpha>\<^sub>;\<^sub>\<eta>\<^sub>;\<^sub>\<zeta>\<^sub>;\<^sub>\<gamma>\<^sub>) (\<Gamma>\<^sub>a,(e\<^sub>a, s\<^sub>a, x\<^sub>a),R\<^sub>a,G\<^sub>a)\<rbrakk> \<Longrightarrow> 
+       \<exists>e\<^sub>a' x\<^sub>a'. (\<Gamma>\<^sub>a \<turnstile>\<^sub>a (e\<^sub>a, s\<^sub>a, x\<^sub>a) -et-EvtEnt (\<eta> ec)\<sharp>k\<rightarrow> (e\<^sub>a', s\<^sub>a, x\<^sub>a')) 
+       \<and> (\<Gamma>\<^sub>c,(e\<^sub>c', s\<^sub>c, x\<^sub>c'),R\<^sub>c,G\<^sub>c) \<preceq>\<^sub>e\<^sub>@\<^sub>k \<^sub>(\<^sub>\<alpha>\<^sub>;\<^sub>\<eta>\<^sub>;\<^sub>\<zeta>\<^sub>;\<^sub>\<gamma>\<^sub>) (\<Gamma>\<^sub>a,(e\<^sub>a', s\<^sub>a, x\<^sub>a'),R\<^sub>a,G\<^sub>a)"
+  by (erule e_sim.cases, simp)
+
+lemma EvtSys_Sound_help2: "\<lbrakk>(\<Gamma>\<^sub>c,(e\<^sub>c, s\<^sub>c, x\<^sub>c),R\<^sub>c,G\<^sub>c) \<preceq>\<^sub>e\<^sub>@\<^sub>k \<^sub>(\<^sub>\<alpha>\<^sub>;\<^sub>\<eta>\<^sub>;\<^sub>\<zeta>\<^sub>;\<^sub>\<gamma>\<^sub>) (\<Gamma>\<^sub>a,(e\<^sub>a, s\<^sub>a, x\<^sub>a),R\<^sub>a,G\<^sub>a);
+       e\<^sub>c \<noteq> AnonyEvent fin_com\<^sub>c\<rbrakk> \<Longrightarrow> e\<^sub>a \<noteq> AnonyEvent fin_com\<^sub>a"
+  by (erule e_sim.cases, simp)
+
+lemma EvtSys_Sound_help3: "\<lbrakk>(\<Gamma>\<^sub>c,(e\<^sub>c, s\<^sub>c, x\<^sub>c),R\<^sub>c,G\<^sub>c) \<preceq>\<^sub>e\<^sub>@\<^sub>k \<^sub>(\<^sub>\<alpha>\<^sub>;\<^sub>\<eta>\<^sub>;\<^sub>\<zeta>\<^sub>;\<^sub>\<gamma>\<^sub>) (\<Gamma>\<^sub>a,(e\<^sub>a, s\<^sub>a, x\<^sub>a),R\<^sub>a,G\<^sub>a);
+       e\<^sub>c = AnonyEvent fin_com\<^sub>c\<rbrakk> \<Longrightarrow> e\<^sub>a = AnonyEvent fin_com\<^sub>a  \<and> (s\<^sub>c, s\<^sub>a) \<in> \<gamma>"
+  by (erule e_sim.cases, simp)
+
+lemma EvtSys_Sound_help4: "\<lbrakk>\<Gamma>\<^sub>c \<turnstile>\<^sub>c (e\<^sub>c, s\<^sub>c, x\<^sub>c) -et-((Cmd Pc)\<sharp>k)\<rightarrow> (e\<^sub>c', s\<^sub>c', x\<^sub>c); \<zeta> (x\<^sub>c k) Pc = None; 
+       (\<Gamma>\<^sub>c,(e\<^sub>c, s\<^sub>c, x\<^sub>c),R\<^sub>c,G\<^sub>c) \<preceq>\<^sub>e\<^sub>@\<^sub>k \<^sub>(\<^sub>\<alpha>\<^sub>;\<^sub>\<eta>\<^sub>;\<^sub>\<zeta>\<^sub>;\<^sub>\<gamma>\<^sub>) (\<Gamma>\<^sub>a,(e\<^sub>a, s\<^sub>a, x\<^sub>a),R\<^sub>a,G\<^sub>a)\<rbrakk> \<Longrightarrow> 
+       (s\<^sub>c, s\<^sub>c') \<in> G\<^sub>c \<and> (\<Gamma>\<^sub>c, (e\<^sub>c', s\<^sub>c', x\<^sub>c), R\<^sub>c, G\<^sub>c) \<preceq>\<^sub>e\<^sub>@\<^sub>k \<^sub>(\<^sub>\<alpha>\<^sub>;\<^sub>\<eta>\<^sub>;\<^sub>\<zeta>\<^sub>;\<^sub>\<gamma>\<^sub>) (\<Gamma>\<^sub>a, (e\<^sub>a, s\<^sub>a, x\<^sub>a), R\<^sub>a, G\<^sub>a)"
+  by (erule e_sim.cases, simp)
+
+lemma EvtSys_Sound_help5: "\<lbrakk>\<Gamma>\<^sub>c \<turnstile>\<^sub>c (e\<^sub>c, s\<^sub>c, x\<^sub>c) -et-((Cmd Pc)\<sharp>k)\<rightarrow> (e\<^sub>c', s\<^sub>c', x\<^sub>c); \<zeta> (x\<^sub>c k) Pc =  Some Pa; 
+       (\<Gamma>\<^sub>c,(e\<^sub>c, s\<^sub>c, x\<^sub>c),R\<^sub>c,G\<^sub>c) \<preceq>\<^sub>e\<^sub>@\<^sub>k \<^sub>(\<^sub>\<alpha>\<^sub>;\<^sub>\<eta>\<^sub>;\<^sub>\<zeta>\<^sub>;\<^sub>\<gamma>\<^sub>) (\<Gamma>\<^sub>a,(e\<^sub>a, s\<^sub>a, x\<^sub>a),R\<^sub>a,G\<^sub>a)\<rbrakk> \<Longrightarrow> \<eta> (x\<^sub>c k) = x\<^sub>a k \<and>
+       (\<exists>e\<^sub>a' s\<^sub>a'. (\<Gamma>\<^sub>a \<turnstile>\<^sub>a (e\<^sub>a, s\<^sub>a, x\<^sub>a) -et-((Cmd Pa)\<sharp>k)\<rightarrow> (e\<^sub>a', s\<^sub>a', x\<^sub>a)) \<and> (s\<^sub>c, s\<^sub>c') \<in> G\<^sub>c \<and> (s\<^sub>a, s\<^sub>a') \<in> G\<^sub>a \<and> 
+       (\<Gamma>\<^sub>c, (e\<^sub>c', s\<^sub>c', x\<^sub>c), R\<^sub>c, G\<^sub>c) \<preceq>\<^sub>e\<^sub>@\<^sub>k \<^sub>(\<^sub>\<alpha>\<^sub>;\<^sub>\<eta>\<^sub>;\<^sub>\<zeta>\<^sub>;\<^sub>\<gamma>\<^sub>) (\<Gamma>\<^sub>a, (e\<^sub>a', s\<^sub>a', x\<^sub>a), R\<^sub>a, G\<^sub>a))"
+  by (erule e_sim.cases, simp)
+
+lemma EvtSys_Sound_help6: "\<lbrakk>(\<Gamma>\<^sub>c,(e\<^sub>c, s\<^sub>c, x\<^sub>c),R\<^sub>c,G\<^sub>c) \<preceq>\<^sub>e\<^sub>@\<^sub>k \<^sub>(\<^sub>\<alpha>\<^sub>;\<^sub>\<eta>\<^sub>;\<^sub>\<zeta>\<^sub>;\<^sub>\<gamma>\<^sub>) (\<Gamma>\<^sub>a,(e\<^sub>a, s\<^sub>a, x\<^sub>a),R\<^sub>a,G\<^sub>a); 
+      ((s\<^sub>c, s\<^sub>c'),(s\<^sub>a, s\<^sub>a')) \<in> (R\<^sub>c \<union> Id, R\<^sub>a \<union> Id)\<^sub>\<alpha>; x\<^sub>c' k = x\<^sub>c k \<and> x\<^sub>a' k = x\<^sub>a k\<rbrakk> \<Longrightarrow> 
+      (\<Gamma>\<^sub>c, (e\<^sub>c, s\<^sub>c', x\<^sub>c'), R\<^sub>c, G\<^sub>c) \<preceq>\<^sub>e\<^sub>@\<^sub>k \<^sub>(\<^sub>\<alpha>\<^sub>;\<^sub>\<eta>\<^sub>;\<^sub>\<zeta>\<^sub>;\<^sub>\<gamma>\<^sub>) (\<Gamma>\<^sub>a, (e\<^sub>a, s\<^sub>a', x\<^sub>a'), R\<^sub>a, G\<^sub>a)"
+  by (erule e_sim.cases, simp)
+
+lemma EvtSeq_Sound_lemma1: "\<lbrakk>(\<Gamma>\<^sub>c,(e\<^sub>c, s\<^sub>c, x\<^sub>c),R\<^sub>c,G\<^sub>c) \<preceq>\<^sub>e\<^sub>@\<^sub>k \<^sub>(\<^sub>\<alpha>\<^sub>;\<^sub>\<eta>\<^sub>;\<^sub>\<zeta>\<^sub>;\<^sub>\<gamma>\<^sub>) (\<Gamma>\<^sub>a,(e\<^sub>a, s\<^sub>a, x\<^sub>a),R\<^sub>a,G\<^sub>a);
+      \<forall>s\<^sub>c s\<^sub>a x\<^sub>c x\<^sub>a. (s\<^sub>c, s\<^sub>a) \<in> \<gamma> \<longrightarrow> (\<Gamma>\<^sub>c,(es\<^sub>c, s\<^sub>c, x\<^sub>c),R\<^sub>c,G\<^sub>c) \<preceq>\<^sub>e\<^sub>s\<^sub>@\<^sub>k \<^sub>(\<^sub>\<alpha>\<^sub>;\<^sub>\<eta>\<^sub>;\<^sub>\<zeta>\<^sub>) (\<Gamma>\<^sub>a,(es\<^sub>a, s\<^sub>a, x\<^sub>a),R\<^sub>a,G\<^sub>a); 
+      \<Gamma>\<^sub>c \<turnstile>\<^sub>c (e\<^sub>c, s\<^sub>c, x\<^sub>c) -et-EvtEnt ec\<sharp>k\<rightarrow> (e\<^sub>c', s\<^sub>c, x\<^sub>c'); e\<^sub>c' \<noteq> AnonyEvent fin_com\<^sub>c \<rbrakk> \<Longrightarrow>  
+      \<exists>e\<^sub>a' x\<^sub>a'.
+          (\<Gamma>\<^sub>a \<turnstile>\<^sub>a (EvtSeq e\<^sub>a es\<^sub>a, s\<^sub>a, x\<^sub>a) -es-EvtEnt (\<eta> ec)\<sharp>k\<rightarrow> (EvtSeq e\<^sub>a' es\<^sub>a, s\<^sub>a, x\<^sub>a')) \<and>
+          (\<Gamma>\<^sub>c,(e\<^sub>c', s\<^sub>c, x\<^sub>c'),R\<^sub>c,G\<^sub>c) \<preceq>\<^sub>e\<^sub>@\<^sub>k \<^sub>(\<^sub>\<alpha>\<^sub>;\<^sub>\<eta>\<^sub>;\<^sub>\<zeta>\<^sub>;\<^sub>\<gamma>\<^sub>) (\<Gamma>\<^sub>a,(e\<^sub>a', s\<^sub>a, x\<^sub>a'),R\<^sub>a,G\<^sub>a)"
+proof-
+  assume a0: "(\<Gamma>\<^sub>c,(e\<^sub>c, s\<^sub>c, x\<^sub>c),R\<^sub>c,G\<^sub>c) \<preceq>\<^sub>e\<^sub>@\<^sub>k \<^sub>(\<^sub>\<alpha>\<^sub>;\<^sub>\<eta>\<^sub>;\<^sub>\<zeta>\<^sub>;\<^sub>\<gamma>\<^sub>) (\<Gamma>\<^sub>a,(e\<^sub>a, s\<^sub>a, x\<^sub>a),R\<^sub>a,G\<^sub>a)"
+     and a1: "\<forall>s\<^sub>c s\<^sub>a x\<^sub>c x\<^sub>a. (s\<^sub>c, s\<^sub>a) \<in> \<gamma> \<longrightarrow> (\<Gamma>\<^sub>c,(es\<^sub>c, s\<^sub>c, x\<^sub>c),R\<^sub>c,G\<^sub>c) \<preceq>\<^sub>e\<^sub>s\<^sub>@\<^sub>k \<^sub>(\<^sub>\<alpha>\<^sub>;\<^sub>\<eta>\<^sub>;\<^sub>\<zeta>\<^sub>) (\<Gamma>\<^sub>a,(es\<^sub>a, s\<^sub>a, x\<^sub>a),R\<^sub>a,G\<^sub>a)"
+     and a2: "\<Gamma>\<^sub>c \<turnstile>\<^sub>c (e\<^sub>c, s\<^sub>c, x\<^sub>c) -et-EvtEnt ec\<sharp>k\<rightarrow> (e\<^sub>c', s\<^sub>c, x\<^sub>c')"
+     and a3: "e\<^sub>c' \<noteq> AnonyEvent fin_com\<^sub>c"
+  from a0 a2 have "\<exists>e\<^sub>a' x\<^sub>a'. (\<Gamma>\<^sub>a \<turnstile>\<^sub>a (e\<^sub>a, s\<^sub>a, x\<^sub>a) -et-((EvtEnt (\<eta> ec))\<sharp>k)\<rightarrow> (e\<^sub>a', s\<^sub>a, x\<^sub>a')) \<and>
+                (\<Gamma>\<^sub>c, (e\<^sub>c', s\<^sub>c, x\<^sub>c'), R\<^sub>c, G\<^sub>c) \<preceq>\<^sub>e\<^sub>@\<^sub>k \<^sub>(\<^sub>\<alpha>\<^sub>;\<^sub>\<eta>\<^sub>;\<^sub>\<zeta>\<^sub>;\<^sub>\<gamma>\<^sub>) (\<Gamma>\<^sub>a, (e\<^sub>a', s\<^sub>a, x\<^sub>a'), R\<^sub>a, G\<^sub>a)"
+    by (simp add: EvtSys_Sound_help1)
+  then obtain e\<^sub>a' x\<^sub>a' where a4: "(\<Gamma>\<^sub>a \<turnstile>\<^sub>a (e\<^sub>a, s\<^sub>a, x\<^sub>a) -et-((EvtEnt (\<eta> ec))\<sharp>k)\<rightarrow> (e\<^sub>a', s\<^sub>a, x\<^sub>a')) \<and>
+                (\<Gamma>\<^sub>c, (e\<^sub>c', s\<^sub>c, x\<^sub>c'), R\<^sub>c, G\<^sub>c) \<preceq>\<^sub>e\<^sub>@\<^sub>k \<^sub>(\<^sub>\<alpha>\<^sub>;\<^sub>\<eta>\<^sub>;\<^sub>\<zeta>\<^sub>;\<^sub>\<gamma>\<^sub>) (\<Gamma>\<^sub>a, (e\<^sub>a', s\<^sub>a, x\<^sub>a'), R\<^sub>a, G\<^sub>a)"
+    by auto
+  with a3 have a5: "e\<^sub>a' \<noteq> AnonyEvent fin_com\<^sub>a"
+    by (meson EvtSys_Sound_help2)
+  with a4 have a6: "\<Gamma>\<^sub>a \<turnstile>\<^sub>a (EvtSeq e\<^sub>a es\<^sub>a, s\<^sub>a, x\<^sub>a) -es-EvtEnt (\<eta> ec)\<sharp>k\<rightarrow> (EvtSeq e\<^sub>a' es\<^sub>a, s\<^sub>a, x\<^sub>a')"
+    by (simp add: Event\<^sub>a.EvtSeq1)
+  with a4 show ?thesis by blast
+qed
+
+lemma EvtSeq_Sound_lemma2: "\<lbrakk>(\<Gamma>\<^sub>c,(e\<^sub>c, s\<^sub>c, x\<^sub>c),R\<^sub>c,G\<^sub>c) \<preceq>\<^sub>e\<^sub>@\<^sub>k \<^sub>(\<^sub>\<alpha>\<^sub>;\<^sub>\<eta>\<^sub>;\<^sub>\<zeta>\<^sub>;\<^sub>\<gamma>\<^sub>) (\<Gamma>\<^sub>a,(e\<^sub>a, s\<^sub>a, x\<^sub>a),R\<^sub>a,G\<^sub>a);
+      \<forall>s\<^sub>c s\<^sub>a x\<^sub>c x\<^sub>a. (s\<^sub>c, s\<^sub>a) \<in> \<gamma> \<longrightarrow> (\<Gamma>\<^sub>c,(es\<^sub>c, s\<^sub>c, x\<^sub>c),R\<^sub>c,G\<^sub>c) \<preceq>\<^sub>e\<^sub>s\<^sub>@\<^sub>k \<^sub>(\<^sub>\<alpha>\<^sub>;\<^sub>\<eta>\<^sub>;\<^sub>\<zeta>\<^sub>) (\<Gamma>\<^sub>a,(es\<^sub>a, s\<^sub>a, x\<^sub>a),R\<^sub>a,G\<^sub>a); 
+      \<Gamma>\<^sub>c \<turnstile>\<^sub>c (e\<^sub>c, s\<^sub>c, x\<^sub>c) -et-EvtEnt ec\<sharp>k\<rightarrow> (AnonyEvent fin_com\<^sub>c, s\<^sub>c, x\<^sub>c') \<rbrakk> \<Longrightarrow>  
+      \<exists>e\<^sub>a' x\<^sub>a'.
+          (\<Gamma>\<^sub>a \<turnstile>\<^sub>a (EvtSeq e\<^sub>a es\<^sub>a, s\<^sub>a, x\<^sub>a) -es-EvtEnt (\<eta> ec)\<sharp>k\<rightarrow> (es\<^sub>a, s\<^sub>a, x\<^sub>a')) \<and>
+          (\<Gamma>\<^sub>c,(es\<^sub>c, s\<^sub>c, x\<^sub>c'),R\<^sub>c,G\<^sub>c) \<preceq>\<^sub>e\<^sub>s\<^sub>@\<^sub>k \<^sub>(\<^sub>\<alpha>\<^sub>;\<^sub>\<eta>\<^sub>;\<^sub>\<zeta>\<^sub>) (\<Gamma>\<^sub>a,(es\<^sub>a, s\<^sub>a, x\<^sub>a'),R\<^sub>a,G\<^sub>a)"
+proof-
+  assume a0: "(\<Gamma>\<^sub>c,(e\<^sub>c, s\<^sub>c, x\<^sub>c),R\<^sub>c,G\<^sub>c) \<preceq>\<^sub>e\<^sub>@\<^sub>k \<^sub>(\<^sub>\<alpha>\<^sub>;\<^sub>\<eta>\<^sub>;\<^sub>\<zeta>\<^sub>;\<^sub>\<gamma>\<^sub>) (\<Gamma>\<^sub>a,(e\<^sub>a, s\<^sub>a, x\<^sub>a),R\<^sub>a,G\<^sub>a)"
+     and a1: "\<forall>s\<^sub>c s\<^sub>a x\<^sub>c x\<^sub>a. (s\<^sub>c, s\<^sub>a) \<in> \<gamma> \<longrightarrow> (\<Gamma>\<^sub>c,(es\<^sub>c, s\<^sub>c, x\<^sub>c),R\<^sub>c,G\<^sub>c) \<preceq>\<^sub>e\<^sub>s\<^sub>@\<^sub>k \<^sub>(\<^sub>\<alpha>\<^sub>;\<^sub>\<eta>\<^sub>;\<^sub>\<zeta>\<^sub>) (\<Gamma>\<^sub>a,(es\<^sub>a, s\<^sub>a, x\<^sub>a),R\<^sub>a,G\<^sub>a)"
+     and a2: "\<Gamma>\<^sub>c \<turnstile>\<^sub>c (e\<^sub>c, s\<^sub>c, x\<^sub>c) -et-EvtEnt ec\<sharp>k\<rightarrow> (AnonyEvent fin_com\<^sub>c, s\<^sub>c, x\<^sub>c')"
+
+  from a0 a2 have "\<exists>e\<^sub>a' x\<^sub>a'. (\<Gamma>\<^sub>a \<turnstile>\<^sub>a (e\<^sub>a, s\<^sub>a, x\<^sub>a) -et-((EvtEnt (\<eta> ec))\<sharp>k)\<rightarrow> (e\<^sub>a', s\<^sub>a, x\<^sub>a')) \<and>
+                (\<Gamma>\<^sub>c, (AnonyEvent fin_com\<^sub>c, s\<^sub>c, x\<^sub>c'), R\<^sub>c, G\<^sub>c) \<preceq>\<^sub>e\<^sub>@\<^sub>k \<^sub>(\<^sub>\<alpha>\<^sub>;\<^sub>\<eta>\<^sub>;\<^sub>\<zeta>\<^sub>;\<^sub>\<gamma>\<^sub>) (\<Gamma>\<^sub>a, (e\<^sub>a', s\<^sub>a, x\<^sub>a'), R\<^sub>a, G\<^sub>a)"
+    by (simp add: EvtSys_Sound_help1)
+  then obtain e\<^sub>a' x\<^sub>a' where a3: "(\<Gamma>\<^sub>a \<turnstile>\<^sub>a (e\<^sub>a, s\<^sub>a, x\<^sub>a) -et-((EvtEnt (\<eta> ec))\<sharp>k)\<rightarrow> (e\<^sub>a', s\<^sub>a, x\<^sub>a')) \<and>
+  (\<Gamma>\<^sub>c, (AnonyEvent fin_com\<^sub>c, s\<^sub>c, x\<^sub>c'), R\<^sub>c, G\<^sub>c) \<preceq>\<^sub>e\<^sub>@\<^sub>k \<^sub>(\<^sub>\<alpha>\<^sub>;\<^sub>\<eta>\<^sub>;\<^sub>\<zeta>\<^sub>;\<^sub>\<gamma>\<^sub>) (\<Gamma>\<^sub>a, (e\<^sub>a', s\<^sub>a, x\<^sub>a'), R\<^sub>a, G\<^sub>a)" by auto
+  then have a4: "e\<^sub>a' = AnonyEvent fin_com\<^sub>a \<and> (s\<^sub>c, s\<^sub>a) \<in> \<gamma>"
+    by (meson EvtSys_Sound_help3)
+  with a3 a4 have a5: "\<Gamma>\<^sub>a \<turnstile>\<^sub>a (EvtSeq e\<^sub>a es\<^sub>a, s\<^sub>a, x\<^sub>a) -es-EvtEnt (\<eta> ec)\<sharp>k\<rightarrow> (es\<^sub>a, s\<^sub>a, x\<^sub>a')"   
+    by (metis Event\<^sub>a.EvtSeq2)
+  from a1 a4 have a6: "(\<Gamma>\<^sub>c,(es\<^sub>c, s\<^sub>c, x\<^sub>c'),R\<^sub>c,G\<^sub>c) \<preceq>\<^sub>e\<^sub>s\<^sub>@\<^sub>k \<^sub>(\<^sub>\<alpha>\<^sub>;\<^sub>\<eta>\<^sub>;\<^sub>\<zeta>\<^sub>) (\<Gamma>\<^sub>a,(es\<^sub>a, s\<^sub>a, x\<^sub>a'),R\<^sub>a,G\<^sub>a)"
+    by blast
+  with a5 show ?thesis by auto
+qed
+
+lemma EvtSeq_Sound_lemma3: "\<lbrakk> \<zeta> (x\<^sub>c k) Pc = Some Pa;
+      (\<Gamma>\<^sub>c,(e\<^sub>c, s\<^sub>c, x\<^sub>c),R\<^sub>c,G\<^sub>c) \<preceq>\<^sub>e\<^sub>@\<^sub>k \<^sub>(\<^sub>\<alpha>\<^sub>;\<^sub>\<eta>\<^sub>;\<^sub>\<zeta>\<^sub>;\<^sub>\<gamma>\<^sub>) (\<Gamma>\<^sub>a,(e\<^sub>a, s\<^sub>a, x\<^sub>a),R\<^sub>a,G\<^sub>a);
+      \<forall>s\<^sub>c s\<^sub>a x\<^sub>c x\<^sub>a. (s\<^sub>c, s\<^sub>a) \<in> \<gamma> \<longrightarrow> (\<Gamma>\<^sub>c,(es\<^sub>c, s\<^sub>c, x\<^sub>c),R\<^sub>c,G\<^sub>c) \<preceq>\<^sub>e\<^sub>s\<^sub>@\<^sub>k \<^sub>(\<^sub>\<alpha>\<^sub>;\<^sub>\<eta>\<^sub>;\<^sub>\<zeta>\<^sub>) (\<Gamma>\<^sub>a,(es\<^sub>a, s\<^sub>a, x\<^sub>a),R\<^sub>a,G\<^sub>a); 
+      \<Gamma>\<^sub>c \<turnstile>\<^sub>c (e\<^sub>c, s\<^sub>c, x\<^sub>c) -et- Cmd Pc\<sharp>k\<rightarrow> (e\<^sub>c', s\<^sub>c', x\<^sub>c); e\<^sub>c' \<noteq> AnonyEvent fin_com\<^sub>c \<rbrakk> \<Longrightarrow>  
+      \<exists>e\<^sub>a' s\<^sub>a'.
+          (\<Gamma>\<^sub>a \<turnstile>\<^sub>a (EvtSeq e\<^sub>a es\<^sub>a, s\<^sub>a, x\<^sub>a) -es-Cmd Pa\<sharp>k\<rightarrow> (EvtSeq e\<^sub>a' es\<^sub>a, s\<^sub>a', x\<^sub>a)) \<and>
+          (s\<^sub>c, s\<^sub>c') \<in> G\<^sub>c \<and> (s\<^sub>a, s\<^sub>a') \<in> G\<^sub>a \<and> 
+          (\<Gamma>\<^sub>c,(e\<^sub>c', s\<^sub>c', x\<^sub>c),R\<^sub>c,G\<^sub>c) \<preceq>\<^sub>e\<^sub>@\<^sub>k \<^sub>(\<^sub>\<alpha>\<^sub>;\<^sub>\<eta>\<^sub>;\<^sub>\<zeta>\<^sub>;\<^sub>\<gamma>\<^sub>) (\<Gamma>\<^sub>a,(e\<^sub>a', s\<^sub>a', x\<^sub>a),R\<^sub>a,G\<^sub>a)"
+proof-
+  assume a0: "(\<Gamma>\<^sub>c,(e\<^sub>c, s\<^sub>c, x\<^sub>c),R\<^sub>c,G\<^sub>c) \<preceq>\<^sub>e\<^sub>@\<^sub>k \<^sub>(\<^sub>\<alpha>\<^sub>;\<^sub>\<eta>\<^sub>;\<^sub>\<zeta>\<^sub>;\<^sub>\<gamma>\<^sub>) (\<Gamma>\<^sub>a,(e\<^sub>a, s\<^sub>a, x\<^sub>a),R\<^sub>a,G\<^sub>a)"
+     and a1: "\<forall>s\<^sub>c s\<^sub>a x\<^sub>c x\<^sub>a. (s\<^sub>c, s\<^sub>a) \<in> \<gamma> \<longrightarrow> (\<Gamma>\<^sub>c,(es\<^sub>c, s\<^sub>c, x\<^sub>c),R\<^sub>c,G\<^sub>c) \<preceq>\<^sub>e\<^sub>s\<^sub>@\<^sub>k \<^sub>(\<^sub>\<alpha>\<^sub>;\<^sub>\<eta>\<^sub>;\<^sub>\<zeta>\<^sub>) (\<Gamma>\<^sub>a,(es\<^sub>a, s\<^sub>a, x\<^sub>a),R\<^sub>a,G\<^sub>a)"
+     and a2: "\<Gamma>\<^sub>c \<turnstile>\<^sub>c (e\<^sub>c, s\<^sub>c, x\<^sub>c) -et- Cmd Pc\<sharp>k\<rightarrow> (e\<^sub>c', s\<^sub>c', x\<^sub>c)"
+     and a3: "e\<^sub>c' \<noteq> AnonyEvent fin_com\<^sub>c"
+     and a4: "\<zeta> (x\<^sub>c k) Pc = Some Pa"
+  from a0 a2 a4 have "(\<exists>e\<^sub>a' s\<^sub>a'. (\<Gamma>\<^sub>a \<turnstile>\<^sub>a (e\<^sub>a, s\<^sub>a, x\<^sub>a) -et-((Cmd Pa)\<sharp>k)\<rightarrow> (e\<^sub>a', s\<^sub>a', x\<^sub>a)) 
+                  \<and> (s\<^sub>c, s\<^sub>c') \<in> G\<^sub>c \<and> (s\<^sub>a, s\<^sub>a') \<in> G\<^sub>a \<and> 
+                  (\<Gamma>\<^sub>c, (e\<^sub>c', s\<^sub>c', x\<^sub>c), R\<^sub>c, G\<^sub>c) \<preceq>\<^sub>e\<^sub>@\<^sub>k \<^sub>(\<^sub>\<alpha>\<^sub>;\<^sub>\<eta>\<^sub>;\<^sub>\<zeta>\<^sub>;\<^sub>\<gamma>\<^sub>) (\<Gamma>\<^sub>a, (e\<^sub>a', s\<^sub>a', x\<^sub>a), R\<^sub>a, G\<^sub>a))"
+    by (simp add: EvtSys_Sound_help5)  
+  then obtain e\<^sub>a' s\<^sub>a' where a4: "(\<Gamma>\<^sub>a \<turnstile>\<^sub>a (e\<^sub>a, s\<^sub>a, x\<^sub>a) -et-((Cmd Pa)\<sharp>k)\<rightarrow> (e\<^sub>a', s\<^sub>a', x\<^sub>a)) \<and>
+                (s\<^sub>c, s\<^sub>c') \<in> G\<^sub>c \<and> (s\<^sub>a, s\<^sub>a') \<in> G\<^sub>a \<and> 
+                (\<Gamma>\<^sub>c, (e\<^sub>c', s\<^sub>c', x\<^sub>c), R\<^sub>c, G\<^sub>c) \<preceq>\<^sub>e\<^sub>@\<^sub>k \<^sub>(\<^sub>\<alpha>\<^sub>;\<^sub>\<eta>\<^sub>;\<^sub>\<zeta>\<^sub>;\<^sub>\<gamma>\<^sub>) (\<Gamma>\<^sub>a, (e\<^sub>a', s\<^sub>a', x\<^sub>a), R\<^sub>a, G\<^sub>a)"
+    by auto
+  with a3 have a5: "e\<^sub>a' \<noteq> AnonyEvent fin_com\<^sub>a"
+    by (meson EvtSys_Sound_help2)
+  with a4 have a6: "\<Gamma>\<^sub>a \<turnstile>\<^sub>a (EvtSeq e\<^sub>a es\<^sub>a, s\<^sub>a, x\<^sub>a) -es-Cmd Pa\<sharp>k\<rightarrow> (EvtSeq e\<^sub>a' es\<^sub>a, s\<^sub>a', x\<^sub>a)"
+    by (simp add: Event\<^sub>a.EvtSeq1)
+  with a4 show ?thesis by blast
+qed
+
+lemma EvtSeq_Sound_lemma4: "\<lbrakk>\<zeta> (x\<^sub>c k) Pc = Some Pa;
+      (\<Gamma>\<^sub>c,(e\<^sub>c, s\<^sub>c, x\<^sub>c),R\<^sub>c,G\<^sub>c) \<preceq>\<^sub>e\<^sub>@\<^sub>k \<^sub>(\<^sub>\<alpha>\<^sub>;\<^sub>\<eta>\<^sub>;\<^sub>\<zeta>\<^sub>;\<^sub>\<gamma>\<^sub>) (\<Gamma>\<^sub>a,(e\<^sub>a, s\<^sub>a, x\<^sub>a),R\<^sub>a,G\<^sub>a);
+      \<forall>s\<^sub>c s\<^sub>a x\<^sub>c x\<^sub>a. (s\<^sub>c, s\<^sub>a) \<in> \<gamma> \<longrightarrow> (\<Gamma>\<^sub>c,(es\<^sub>c, s\<^sub>c, x\<^sub>c),R\<^sub>c,G\<^sub>c) \<preceq>\<^sub>e\<^sub>s\<^sub>@\<^sub>k \<^sub>(\<^sub>\<alpha>\<^sub>;\<^sub>\<eta>\<^sub>;\<^sub>\<zeta>\<^sub>) (\<Gamma>\<^sub>a,(es\<^sub>a, s\<^sub>a, x\<^sub>a),R\<^sub>a,G\<^sub>a); 
+      \<Gamma>\<^sub>c \<turnstile>\<^sub>c (e\<^sub>c, s\<^sub>c, x\<^sub>c) -et- Cmd Pc\<sharp>k\<rightarrow> (AnonyEvent fin_com\<^sub>c, s\<^sub>c', x\<^sub>c)\<rbrakk> \<Longrightarrow>  
+      \<exists>e\<^sub>a' s\<^sub>a'.
+          (\<Gamma>\<^sub>a \<turnstile>\<^sub>a (EvtSeq e\<^sub>a es\<^sub>a, s\<^sub>a, x\<^sub>a) -es-Cmd Pa\<sharp>k\<rightarrow> (es\<^sub>a, s\<^sub>a', x\<^sub>a)) \<and>
+          (s\<^sub>c, s\<^sub>c') \<in> G\<^sub>c \<and> (s\<^sub>a, s\<^sub>a') \<in> G\<^sub>a \<and> 
+          (\<Gamma>\<^sub>c,(es\<^sub>c, s\<^sub>c', x\<^sub>c),R\<^sub>c,G\<^sub>c) \<preceq>\<^sub>e\<^sub>s\<^sub>@\<^sub>k \<^sub>(\<^sub>\<alpha>\<^sub>;\<^sub>\<eta>\<^sub>;\<^sub>\<zeta>\<^sub>) (\<Gamma>\<^sub>a,(es\<^sub>a, s\<^sub>a', x\<^sub>a),R\<^sub>a,G\<^sub>a)"
+proof-
+  assume a0: "(\<Gamma>\<^sub>c,(e\<^sub>c, s\<^sub>c, x\<^sub>c),R\<^sub>c,G\<^sub>c) \<preceq>\<^sub>e\<^sub>@\<^sub>k \<^sub>(\<^sub>\<alpha>\<^sub>;\<^sub>\<eta>\<^sub>;\<^sub>\<zeta>\<^sub>;\<^sub>\<gamma>\<^sub>) (\<Gamma>\<^sub>a,(e\<^sub>a, s\<^sub>a, x\<^sub>a),R\<^sub>a,G\<^sub>a)"
+     and a1: "\<forall>s\<^sub>c s\<^sub>a x\<^sub>c x\<^sub>a. (s\<^sub>c, s\<^sub>a) \<in> \<gamma> \<longrightarrow> (\<Gamma>\<^sub>c,(es\<^sub>c, s\<^sub>c, x\<^sub>c),R\<^sub>c,G\<^sub>c) \<preceq>\<^sub>e\<^sub>s\<^sub>@\<^sub>k \<^sub>(\<^sub>\<alpha>\<^sub>;\<^sub>\<eta>\<^sub>;\<^sub>\<zeta>\<^sub>) (\<Gamma>\<^sub>a,(es\<^sub>a, s\<^sub>a, x\<^sub>a),R\<^sub>a,G\<^sub>a)"
+     and a2: "\<Gamma>\<^sub>c \<turnstile>\<^sub>c (e\<^sub>c, s\<^sub>c, x\<^sub>c) -et- Cmd Pc\<sharp>k\<rightarrow> (AnonyEvent fin_com\<^sub>c, s\<^sub>c', x\<^sub>c)"
+     and a3: "\<zeta> (x\<^sub>c k) Pc = Some Pa"
+  from a0 a2 a3 have "(\<exists>e\<^sub>a' s\<^sub>a'. (\<Gamma>\<^sub>a \<turnstile>\<^sub>a (e\<^sub>a, s\<^sub>a, x\<^sub>a) -et-((Cmd Pa)\<sharp>k)\<rightarrow> (e\<^sub>a', s\<^sub>a', x\<^sub>a)) 
+                  \<and> (s\<^sub>c, s\<^sub>c') \<in> G\<^sub>c \<and> (s\<^sub>a, s\<^sub>a') \<in> G\<^sub>a \<and> 
+                  (\<Gamma>\<^sub>c, (AnonyEvent fin_com\<^sub>c, s\<^sub>c', x\<^sub>c), R\<^sub>c, G\<^sub>c) \<preceq>\<^sub>e\<^sub>@\<^sub>k \<^sub>(\<^sub>\<alpha>\<^sub>;\<^sub>\<eta>\<^sub>;\<^sub>\<zeta>\<^sub>;\<^sub>\<gamma>\<^sub>) (\<Gamma>\<^sub>a, (e\<^sub>a', s\<^sub>a', x\<^sub>a), R\<^sub>a, G\<^sub>a))"
+    by (simp add: EvtSys_Sound_help5)
+  then obtain e\<^sub>a' s\<^sub>a' where a4: "(\<Gamma>\<^sub>a \<turnstile>\<^sub>a (e\<^sub>a, s\<^sub>a, x\<^sub>a) -et-((Cmd Pa)\<sharp>k)\<rightarrow> (e\<^sub>a', s\<^sub>a', x\<^sub>a)) 
+                  \<and> (s\<^sub>c, s\<^sub>c') \<in> G\<^sub>c \<and> (s\<^sub>a, s\<^sub>a') \<in> G\<^sub>a \<and> 
+                  (\<Gamma>\<^sub>c, (AnonyEvent fin_com\<^sub>c, s\<^sub>c', x\<^sub>c), R\<^sub>c, G\<^sub>c) \<preceq>\<^sub>e\<^sub>@\<^sub>k \<^sub>(\<^sub>\<alpha>\<^sub>;\<^sub>\<eta>\<^sub>;\<^sub>\<zeta>\<^sub>;\<^sub>\<gamma>\<^sub>) (\<Gamma>\<^sub>a, (e\<^sub>a', s\<^sub>a', x\<^sub>a), R\<^sub>a, G\<^sub>a)"
+    by auto
+  then have a5: "e\<^sub>a' = AnonyEvent fin_com\<^sub>a \<and> (s\<^sub>c', s\<^sub>a') \<in> \<gamma>"
+    by (meson EvtSys_Sound_help3)
+  with a4 have a6: "\<Gamma>\<^sub>a \<turnstile>\<^sub>a (EvtSeq e\<^sub>a es\<^sub>a, s\<^sub>a, x\<^sub>a) -es-Cmd Pa\<sharp>k\<rightarrow> (es\<^sub>a, s\<^sub>a', x\<^sub>a)"
+    by (metis Event\<^sub>a.EvtSeq2)
+  from a1 a5 have a7: "(\<Gamma>\<^sub>c,(es\<^sub>c, s\<^sub>c', x\<^sub>c),R\<^sub>c,G\<^sub>c) \<preceq>\<^sub>e\<^sub>s\<^sub>@\<^sub>k \<^sub>(\<^sub>\<alpha>\<^sub>;\<^sub>\<eta>\<^sub>;\<^sub>\<zeta>\<^sub>) (\<Gamma>\<^sub>a,(es\<^sub>a, s\<^sub>a', x\<^sub>a),R\<^sub>a,G\<^sub>a)"
+    by blast
+  with a4 a6 show ?thesis by blast
+qed
+
+theorem EvtSeq_rule: "\<lbrakk> \<eta> (x\<^sub>c k) = x\<^sub>a k; 
+     (\<Gamma>\<^sub>c, (e\<^sub>c, s\<^sub>c, x\<^sub>c), R\<^sub>c, G\<^sub>c) \<preceq>\<^sub>e\<^sub>@\<^sub>k \<^sub>(\<^sub>\<alpha>\<^sub>;\<^sub>\<eta>\<^sub>;\<^sub>\<zeta>\<^sub>;\<^sub>\<gamma>\<^sub>) (\<Gamma>\<^sub>a, (e\<^sub>a, s\<^sub>a, x\<^sub>a), R\<^sub>a, G\<^sub>a);
+      \<forall>s\<^sub>c s\<^sub>a x\<^sub>c x\<^sub>a. (s\<^sub>c, s\<^sub>a) \<in> \<gamma> \<longrightarrow> (\<Gamma>\<^sub>c, (es\<^sub>c, s\<^sub>c, x\<^sub>c), R\<^sub>c, G\<^sub>c)\<preceq>\<^sub>e\<^sub>s\<^sub>@\<^sub>k \<^sub>(\<^sub>\<alpha>\<^sub>;\<^sub>\<eta>\<^sub>;\<^sub>\<zeta>\<^sub>) (\<Gamma>\<^sub>a, (es\<^sub>a, s\<^sub>a, x\<^sub>a), R\<^sub>a, G\<^sub>a)\<rbrakk> 
+       \<Longrightarrow> (\<Gamma>\<^sub>c, (EvtSeq e\<^sub>c es\<^sub>c, s\<^sub>c, x\<^sub>c), R\<^sub>c, G\<^sub>c) \<preceq>\<^sub>e\<^sub>s\<^sub>@\<^sub>k \<^sub>(\<^sub>\<alpha>\<^sub>;\<^sub>\<eta>\<^sub>;\<^sub>\<zeta>\<^sub>) (\<Gamma>\<^sub>a, (EvtSeq e\<^sub>a es\<^sub>a, s\<^sub>a, x\<^sub>a), R\<^sub>a, G\<^sub>a)"
+  apply (coinduction arbitrary: e\<^sub>c s\<^sub>c x\<^sub>c e\<^sub>a s\<^sub>a x\<^sub>a, clarsimp)
+  apply (rule conjI, simp add: e_sim_init)
+  apply (rule conjI, clarsimp)
+   apply (erule Event\<^sub>c.estran.cases, simp)
+    apply (drule_tac  x\<^sub>c = x\<^sub>c and k = k  and ec = e\<^sub>c' in EvtSeq_Sound_lemma1, simp_all)
+    apply (metis Event\<^sub>a.entevt_ines_chg_selfx Event\<^sub>c.EvtSeq1 Event\<^sub>c.entevt_ines_chg_selfx)
+   apply (drule_tac  x\<^sub>c = x\<^sub>c and k = k  and ec = e\<^sub>c' in EvtSeq_Sound_lemma2, simp_all)
+   apply blast
+  apply (rule conjI, clarsimp)
+   apply (erule Event\<^sub>c.estran.cases, simp)
+    apply (metis EvtSys_Sound_help4 esys.inject(1) fst_conv snd_conv)
+   apply (metis Event\<^sub>c.evt_not_eq_in_tran EvtSys_Sound_help2 EvtSys_Sound_help3 EvtSys_Sound_help4 
+          esys.inject(1) fst_conv snd_conv)
+  apply (rule conjI, clarsimp)
+   apply (erule Event\<^sub>c.estran.cases, simp)
+    apply (drule_tac x\<^sub>c = x\<^sub>c and k = k and Pc = Pc in EvtSeq_Sound_lemma3, simp_all)
+    apply blast
+   apply (drule_tac x\<^sub>c = x\<^sub>c and k = k and Pc = Pc in EvtSeq_Sound_lemma4, simp_all)
+   apply auto[1]
+  by (meson EvtSys_Sound_help6 Un_iff pair_in_Id_conv)
+
+definition coPre :: "[('s\<^sub>c \<times> 's\<^sub>a) set, 'Env\<^sub>c, ('l\<^sub>c,'k,'s\<^sub>c,'prog\<^sub>c) event set, ('s\<^sub>c \<times> 's\<^sub>c) set, ('s\<^sub>c \<times> 's\<^sub>c) set, 
+                  'k, ('s\<^sub>c \<times> 's\<^sub>a) set, 
                   ('l\<^sub>c,'k,'s\<^sub>c,'prog\<^sub>c) event \<Rightarrow> ('l\<^sub>a,'k,'s\<^sub>a,'prog\<^sub>a) event, 
                   ('l\<^sub>c,'k,'s\<^sub>c,'prog\<^sub>c) event \<Rightarrow> 'prog\<^sub>c \<Rightarrow> 'prog\<^sub>a option,
-                  'Env\<^sub>a, ('l\<^sub>a,'k,'s\<^sub>a,'prog\<^sub>a) esys, ('s\<^sub>a \<times> 's\<^sub>a) set, ('s\<^sub>a \<times> 's\<^sub>a) set] \<Rightarrow> bool" 
-  ("'(_,_,_,_')/ \<preceq>\<^sub>e\<^sub>s \<^sub>'(\<^sub>_\<^sub>;\<^sub>_\<^sub>;\<^sub>_\<^sub>;\<^sub>_\<^sub>') /'(_,_,_,_')" [81,81,81,81,81,81,81,81,81,81,81,81] 100)
-  where "(\<Gamma>\<^sub>c,es\<^sub>c,R\<^sub>c,G\<^sub>c) \<preceq>\<^sub>e\<^sub>s \<^sub>(\<^sub>\<xi>\<^sub>;\<^sub>\<alpha>\<^sub>;\<^sub>\<eta>\<^sub>;\<^sub>\<kappa>\<^sub>) (\<Gamma>\<^sub>a,es\<^sub>a,R\<^sub>a,G\<^sub>a) \<equiv> (\<forall>s\<^sub>c s\<^sub>a x\<^sub>c x\<^sub>a k. (s\<^sub>c, s\<^sub>a) \<in> \<xi> \<longrightarrow> \<eta> (x\<^sub>c k) = x\<^sub>a k  
-         \<longrightarrow> (\<Gamma>\<^sub>c, (es\<^sub>c, s\<^sub>c, x\<^sub>c), R\<^sub>c, G\<^sub>c) \<preceq>\<^sub>e\<^sub>s \<^sub>(\<^sub>\<alpha>\<^sub>;\<^sub>\<eta>\<^sub>;\<^sub>\<kappa>\<^sub>) (\<Gamma>\<^sub>a, (es\<^sub>a, s\<^sub>a, x\<^sub>a), R\<^sub>a, G\<^sub>a))"
+                  'Env\<^sub>a, ('l\<^sub>a,'k,'s\<^sub>a,'prog\<^sub>a) event set, ('s\<^sub>a \<times> 's\<^sub>a) set, ('s\<^sub>a \<times> 's\<^sub>a) set,
+                  'Env\<^sub>c, ('l\<^sub>c,'k,'s\<^sub>c,'prog\<^sub>c) esconf, ('s\<^sub>c \<times> 's\<^sub>c) set, ('s\<^sub>c \<times> 's\<^sub>c) set,
+                  'k, ('s\<^sub>c \<times> 's\<^sub>a) set, 
+                  ('l\<^sub>c,'k,'s\<^sub>c,'prog\<^sub>c) event \<Rightarrow> ('l\<^sub>a,'k,'s\<^sub>a,'prog\<^sub>a) event, 
+                  ('l\<^sub>c,'k,'s\<^sub>c,'prog\<^sub>c) event \<Rightarrow> 'prog\<^sub>c \<Rightarrow> 'prog\<^sub>a option,
+                  'Env\<^sub>a, ('l\<^sub>a,'k,'s\<^sub>a,'prog\<^sub>a) esconf, ('s\<^sub>a \<times> 's\<^sub>a) set, ('s\<^sub>a \<times> 's\<^sub>a) set] \<Rightarrow> bool"
+  where "coPre \<gamma> \<Gamma>\<^sub>c es\<^sub>c R\<^sub>c G\<^sub>c k \<alpha> \<eta> \<zeta> \<Gamma>\<^sub>a es\<^sub>a R\<^sub>a G\<^sub>a \<Gamma>\<^sub>c' esconf\<^sub>c' R\<^sub>c' G\<^sub>c' k' \<alpha>' \<eta>' \<zeta>' \<Gamma>\<^sub>a' esconf\<^sub>a' R\<^sub>a' G\<^sub>a' \<equiv> 
+         \<exists>s\<^sub>c s\<^sub>a x\<^sub>c x\<^sub>a e\<^sub>c e\<^sub>a.
+         \<Gamma>\<^sub>c' = \<Gamma>\<^sub>c \<and> R\<^sub>c' = R\<^sub>c \<and> G\<^sub>c' = G\<^sub>c \<and> k' = k \<and> \<alpha>' = \<alpha> \<and> \<eta>' = \<eta> \<and> \<zeta>' = \<zeta> \<and> \<Gamma>\<^sub>a' = \<Gamma>\<^sub>a \<and> R\<^sub>a' = R\<^sub>a \<and> G\<^sub>a' = G\<^sub>a \<and>
+         ((esconf\<^sub>c' = (EvtSeq e\<^sub>c (EvtSys es\<^sub>c), s\<^sub>c, x\<^sub>c) \<and> esconf\<^sub>a' = (EvtSeq e\<^sub>a (EvtSys es\<^sub>a), s\<^sub>a, x\<^sub>a) \<and>
+          (\<Gamma>\<^sub>c, (e\<^sub>c, s\<^sub>c, x\<^sub>c), R\<^sub>c, G\<^sub>c) \<preceq>\<^sub>e\<^sub>@\<^sub>k \<^sub>(\<^sub>\<alpha>\<^sub>;\<^sub>\<eta>\<^sub>;\<^sub>\<zeta>\<^sub>;\<^sub>\<gamma>\<^sub>) (\<Gamma>\<^sub>a, (e\<^sub>a, s\<^sub>a, x\<^sub>a), R\<^sub>a, G\<^sub>a)) \<or>
+          (esconf\<^sub>c' = (EvtSys es\<^sub>c, s\<^sub>c, x\<^sub>c) \<and> esconf\<^sub>a' = (EvtSys es\<^sub>a, s\<^sub>a, x\<^sub>a) \<and> (s\<^sub>c, s\<^sub>a) \<in> \<gamma>)
+         )
+         "
 
-lemma es_sim_init :"(\<Gamma>\<^sub>c, (es\<^sub>c, s\<^sub>c, x\<^sub>c), R\<^sub>c, G\<^sub>c) \<preceq>\<^sub>e\<^sub>s \<^sub>(\<^sub>\<alpha>\<^sub>;\<^sub>\<eta>\<^sub>;\<^sub>\<kappa>\<^sub>) (\<Gamma>\<^sub>a, (es\<^sub>a, s\<^sub>a, x\<^sub>a), R\<^sub>a, G\<^sub>a) \<Longrightarrow> (s\<^sub>c, s\<^sub>a) \<in> \<alpha>"
-  by (erule es_sim.cases, simp_all)
+lemma EvtSys_Sound_lemma1: "\<lbrakk>\<Gamma>\<^sub>c \<turnstile>\<^sub>c (e\<^sub>c, s\<^sub>c, x\<^sub>c) -et-Cmd Pc\<sharp>k\<rightarrow> (e\<^sub>c', s\<^sub>c', x\<^sub>c); \<zeta> (x\<^sub>c k) Pc = Some Pa;
+      (\<Gamma>\<^sub>c,(e\<^sub>c, s\<^sub>c, x\<^sub>c),R\<^sub>c,G\<^sub>c) \<preceq>\<^sub>e\<^sub>@\<^sub>k \<^sub>(\<^sub>\<alpha>\<^sub>;\<^sub>\<eta>\<^sub>;\<^sub>\<zeta>\<^sub>;\<^sub>\<gamma>\<^sub>) (\<Gamma>\<^sub>a,(e\<^sub>a, s\<^sub>a, x\<^sub>a),R\<^sub>a,G\<^sub>a); e\<^sub>c' \<noteq> AnonyEvent fin_com\<^sub>c \<rbrakk> \<Longrightarrow>
+      \<eta> (x\<^sub>c k) = x\<^sub>a k \<and>
+       (\<exists>es\<^sub>a' s\<^sub>a'.
+           (\<Gamma>\<^sub>a \<turnstile>\<^sub>a (EvtSeq e\<^sub>a (EvtSys es\<^sub>a), s\<^sub>a, x\<^sub>a) -es-Cmd Pa\<sharp>k\<rightarrow> (es\<^sub>a', s\<^sub>a', x\<^sub>a)) \<and>
+           (s\<^sub>c, s\<^sub>c') \<in> G\<^sub>c \<and>
+           (s\<^sub>a, s\<^sub>a') \<in> G\<^sub>a \<and>
+           ((\<exists>e\<^sub>a. es\<^sub>a' = EvtSeq e\<^sub>a (EvtSys es\<^sub>a) \<and> (\<Gamma>\<^sub>c,(e\<^sub>c', s\<^sub>c', x\<^sub>c),R\<^sub>c,G\<^sub>c) \<preceq>\<^sub>e\<^sub>@\<^sub>k \<^sub>(\<^sub>\<alpha>\<^sub>;\<^sub>\<eta>\<^sub>;\<^sub>\<zeta>\<^sub>;\<^sub>\<gamma>\<^sub>) (\<Gamma>\<^sub>a,(e\<^sub>a, s\<^sub>a', x\<^sub>a),R\<^sub>a,G\<^sub>a)) \<or>
+            (\<Gamma>\<^sub>c,(EvtSeq e\<^sub>c' (EvtSys es\<^sub>c), s\<^sub>c', x\<^sub>c),R\<^sub>c,G\<^sub>c) \<preceq>\<^sub>e\<^sub>s\<^sub>@\<^sub>k \<^sub>(\<^sub>\<alpha>\<^sub>;\<^sub>\<eta>\<^sub>;\<^sub>\<zeta>\<^sub>) (\<Gamma>\<^sub>a,(es\<^sub>a', s\<^sub>a', x\<^sub>a),R\<^sub>a,G\<^sub>a)))"
+proof-
+  assume a0: "\<Gamma>\<^sub>c \<turnstile>\<^sub>c (e\<^sub>c, s\<^sub>c, x\<^sub>c) -et-Cmd Pc\<sharp>k\<rightarrow> (e\<^sub>c', s\<^sub>c', x\<^sub>c)"
+     and a1: "\<zeta> (x\<^sub>c k) Pc = Some Pa"
+     and a2: "(\<Gamma>\<^sub>c,(e\<^sub>c, s\<^sub>c, x\<^sub>c),R\<^sub>c,G\<^sub>c) \<preceq>\<^sub>e\<^sub>@\<^sub>k \<^sub>(\<^sub>\<alpha>\<^sub>;\<^sub>\<eta>\<^sub>;\<^sub>\<zeta>\<^sub>;\<^sub>\<gamma>\<^sub>) (\<Gamma>\<^sub>a,(e\<^sub>a, s\<^sub>a, x\<^sub>a),R\<^sub>a,G\<^sub>a)"
+     and a3: "e\<^sub>c' \<noteq> AnonyEvent fin_com\<^sub>c"
+
+  then have "\<eta> (x\<^sub>c k) = x\<^sub>a k \<and> (\<exists>e\<^sub>a' s\<^sub>a'. (\<Gamma>\<^sub>a \<turnstile>\<^sub>a (e\<^sub>a, s\<^sub>a, x\<^sub>a) -et-((Cmd Pa)\<sharp>k)\<rightarrow> (e\<^sub>a', s\<^sub>a', x\<^sub>a))
+             \<and> (s\<^sub>c, s\<^sub>c') \<in> G\<^sub>c \<and> (s\<^sub>a, s\<^sub>a') \<in> G\<^sub>a \<and> 
+             (\<Gamma>\<^sub>c, (e\<^sub>c', s\<^sub>c', x\<^sub>c), R\<^sub>c, G\<^sub>c) \<preceq>\<^sub>e\<^sub>@\<^sub>k \<^sub>(\<^sub>\<alpha>\<^sub>;\<^sub>\<eta>\<^sub>;\<^sub>\<zeta>\<^sub>;\<^sub>\<gamma>\<^sub>) (\<Gamma>\<^sub>a, (e\<^sub>a', s\<^sub>a', x\<^sub>a), R\<^sub>a, G\<^sub>a))"
+    by (simp add: EvtSys_Sound_help5)
+  then obtain e\<^sub>a' s\<^sub>a' where a4: "\<eta> (x\<^sub>c k) = x\<^sub>a k \<and> (\<Gamma>\<^sub>a \<turnstile>\<^sub>a (e\<^sub>a, s\<^sub>a, x\<^sub>a) -et-((Cmd Pa)\<sharp>k)\<rightarrow> (e\<^sub>a', s\<^sub>a', x\<^sub>a))
+             \<and> (s\<^sub>c, s\<^sub>c') \<in> G\<^sub>c \<and> (s\<^sub>a, s\<^sub>a') \<in> G\<^sub>a \<and> 
+             (\<Gamma>\<^sub>c, (e\<^sub>c', s\<^sub>c', x\<^sub>c), R\<^sub>c, G\<^sub>c) \<preceq>\<^sub>e\<^sub>@\<^sub>k \<^sub>(\<^sub>\<alpha>\<^sub>;\<^sub>\<eta>\<^sub>;\<^sub>\<zeta>\<^sub>;\<^sub>\<gamma>\<^sub>) (\<Gamma>\<^sub>a, (e\<^sub>a', s\<^sub>a', x\<^sub>a), R\<^sub>a, G\<^sub>a)" by auto
+  with a3 have a5: "e\<^sub>a' \<noteq> AnonyEvent fin_com\<^sub>a" 
+    by (meson EvtSys_Sound_help2)
+  with a4 have a6: "\<Gamma>\<^sub>a \<turnstile>\<^sub>a (EvtSeq e\<^sub>a (EvtSys es\<^sub>a), s\<^sub>a, x\<^sub>a) -es-Cmd Pa\<sharp>k\<rightarrow> (EvtSeq e\<^sub>a' (EvtSys es\<^sub>a), s\<^sub>a', x\<^sub>a)"
+    by (simp add: Event\<^sub>a.EvtSeq1)
+  with a4 show ?thesis by auto
+qed
+
+lemma EvtSys_Sound_lemma2: "\<lbrakk>\<Gamma>\<^sub>c \<turnstile>\<^sub>c (e\<^sub>c, s\<^sub>c, x\<^sub>c) -et-Cmd Pc\<sharp>k\<rightarrow> (e\<^sub>c', s\<^sub>c', x\<^sub>c); \<zeta> (x\<^sub>c k) Pc = Some Pa;
+      (\<Gamma>\<^sub>c,(e\<^sub>c, s\<^sub>c, x\<^sub>c),R\<^sub>c,G\<^sub>c) \<preceq>\<^sub>e\<^sub>@\<^sub>k \<^sub>(\<^sub>\<alpha>\<^sub>;\<^sub>\<eta>\<^sub>;\<^sub>\<zeta>\<^sub>;\<^sub>\<gamma>\<^sub>) (\<Gamma>\<^sub>a,(e\<^sub>a, s\<^sub>a, x\<^sub>a),R\<^sub>a,G\<^sub>a); e\<^sub>c' = AnonyEvent fin_com\<^sub>c \<rbrakk> \<Longrightarrow>
+      \<eta> (x\<^sub>c k) = x\<^sub>a k \<and>
+      (\<exists>es\<^sub>a' s\<^sub>a'. (\<Gamma>\<^sub>a \<turnstile>\<^sub>a (EvtSeq e\<^sub>a (EvtSys es\<^sub>a), s\<^sub>a, x\<^sub>a) -es-Cmd Pa\<sharp>k\<rightarrow> (es\<^sub>a', s\<^sub>a', x\<^sub>a)) \<and>
+      (s\<^sub>c, s\<^sub>c') \<in> G\<^sub>c \<and> (s\<^sub>a, s\<^sub>a') \<in> G\<^sub>a \<and> 
+      (es\<^sub>a' = EvtSys es\<^sub>a \<and> (s\<^sub>c', s\<^sub>a') \<in> \<gamma> \<or> (\<Gamma>,(EvtSys es\<^sub>c, s\<^sub>c', x\<^sub>c),R\<^sub>c,G\<^sub>c) \<preceq>\<^sub>e\<^sub>s\<^sub>@\<^sub>k \<^sub>(\<^sub>\<alpha>\<^sub>;\<^sub>\<eta>\<^sub>;\<^sub>\<zeta>\<^sub>) (\<Gamma>\<^sub>a,(es\<^sub>a', s\<^sub>a', x\<^sub>a),R\<^sub>a,G\<^sub>a)))"
+proof-
+  assume a0: "\<Gamma>\<^sub>c \<turnstile>\<^sub>c (e\<^sub>c, s\<^sub>c, x\<^sub>c) -et-Cmd Pc\<sharp>k\<rightarrow> (e\<^sub>c', s\<^sub>c', x\<^sub>c)"
+     and a1: "\<zeta> (x\<^sub>c k) Pc = Some Pa"
+     and a2: "(\<Gamma>\<^sub>c,(e\<^sub>c, s\<^sub>c, x\<^sub>c),R\<^sub>c,G\<^sub>c) \<preceq>\<^sub>e\<^sub>@\<^sub>k \<^sub>(\<^sub>\<alpha>\<^sub>;\<^sub>\<eta>\<^sub>;\<^sub>\<zeta>\<^sub>;\<^sub>\<gamma>\<^sub>) (\<Gamma>\<^sub>a,(e\<^sub>a, s\<^sub>a, x\<^sub>a),R\<^sub>a,G\<^sub>a)"
+     and a3: "e\<^sub>c' = AnonyEvent fin_com\<^sub>c"
+
+  then have "\<eta> (x\<^sub>c k) = x\<^sub>a k \<and> (\<exists>e\<^sub>a' s\<^sub>a'. (\<Gamma>\<^sub>a \<turnstile>\<^sub>a (e\<^sub>a, s\<^sub>a, x\<^sub>a) -et-((Cmd Pa)\<sharp>k)\<rightarrow> (e\<^sub>a', s\<^sub>a', x\<^sub>a))
+             \<and> (s\<^sub>c, s\<^sub>c') \<in> G\<^sub>c \<and> (s\<^sub>a, s\<^sub>a') \<in> G\<^sub>a \<and> 
+             (\<Gamma>\<^sub>c, (e\<^sub>c', s\<^sub>c', x\<^sub>c), R\<^sub>c, G\<^sub>c) \<preceq>\<^sub>e\<^sub>@\<^sub>k \<^sub>(\<^sub>\<alpha>\<^sub>;\<^sub>\<eta>\<^sub>;\<^sub>\<zeta>\<^sub>;\<^sub>\<gamma>\<^sub>) (\<Gamma>\<^sub>a, (e\<^sub>a', s\<^sub>a', x\<^sub>a), R\<^sub>a, G\<^sub>a))"
+    by (simp add: EvtSys_Sound_help5)
+  then obtain e\<^sub>a' s\<^sub>a' where a4: "\<eta> (x\<^sub>c k) = x\<^sub>a k \<and> (\<Gamma>\<^sub>a \<turnstile>\<^sub>a (e\<^sub>a, s\<^sub>a, x\<^sub>a) -et-((Cmd Pa)\<sharp>k)\<rightarrow> (e\<^sub>a', s\<^sub>a', x\<^sub>a))
+             \<and> (s\<^sub>c, s\<^sub>c') \<in> G\<^sub>c \<and> (s\<^sub>a, s\<^sub>a') \<in> G\<^sub>a \<and> 
+             (\<Gamma>\<^sub>c, (e\<^sub>c', s\<^sub>c', x\<^sub>c), R\<^sub>c, G\<^sub>c) \<preceq>\<^sub>e\<^sub>@\<^sub>k \<^sub>(\<^sub>\<alpha>\<^sub>;\<^sub>\<eta>\<^sub>;\<^sub>\<zeta>\<^sub>;\<^sub>\<gamma>\<^sub>) (\<Gamma>\<^sub>a, (e\<^sub>a', s\<^sub>a', x\<^sub>a), R\<^sub>a, G\<^sub>a)" by auto
+  with a3 have a5: "e\<^sub>a' = AnonyEvent fin_com\<^sub>a" 
+    by (meson EvtSys_Sound_help3)
+  with a4 have a6: "\<Gamma>\<^sub>a \<turnstile>\<^sub>a (EvtSeq e\<^sub>a (EvtSys es\<^sub>a), s\<^sub>a, x\<^sub>a) -es-Cmd Pa\<sharp>k\<rightarrow> (EvtSys es\<^sub>a, s\<^sub>a', x\<^sub>a)"
+    by (meson Event\<^sub>a.EvtSeq2)
+  with a3 a4 show ?thesis by (metis EvtSys_Sound_help3 )
+qed
+
+theorem EvtSys_rule: "\<lbrakk>\<forall>e\<^sub>c \<in> es\<^sub>c. is_basicevt e\<^sub>c; \<forall>e\<^sub>a \<in> es\<^sub>a. is_basicevt e\<^sub>a; \<forall>e\<^sub>c \<in> es\<^sub>c. \<eta> e\<^sub>c \<in> es\<^sub>a;
+                      \<forall>s\<^sub>c s\<^sub>a x\<^sub>c x\<^sub>a e\<^sub>c. e\<^sub>c \<in> es\<^sub>c \<longrightarrow>(s\<^sub>c, s\<^sub>a) \<in> \<gamma> \<longrightarrow> 
+                      (\<Gamma>\<^sub>c, (e\<^sub>c, s\<^sub>c, x\<^sub>c), R\<^sub>c, G\<^sub>c) \<preceq>\<^sub>e\<^sub>@\<^sub>k \<^sub>(\<^sub>\<alpha>\<^sub>;\<^sub>\<eta>\<^sub>;\<^sub>\<zeta>\<^sub>;\<^sub>\<gamma>\<^sub>) (\<Gamma>\<^sub>a, (\<eta> e\<^sub>c, s\<^sub>a, x\<^sub>a), R\<^sub>a, G\<^sub>a);
+                      (s\<^sub>c, s\<^sub>a) \<in> \<gamma>; \<gamma> \<subseteq> \<alpha>; Stable \<gamma> ((R\<^sub>c \<union> Id, R\<^sub>a \<union> Id)\<^sub>\<alpha>)\<rbrakk> \<Longrightarrow> 
+       (\<Gamma>\<^sub>c, (EvtSys es\<^sub>c, s\<^sub>c, x\<^sub>c), R\<^sub>c, G\<^sub>c) \<preceq>\<^sub>e\<^sub>s\<^sub>@\<^sub>k \<^sub>(\<^sub>\<alpha>\<^sub>;\<^sub>\<eta>\<^sub>;\<^sub>\<zeta>\<^sub>) (\<Gamma>\<^sub>a, (EvtSys es\<^sub>a, s\<^sub>a, x\<^sub>a), R\<^sub>a, G\<^sub>a)"
+  apply (coinduct taking: "coPre \<gamma> \<Gamma>\<^sub>c es\<^sub>c R\<^sub>c G\<^sub>c k \<alpha> \<eta> \<zeta> \<Gamma>\<^sub>a es\<^sub>a R\<^sub>a G\<^sub>a" rule:es_sim.coinduct)
+   apply (simp add: coPre_def, clarsimp)
+  apply (rule conjI, simp add: coPre_def, clarsimp)
+  apply (meson e_sim_init subsetD)
+  apply (rule conjI, clarsimp)
+   apply (erule Event\<^sub>c.estran.cases, simp_all add: coPre_def)
+     apply (metis Event\<^sub>a.event_axioms Event\<^sub>c.ent_spec1 EvtSys_Sound_help1 event.EvtOccur)
+  apply (metis Event\<^sub>a.event_axioms EvtSys_Sound_help1 EvtSys_Sound_help2 event.EvtSeq1)
+   apply (metis Event\<^sub>c.basicevt_not_tran_fin Event\<^sub>c.ent_spec1)
+  apply (rule conjI, clarsimp)
+   apply (erule Event\<^sub>c.estran.cases, simp_all add: coPre_def)
+     apply (metis Event\<^sub>c.EvtOccur Event\<^sub>c.cmd_enable_impl_notesys)
+    apply (metis EvtSys_Sound_help4)
+   apply (metis Event\<^sub>c.evt_not_eq_in_tran EvtSys_Sound_help2 EvtSys_Sound_help3 EvtSys_Sound_help4)
+  apply (rule conjI, clarsimp)
+   apply (erule Event\<^sub>c.estran.cases, simp_all add: coPre_def)
+     apply (metis Event\<^sub>c.cmd_enable_impl_notesys Event\<^sub>c.event_axioms event.EvtOccur)
+  apply clarsimp
+    apply (rule EvtSys_Sound_lemma1, simp_all)
+   apply clarsimp
+   apply (rule EvtSys_Sound_lemma2, simp_all)
+  apply clarsimp
+  apply (rule_tac x = s\<^sub>c'' and y = s\<^sub>a'' in ex2I)
+  apply (rule_tac x = x\<^sub>c' and y = x\<^sub>a' in ex2I, simp)
+  apply (case_tac "a = EvtSys es\<^sub>c \<and> aa = s\<^sub>c' \<and> b = x\<^sub>c \<and> ab = EvtSys es\<^sub>a \<and> ac = s\<^sub>a' \<and> ba = x\<^sub>a \<and> (s\<^sub>c', s\<^sub>a') \<in> \<gamma>", 
+          simp add: Stable_def)
+  apply clarsimp
+  by (meson EvtSys_Sound_help6)
 
 coinductive pes_sim :: "['Env\<^sub>c, ('l\<^sub>c,'k,'s\<^sub>c,'prog\<^sub>c) pesconf, 
                   ('s\<^sub>c \<times> 's\<^sub>a) set, 
@@ -286,52 +508,52 @@ coinductive pes_sim :: "['Env\<^sub>c, ('l\<^sub>c,'k,'s\<^sub>c,'prog\<^sub>c) 
   ("'(_,_')/ \<preceq>\<^sub>p\<^sub>e\<^sub>s \<^sub>'(\<^sub>_\<^sub>;\<^sub>_\<^sub>;\<^sub>_\<^sub>') /'(_,_')" [81,81,81,81,81,81,81] 100)
   where rgsim : "\<lbrakk>(s\<^sub>c, s\<^sub>a) \<in> \<alpha>; 
                   
-                  (\<forall>ec pes\<^sub>c' x\<^sub>c' k. (\<Gamma>\<^sub>c \<turnstile>\<^sub>c (pes\<^sub>c, s\<^sub>c, x\<^sub>c) -pes-((EvtEnt ec)\<sharp>k)\<rightarrow> (pes\<^sub>c', s\<^sub>c, x\<^sub>c')) \<longrightarrow>(\<exists>ea pes\<^sub>a' x\<^sub>a'. 
-                  (\<Gamma>\<^sub>a \<turnstile>\<^sub>a (pes\<^sub>a, s\<^sub>a, x\<^sub>a) -pes-((EvtEnt ea)\<sharp>k)\<rightarrow> (pes\<^sub>a', s\<^sub>a, x\<^sub>a')) \<and> \<eta> ec = ea \<and> 
-                  (\<Gamma>\<^sub>c, (pes\<^sub>c', s\<^sub>c, x\<^sub>c')) \<preceq>\<^sub>p\<^sub>e\<^sub>s \<^sub>(\<^sub>\<alpha>\<^sub>;\<^sub>\<eta>\<^sub>;\<^sub>\<kappa>\<^sub>) (\<Gamma>\<^sub>a, (pes\<^sub>a', s\<^sub>a, x\<^sub>a'))));
+                  \<forall>ec pes\<^sub>c' x\<^sub>c' k. (\<Gamma>\<^sub>c \<turnstile>\<^sub>c (pes\<^sub>c, s\<^sub>c, x\<^sub>c) -pes-((EvtEnt ec)\<sharp>k)\<rightarrow> (pes\<^sub>c', s\<^sub>c, x\<^sub>c')) \<longrightarrow>(\<exists>pes\<^sub>a' x\<^sub>a'. 
+                  (\<Gamma>\<^sub>a \<turnstile>\<^sub>a (pes\<^sub>a, s\<^sub>a, x\<^sub>a) -pes-((EvtEnt (\<eta> ec))\<sharp>k)\<rightarrow> (pes\<^sub>a', s\<^sub>a, x\<^sub>a')) \<and> 
+                  (\<Gamma>\<^sub>c, (pes\<^sub>c', s\<^sub>c, x\<^sub>c')) \<preceq>\<^sub>p\<^sub>e\<^sub>s \<^sub>(\<^sub>\<alpha>\<^sub>;\<^sub>\<eta>\<^sub>;\<^sub>\<zeta>\<^sub>) (\<Gamma>\<^sub>a, (pes\<^sub>a', s\<^sub>a, x\<^sub>a')));
 
-                  (\<forall>Pc pes\<^sub>c' s\<^sub>c' k. (\<Gamma>\<^sub>c \<turnstile>\<^sub>c (pes\<^sub>c, s\<^sub>c, x\<^sub>c) -pes-((Cmd Pc)\<sharp>k)\<rightarrow> (pes\<^sub>c', s\<^sub>c', x\<^sub>c)) \<and> \<kappa> (x\<^sub>c k) Pc = None \<longrightarrow>
-                  (\<Gamma>\<^sub>c, (pes\<^sub>c', s\<^sub>c', x\<^sub>c)) \<preceq>\<^sub>p\<^sub>e\<^sub>s \<^sub>(\<^sub>\<alpha>\<^sub>;\<^sub>\<eta>\<^sub>;\<^sub>\<kappa>\<^sub>) (\<Gamma>\<^sub>a, (pes\<^sub>a, s\<^sub>a, x\<^sub>a)));
+                  \<forall>Pc pes\<^sub>c' s\<^sub>c' k. (\<Gamma>\<^sub>c \<turnstile>\<^sub>c (pes\<^sub>c, s\<^sub>c, x\<^sub>c) -pes-((Cmd Pc)\<sharp>k)\<rightarrow> (pes\<^sub>c', s\<^sub>c', x\<^sub>c)) \<and> \<zeta> (x\<^sub>c k) Pc = None \<longrightarrow>
+                  (\<Gamma>\<^sub>c, (pes\<^sub>c', s\<^sub>c', x\<^sub>c)) \<preceq>\<^sub>p\<^sub>e\<^sub>s \<^sub>(\<^sub>\<alpha>\<^sub>;\<^sub>\<eta>\<^sub>;\<^sub>\<zeta>\<^sub>) (\<Gamma>\<^sub>a, (pes\<^sub>a, s\<^sub>a, x\<^sub>a));
 
-                  (\<forall>Pc pes\<^sub>c' s\<^sub>c' k Pa. (\<Gamma>\<^sub>c \<turnstile>\<^sub>c (pes\<^sub>c, s\<^sub>c, x\<^sub>c) -pes-((Cmd Pc)\<sharp>k)\<rightarrow> (pes\<^sub>c', s\<^sub>c', x\<^sub>c)) \<and> \<kappa> (x\<^sub>c k) Pc = Some Pa \<longrightarrow>
+                  \<forall>Pc pes\<^sub>c' s\<^sub>c' k Pa. (\<Gamma>\<^sub>c \<turnstile>\<^sub>c (pes\<^sub>c, s\<^sub>c, x\<^sub>c) -pes-((Cmd Pc)\<sharp>k)\<rightarrow> (pes\<^sub>c', s\<^sub>c', x\<^sub>c)) \<and> \<zeta> (x\<^sub>c k) Pc = Some Pa \<longrightarrow>
                   (\<exists>pes\<^sub>a' s\<^sub>a'. (\<Gamma>\<^sub>a \<turnstile>\<^sub>a (pes\<^sub>a, s\<^sub>a, x\<^sub>a) -pes-((Cmd Pa)\<sharp>k)\<rightarrow> (pes\<^sub>a', s\<^sub>a', x\<^sub>a)) \<and> \<eta> (x\<^sub>c k) = (x\<^sub>a k)
-                  \<and> (\<Gamma>\<^sub>c, (pes\<^sub>c', s\<^sub>c', x\<^sub>c)) \<preceq>\<^sub>p\<^sub>e\<^sub>s \<^sub>(\<^sub>\<alpha>\<^sub>;\<^sub>\<eta>\<^sub>;\<^sub>\<kappa>\<^sub>) (\<Gamma>\<^sub>a, (pes\<^sub>a', s\<^sub>a', x\<^sub>a)))) 
+                  \<and> (\<Gamma>\<^sub>c, (pes\<^sub>c', s\<^sub>c', x\<^sub>c)) \<preceq>\<^sub>p\<^sub>e\<^sub>s \<^sub>(\<^sub>\<alpha>\<^sub>;\<^sub>\<eta>\<^sub>;\<^sub>\<zeta>\<^sub>) (\<Gamma>\<^sub>a, (pes\<^sub>a', s\<^sub>a', x\<^sub>a))) 
      
-                  \<rbrakk> \<Longrightarrow> (\<Gamma>\<^sub>c, (pes\<^sub>c, s\<^sub>c, x\<^sub>c)) \<preceq>\<^sub>p\<^sub>e\<^sub>s \<^sub>(\<^sub>\<alpha>\<^sub>;\<^sub>\<eta>\<^sub>;\<^sub>\<kappa>\<^sub>) (\<Gamma>\<^sub>a, (pes\<^sub>a, s\<^sub>a, x\<^sub>a))"
+                  \<rbrakk> \<Longrightarrow> (\<Gamma>\<^sub>c, (pes\<^sub>c, s\<^sub>c, x\<^sub>c)) \<preceq>\<^sub>p\<^sub>e\<^sub>s \<^sub>(\<^sub>\<alpha>\<^sub>;\<^sub>\<eta>\<^sub>;\<^sub>\<zeta>\<^sub>) (\<Gamma>\<^sub>a, (pes\<^sub>a, s\<^sub>a, x\<^sub>a))"
 
 
-lemma pes_sim_init :"(\<Gamma>\<^sub>c, (pes\<^sub>c, s\<^sub>c, x\<^sub>c)) \<preceq>\<^sub>p\<^sub>e\<^sub>s \<^sub>(\<^sub>\<alpha>\<^sub>;\<^sub>\<eta>\<^sub>;\<^sub>\<kappa>\<^sub>) (\<Gamma>\<^sub>a, (pes\<^sub>a, s\<^sub>a, x\<^sub>a)) \<Longrightarrow> (s\<^sub>c, s\<^sub>a) \<in> \<alpha>"
+lemma pes_sim_init :"(\<Gamma>\<^sub>c, (pes\<^sub>c, s\<^sub>c, x\<^sub>c)) \<preceq>\<^sub>p\<^sub>e\<^sub>s \<^sub>(\<^sub>\<alpha>\<^sub>;\<^sub>\<eta>\<^sub>;\<^sub>\<zeta>\<^sub>) (\<Gamma>\<^sub>a, (pes\<^sub>a, s\<^sub>a, x\<^sub>a)) \<Longrightarrow> (s\<^sub>c, s\<^sub>a) \<in> \<alpha>"
   by (erule pes_sim.cases, simp_all)
 
-lemma Pes_Sound_help1: "\<lbrakk>(\<Gamma>\<^sub>c, (es\<^sub>c, s\<^sub>c, x\<^sub>c), R\<^sub>c, G\<^sub>c) \<preceq>\<^sub>e\<^sub>s \<^sub>(\<^sub>\<alpha>\<^sub>;\<^sub>\<eta>\<^sub>;\<^sub>\<kappa>\<^sub>) (\<Gamma>\<^sub>a, (es\<^sub>a, s\<^sub>a, x\<^sub>a), R\<^sub>a, G\<^sub>a);
+lemma Pes_Sound_help1: "\<lbrakk>(\<Gamma>\<^sub>c, (es\<^sub>c, s\<^sub>c, x\<^sub>c), R\<^sub>c, G\<^sub>c) \<preceq>\<^sub>e\<^sub>s\<^sub>@\<^sub>k \<^sub>(\<^sub>\<alpha>\<^sub>;\<^sub>\<eta>\<^sub>;\<^sub>\<zeta>\<^sub>) (\<Gamma>\<^sub>a, (es\<^sub>a, s\<^sub>a, x\<^sub>a), R\<^sub>a, G\<^sub>a);
        \<Gamma>\<^sub>c \<turnstile>\<^sub>c (es\<^sub>c, s\<^sub>c, x\<^sub>c) -es-((EvtEnt e\<^sub>c)\<sharp>k)\<rightarrow> (es\<^sub>c', s\<^sub>c, x\<^sub>c')\<rbrakk> \<Longrightarrow> \<exists> es\<^sub>a' x\<^sub>a'. 
                    (\<Gamma>\<^sub>a \<turnstile>\<^sub>a (es\<^sub>a, s\<^sub>a, x\<^sub>a) -es-((EvtEnt (\<eta> e\<^sub>c))\<sharp>k)\<rightarrow> (es\<^sub>a', s\<^sub>a, x\<^sub>a')) \<and> 
-                    (\<Gamma>\<^sub>c, (es\<^sub>c', s\<^sub>c, x\<^sub>c'), R\<^sub>c, G\<^sub>c) \<preceq>\<^sub>e\<^sub>s \<^sub>(\<^sub>\<alpha>\<^sub>;\<^sub>\<eta>\<^sub>;\<^sub>\<kappa>\<^sub>) (\<Gamma>\<^sub>a, (es\<^sub>a', s\<^sub>a, x\<^sub>a'), R\<^sub>a, G\<^sub>a)"
+                    (\<Gamma>\<^sub>c, (es\<^sub>c', s\<^sub>c, x\<^sub>c'), R\<^sub>c, G\<^sub>c) \<preceq>\<^sub>e\<^sub>s\<^sub>@\<^sub>k \<^sub>(\<^sub>\<alpha>\<^sub>;\<^sub>\<eta>\<^sub>;\<^sub>\<zeta>\<^sub>) (\<Gamma>\<^sub>a, (es\<^sub>a', s\<^sub>a, x\<^sub>a'), R\<^sub>a, G\<^sub>a)"
   by (erule es_sim.cases, simp)
 
-lemma Pes_Sound_help2: "\<lbrakk>(\<Gamma>\<^sub>c, (es\<^sub>c, s\<^sub>c, x\<^sub>c), R\<^sub>c, G\<^sub>c) \<preceq>\<^sub>e\<^sub>s \<^sub>(\<^sub>\<alpha>\<^sub>;\<^sub>\<eta>\<^sub>;\<^sub>\<kappa>\<^sub>) (\<Gamma>\<^sub>a, (es\<^sub>a, s\<^sub>a, x\<^sub>a), R\<^sub>a, G\<^sub>a);
-      (s\<^sub>c, s\<^sub>c') \<in> R\<^sub>c \<union> Id \<and> (s\<^sub>a, s\<^sub>a') \<in>  R\<^sub>a \<union> Id; x\<^sub>c' k = x\<^sub>c k \<and> x\<^sub>a' k = x\<^sub>a k\<rbrakk> \<Longrightarrow>
-      (\<Gamma>\<^sub>c, (es\<^sub>c, s\<^sub>c', x\<^sub>c'), R\<^sub>c, G\<^sub>c) \<preceq>\<^sub>e\<^sub>s \<^sub>(\<^sub>\<alpha>\<^sub>;\<^sub>\<eta>\<^sub>;\<^sub>\<kappa>\<^sub>) (\<Gamma>\<^sub>a, (es\<^sub>a, s\<^sub>a', x\<^sub>a'), R\<^sub>a, G\<^sub>a)"
+lemma Pes_Sound_help2: "\<lbrakk>(\<Gamma>\<^sub>c, (es\<^sub>c, s\<^sub>c, x\<^sub>c), R\<^sub>c, G\<^sub>c) \<preceq>\<^sub>e\<^sub>s\<^sub>@\<^sub>k \<^sub>(\<^sub>\<alpha>\<^sub>;\<^sub>\<eta>\<^sub>;\<^sub>\<zeta>\<^sub>) (\<Gamma>\<^sub>a, (es\<^sub>a, s\<^sub>a, x\<^sub>a), R\<^sub>a, G\<^sub>a);
+      ((s\<^sub>c, s\<^sub>c'),(s\<^sub>a, s\<^sub>a')) \<in> (R\<^sub>c \<union> Id, R\<^sub>a \<union> Id)\<^sub>\<alpha>; x\<^sub>c' k = x\<^sub>c k \<and> x\<^sub>a' k = x\<^sub>a k\<rbrakk> \<Longrightarrow>
+      (\<Gamma>\<^sub>c, (es\<^sub>c, s\<^sub>c', x\<^sub>c'), R\<^sub>c, G\<^sub>c) \<preceq>\<^sub>e\<^sub>s\<^sub>@\<^sub>k \<^sub>(\<^sub>\<alpha>\<^sub>;\<^sub>\<eta>\<^sub>;\<^sub>\<zeta>\<^sub>) (\<Gamma>\<^sub>a, (es\<^sub>a, s\<^sub>a', x\<^sub>a'), R\<^sub>a, G\<^sub>a)"
   by (erule es_sim.cases, simp)
 
-lemma Pes_Sound_help3: "\<lbrakk>(\<Gamma>\<^sub>c, (es\<^sub>c, s\<^sub>c, x\<^sub>c), R\<^sub>c, G\<^sub>c) \<preceq>\<^sub>e\<^sub>s \<^sub>(\<^sub>\<alpha>\<^sub>;\<^sub>\<eta>\<^sub>;\<^sub>\<kappa>\<^sub>) (\<Gamma>\<^sub>a, (es\<^sub>a, s\<^sub>a, x\<^sub>a), R\<^sub>a, G\<^sub>a);
-      (\<Gamma>\<^sub>c \<turnstile>\<^sub>c (es\<^sub>c, s\<^sub>c, x\<^sub>c) -es-((Cmd Pc)\<sharp>k)\<rightarrow> (es\<^sub>c', s\<^sub>c', x\<^sub>c)) \<and> \<kappa> (x\<^sub>c k) Pc = None\<rbrakk> \<Longrightarrow>
-      (s\<^sub>c, s\<^sub>c') \<in> G\<^sub>c \<and> (\<Gamma>\<^sub>c, (es\<^sub>c', s\<^sub>c', x\<^sub>c), R\<^sub>c, G\<^sub>c) \<preceq>\<^sub>e\<^sub>s \<^sub>(\<^sub>\<alpha>\<^sub>;\<^sub>\<eta>\<^sub>;\<^sub>\<kappa>\<^sub>) (\<Gamma>\<^sub>a, (es\<^sub>a, s\<^sub>a, x\<^sub>a), R\<^sub>a, G\<^sub>a)"
+lemma Pes_Sound_help3: "\<lbrakk>(\<Gamma>\<^sub>c, (es\<^sub>c, s\<^sub>c, x\<^sub>c), R\<^sub>c, G\<^sub>c) \<preceq>\<^sub>e\<^sub>s\<^sub>@\<^sub>k \<^sub>(\<^sub>\<alpha>\<^sub>;\<^sub>\<eta>\<^sub>;\<^sub>\<zeta>\<^sub>) (\<Gamma>\<^sub>a, (es\<^sub>a, s\<^sub>a, x\<^sub>a), R\<^sub>a, G\<^sub>a);
+      (\<Gamma>\<^sub>c \<turnstile>\<^sub>c (es\<^sub>c, s\<^sub>c, x\<^sub>c) -es-((Cmd Pc)\<sharp>k)\<rightarrow> (es\<^sub>c', s\<^sub>c', x\<^sub>c)) \<and> \<zeta> (x\<^sub>c k) Pc = None\<rbrakk> \<Longrightarrow>
+      (s\<^sub>c, s\<^sub>c') \<in> G\<^sub>c \<and> (\<Gamma>\<^sub>c, (es\<^sub>c', s\<^sub>c', x\<^sub>c), R\<^sub>c, G\<^sub>c) \<preceq>\<^sub>e\<^sub>s\<^sub>@\<^sub>k \<^sub>(\<^sub>\<alpha>\<^sub>;\<^sub>\<eta>\<^sub>;\<^sub>\<zeta>\<^sub>) (\<Gamma>\<^sub>a, (es\<^sub>a, s\<^sub>a, x\<^sub>a), R\<^sub>a, G\<^sub>a)"
   by (erule es_sim.cases, simp)
 
-lemma Pes_Sound_help4: "\<lbrakk>(\<Gamma>\<^sub>c, (es\<^sub>c, s\<^sub>c, x\<^sub>c), R\<^sub>c, G\<^sub>c) \<preceq>\<^sub>e\<^sub>s \<^sub>(\<^sub>\<alpha>\<^sub>;\<^sub>\<eta>\<^sub>;\<^sub>\<kappa>\<^sub>) (\<Gamma>\<^sub>a, (es\<^sub>a, s\<^sub>a, x\<^sub>a), R\<^sub>a, G\<^sub>a);
-      (\<Gamma>\<^sub>c \<turnstile>\<^sub>c (es\<^sub>c, s\<^sub>c, x\<^sub>c) -es-((Cmd Pc)\<sharp>k)\<rightarrow> (es\<^sub>c', s\<^sub>c', x\<^sub>c)) \<and> \<kappa> (x\<^sub>c k) Pc = Some Pa\<rbrakk> \<Longrightarrow>
+lemma Pes_Sound_help4: "\<lbrakk>(\<Gamma>\<^sub>c, (es\<^sub>c, s\<^sub>c, x\<^sub>c), R\<^sub>c, G\<^sub>c) \<preceq>\<^sub>e\<^sub>s\<^sub>@\<^sub>k \<^sub>(\<^sub>\<alpha>\<^sub>;\<^sub>\<eta>\<^sub>;\<^sub>\<zeta>\<^sub>) (\<Gamma>\<^sub>a, (es\<^sub>a, s\<^sub>a, x\<^sub>a), R\<^sub>a, G\<^sub>a);
+      (\<Gamma>\<^sub>c \<turnstile>\<^sub>c (es\<^sub>c, s\<^sub>c, x\<^sub>c) -es-((Cmd Pc)\<sharp>k)\<rightarrow> (es\<^sub>c', s\<^sub>c', x\<^sub>c)) \<and> \<zeta> (x\<^sub>c k) Pc = Some Pa\<rbrakk> \<Longrightarrow>
       \<eta> (x\<^sub>c k) = x\<^sub>a k \<and>(\<exists>es\<^sub>a' s\<^sub>a'. (\<Gamma>\<^sub>a \<turnstile>\<^sub>a (es\<^sub>a, s\<^sub>a, x\<^sub>a) -es-((Cmd Pa)\<sharp>k)\<rightarrow> (es\<^sub>a', s\<^sub>a', x\<^sub>a)) \<and> 
-      (s\<^sub>c, s\<^sub>c') \<in> G\<^sub>c \<and> (s\<^sub>a, s\<^sub>a') \<in> G\<^sub>a \<and> (\<Gamma>\<^sub>c, (es\<^sub>c', s\<^sub>c', x\<^sub>c), R\<^sub>c, G\<^sub>c) \<preceq>\<^sub>e\<^sub>s \<^sub>(\<^sub>\<alpha>\<^sub>;\<^sub>\<eta>\<^sub>;\<^sub>\<kappa>\<^sub>) (\<Gamma>\<^sub>a, (es\<^sub>a', s\<^sub>a', x\<^sub>a), R\<^sub>a, G\<^sub>a))"
+      (s\<^sub>c, s\<^sub>c') \<in> G\<^sub>c \<and> (s\<^sub>a, s\<^sub>a') \<in> G\<^sub>a \<and> (\<Gamma>\<^sub>c, (es\<^sub>c', s\<^sub>c', x\<^sub>c), R\<^sub>c, G\<^sub>c) \<preceq>\<^sub>e\<^sub>s\<^sub>@\<^sub>k \<^sub>(\<^sub>\<alpha>\<^sub>;\<^sub>\<eta>\<^sub>;\<^sub>\<zeta>\<^sub>) (\<Gamma>\<^sub>a, (es\<^sub>a', s\<^sub>a', x\<^sub>a), R\<^sub>a, G\<^sub>a))"
   by (erule es_sim.cases, simp)
 
-lemma Pes_Sound_lemma1: " \<lbrakk>\<forall>k. (\<Gamma>\<^sub>c,(pes\<^sub>c k, s\<^sub>c, x\<^sub>c),R\<^sub>c k,G\<^sub>c k) \<preceq>\<^sub>e\<^sub>s \<^sub>(\<^sub>\<alpha>\<^sub>;\<^sub>\<eta>\<^sub>;\<^sub>\<kappa>\<^sub>) (\<Gamma>\<^sub>a,(pes\<^sub>a k, s\<^sub>a, x\<^sub>a),R\<^sub>a k,G\<^sub>a k);
+lemma Pes_Sound_lemma1: " \<lbrakk>\<forall>k. (\<Gamma>\<^sub>c,(pes\<^sub>c k, s\<^sub>c, x\<^sub>c),R\<^sub>c k,G\<^sub>c k) \<preceq>\<^sub>e\<^sub>s\<^sub>@\<^sub>k \<^sub>(\<^sub>\<alpha>\<^sub>;\<^sub>\<eta>\<^sub>;\<^sub>\<zeta>\<^sub>) (\<Gamma>\<^sub>a,(pes\<^sub>a k, s\<^sub>a, x\<^sub>a),R\<^sub>a k,G\<^sub>a k);
       \<forall>i j. i \<noteq> j \<longrightarrow> G\<^sub>c i \<subseteq> R\<^sub>c j \<and> G\<^sub>a i \<subseteq> R\<^sub>a j; \<Gamma>\<^sub>c \<turnstile>\<^sub>c (pes\<^sub>c, s\<^sub>c, x\<^sub>c) -pes-EvtEnt e\<^sub>c\<sharp>k\<rightarrow> (pes\<^sub>c', s\<^sub>c, x\<^sub>c')\<rbrakk>
        \<Longrightarrow> \<exists>pes\<^sub>a' x\<^sub>a'.
             (\<Gamma>\<^sub>a \<turnstile>\<^sub>a (pes\<^sub>a, s\<^sub>a, x\<^sub>a) -pes-EvtEnt (\<eta> e\<^sub>c)\<sharp>k\<rightarrow> (pes\<^sub>a', s\<^sub>a, x\<^sub>a')) \<and>
-            (\<forall>k. (\<Gamma>\<^sub>c,(pes\<^sub>c' k, s\<^sub>c, x\<^sub>c'),R\<^sub>c k,G\<^sub>c k) \<preceq>\<^sub>e\<^sub>s \<^sub>(\<^sub>\<alpha>\<^sub>;\<^sub>\<eta>\<^sub>;\<^sub>\<kappa>\<^sub>) (\<Gamma>\<^sub>a,(pes\<^sub>a' k, s\<^sub>a, x\<^sub>a'),R\<^sub>a k,G\<^sub>a k))"
+            (\<forall>k. (\<Gamma>\<^sub>c,(pes\<^sub>c' k, s\<^sub>c, x\<^sub>c'),R\<^sub>c k,G\<^sub>c k) \<preceq>\<^sub>e\<^sub>s\<^sub>@\<^sub>k \<^sub>(\<^sub>\<alpha>\<^sub>;\<^sub>\<eta>\<^sub>;\<^sub>\<zeta>\<^sub>) (\<Gamma>\<^sub>a,(pes\<^sub>a' k, s\<^sub>a, x\<^sub>a'),R\<^sub>a k,G\<^sub>a k))"
 proof-
-  assume a0: "\<forall>k. (\<Gamma>\<^sub>c,(pes\<^sub>c k, s\<^sub>c, x\<^sub>c),R\<^sub>c k,G\<^sub>c k) \<preceq>\<^sub>e\<^sub>s \<^sub>(\<^sub>\<alpha>\<^sub>;\<^sub>\<eta>\<^sub>;\<^sub>\<kappa>\<^sub>) (\<Gamma>\<^sub>a,(pes\<^sub>a k, s\<^sub>a, x\<^sub>a),R\<^sub>a k,G\<^sub>a k)"
+  assume a0: "\<forall>k. (\<Gamma>\<^sub>c,(pes\<^sub>c k, s\<^sub>c, x\<^sub>c),R\<^sub>c k,G\<^sub>c k) \<preceq>\<^sub>e\<^sub>s\<^sub>@\<^sub>k \<^sub>(\<^sub>\<alpha>\<^sub>;\<^sub>\<eta>\<^sub>;\<^sub>\<zeta>\<^sub>) (\<Gamma>\<^sub>a,(pes\<^sub>a k, s\<^sub>a, x\<^sub>a),R\<^sub>a k,G\<^sub>a k)"
      and a1: "\<forall>i j. i \<noteq> j \<longrightarrow> G\<^sub>c i \<subseteq> R\<^sub>c j \<and> G\<^sub>a i \<subseteq> R\<^sub>a j"
      and a2: "\<Gamma>\<^sub>c \<turnstile>\<^sub>c (pes\<^sub>c, s\<^sub>c, x\<^sub>c) -pes-EvtEnt e\<^sub>c\<sharp>k\<rightarrow> (pes\<^sub>c', s\<^sub>c, x\<^sub>c')"
 
@@ -342,30 +564,33 @@ proof-
   then have a4: "\<forall>k'. k' \<noteq> k \<longrightarrow> x\<^sub>c k' = x\<^sub>c' k'"
     by (meson Event\<^sub>c.entevt_ines_notchg_otherx)
   from a0 a3 have "\<exists>es\<^sub>a' x\<^sub>a'. (\<Gamma>\<^sub>a \<turnstile>\<^sub>a (pes\<^sub>a k, s\<^sub>a, x\<^sub>a) -es-(EvtEnt (\<eta> e\<^sub>c)\<sharp>k)\<rightarrow> (es\<^sub>a', s\<^sub>a, x\<^sub>a')) 
-                    \<and> (\<Gamma>\<^sub>c, (es\<^sub>c', s\<^sub>c, x\<^sub>c'), R\<^sub>c k, G\<^sub>c k) \<preceq>\<^sub>e\<^sub>s \<^sub>(\<^sub>\<alpha>\<^sub>;\<^sub>\<eta>\<^sub>;\<^sub>\<kappa>\<^sub>) (\<Gamma>\<^sub>a, (es\<^sub>a', s\<^sub>a, x\<^sub>a'), R\<^sub>a k, G\<^sub>a k)"
+                    \<and> (\<Gamma>\<^sub>c, (es\<^sub>c', s\<^sub>c, x\<^sub>c'), R\<^sub>c k, G\<^sub>c k) \<preceq>\<^sub>e\<^sub>s\<^sub>@\<^sub>k \<^sub>(\<^sub>\<alpha>\<^sub>;\<^sub>\<eta>\<^sub>;\<^sub>\<zeta>\<^sub>) (\<Gamma>\<^sub>a, (es\<^sub>a', s\<^sub>a, x\<^sub>a'), R\<^sub>a k, G\<^sub>a k)"
     by (meson Pes_Sound_help1)
   then obtain es\<^sub>a' x\<^sub>a' where a5: "(\<Gamma>\<^sub>a \<turnstile>\<^sub>a (pes\<^sub>a k, s\<^sub>a, x\<^sub>a) -es-(EvtEnt (\<eta> e\<^sub>c)\<sharp>k)\<rightarrow> (es\<^sub>a', s\<^sub>a, x\<^sub>a'))
-  \<and> (\<Gamma>\<^sub>c, (es\<^sub>c', s\<^sub>c, x\<^sub>c'), R\<^sub>c k, G\<^sub>c k) \<preceq>\<^sub>e\<^sub>s \<^sub>(\<^sub>\<alpha>\<^sub>;\<^sub>\<eta>\<^sub>;\<^sub>\<kappa>\<^sub>) (\<Gamma>\<^sub>a, (es\<^sub>a', s\<^sub>a, x\<^sub>a'), R\<^sub>a k, G\<^sub>a k)" by blast
+  \<and> (\<Gamma>\<^sub>c, (es\<^sub>c', s\<^sub>c, x\<^sub>c'), R\<^sub>c k, G\<^sub>c k) \<preceq>\<^sub>e\<^sub>s\<^sub>@\<^sub>k \<^sub>(\<^sub>\<alpha>\<^sub>;\<^sub>\<eta>\<^sub>;\<^sub>\<zeta>\<^sub>) (\<Gamma>\<^sub>a, (es\<^sub>a', s\<^sub>a, x\<^sub>a'), R\<^sub>a k, G\<^sub>a k)" by blast
   then have a6: "\<forall>k'. k' \<noteq> k \<longrightarrow> x\<^sub>a k' = x\<^sub>a' k'"
     by (meson Event\<^sub>a.entevt_ines_notchg_otherx)
   from a5 have a7: "\<Gamma>\<^sub>a \<turnstile>\<^sub>a (pes\<^sub>a, s\<^sub>a, x\<^sub>a) -pes-EvtEnt (\<eta> e\<^sub>c)\<sharp>k\<rightarrow> (pes\<^sub>a(k := es\<^sub>a'), s\<^sub>a, x\<^sub>a')"
     by (meson Event\<^sub>a.pestran.intros a4)
-  have "\<forall>j. (\<Gamma>\<^sub>c,(pes\<^sub>c' j, s\<^sub>c, x\<^sub>c'),R\<^sub>c j,G\<^sub>c j) \<preceq>\<^sub>e\<^sub>s \<^sub>(\<^sub>\<alpha>\<^sub>;\<^sub>\<eta>\<^sub>;\<^sub>\<kappa>\<^sub>) (\<Gamma>\<^sub>a, ((pes\<^sub>a(k := es\<^sub>a')) j, s\<^sub>a, x\<^sub>a'),R\<^sub>a j,G\<^sub>a j)"
+  have "\<forall>j. (\<Gamma>\<^sub>c,(pes\<^sub>c' j, s\<^sub>c, x\<^sub>c'),R\<^sub>c j,G\<^sub>c j) \<preceq>\<^sub>e\<^sub>s\<^sub>@\<^sub>j \<^sub>(\<^sub>\<alpha>\<^sub>;\<^sub>\<eta>\<^sub>;\<^sub>\<zeta>\<^sub>) (\<Gamma>\<^sub>a, ((pes\<^sub>a(k := es\<^sub>a')) j, s\<^sub>a, x\<^sub>a'),R\<^sub>a j,G\<^sub>a j)"
   proof-
     {
       fix j
-      have "(\<Gamma>\<^sub>c,(pes\<^sub>c' j, s\<^sub>c, x\<^sub>c'),R\<^sub>c j,G\<^sub>c j) \<preceq>\<^sub>e\<^sub>s \<^sub>(\<^sub>\<alpha>\<^sub>;\<^sub>\<eta>\<^sub>;\<^sub>\<kappa>\<^sub>) (\<Gamma>\<^sub>a, ((pes\<^sub>a(k := es\<^sub>a')) j, s\<^sub>a, x\<^sub>a'),R\<^sub>a j,G\<^sub>a j)"
+      have "(\<Gamma>\<^sub>c,(pes\<^sub>c' j, s\<^sub>c, x\<^sub>c'),R\<^sub>c j,G\<^sub>c j) \<preceq>\<^sub>e\<^sub>s\<^sub>@\<^sub>j \<^sub>(\<^sub>\<alpha>\<^sub>;\<^sub>\<eta>\<^sub>;\<^sub>\<zeta>\<^sub>) (\<Gamma>\<^sub>a, ((pes\<^sub>a(k := es\<^sub>a')) j, s\<^sub>a, x\<^sub>a'),R\<^sub>a j,G\<^sub>a j)"
       proof(case_tac "j = k")
         assume "j = k"
         with a3 a5 show ?thesis by simp
       next
         assume b0: "j \<noteq> k"
-        with a0 a3 a4 have b1: "(\<Gamma>\<^sub>c,(pes\<^sub>c' j, s\<^sub>c, x\<^sub>c),R\<^sub>c j,G\<^sub>c j) \<preceq>\<^sub>e\<^sub>s \<^sub>(\<^sub>\<alpha>\<^sub>;\<^sub>\<eta>\<^sub>;\<^sub>\<kappa>\<^sub>) (\<Gamma>\<^sub>a,((pes\<^sub>a(k := es\<^sub>a')) j, s\<^sub>a, x\<^sub>a),R\<^sub>a j,G\<^sub>a j)"
+        with a0 a3 a4 have b1: "(\<Gamma>\<^sub>c,(pes\<^sub>c' j, s\<^sub>c, x\<^sub>c),R\<^sub>c j,G\<^sub>c j) \<preceq>\<^sub>e\<^sub>s\<^sub>@\<^sub>j \<^sub>(\<^sub>\<alpha>\<^sub>;\<^sub>\<eta>\<^sub>;\<^sub>\<zeta>\<^sub>) (\<Gamma>\<^sub>a,((pes\<^sub>a(k := es\<^sub>a')) j, s\<^sub>a, x\<^sub>a),R\<^sub>a j,G\<^sub>a j)"
           by simp
-        have b2: "(s\<^sub>c, s\<^sub>c) \<in> R\<^sub>c j \<union> Id \<and> (s\<^sub>a, s\<^sub>a) \<in> R\<^sub>a j \<union> Id" by blast
+        from b1 have "(s\<^sub>c, s\<^sub>a) \<in> \<alpha>"
+          by (simp add: es_sim_init)
+        then have b2: "((s\<^sub>c, s\<^sub>c),(s\<^sub>a, s\<^sub>a)) \<in> (R\<^sub>c j \<union> Id, R\<^sub>a j \<union> Id)\<^sub>\<alpha>"
+          by (simp add: related_transitions_def)
         from b0 a4 a6 have "x\<^sub>c j = x\<^sub>c' j \<and> x\<^sub>a j = x\<^sub>a' j" by auto
-        with b1 b2 show ?thesis
-          by (metis (full_types) Pes_Sound_help2)
+        with b1 b2 show ?thesis 
+          using Pes_Sound_help2 by fastforce        
       qed 
     }
     then show ?thesis by auto
@@ -374,52 +599,56 @@ proof-
   with a7 show ?thesis by blast
 qed
 
-lemma Pes_Sound_lemma2: "\<lbrakk>\<forall>k. (\<Gamma>\<^sub>c,(pes\<^sub>c k, s\<^sub>c, x\<^sub>c),R\<^sub>c k,G\<^sub>c k) \<preceq>\<^sub>e\<^sub>s \<^sub>(\<^sub>\<alpha>\<^sub>;\<^sub>\<eta>\<^sub>;\<^sub>\<kappa>\<^sub>) (\<Gamma>\<^sub>a,(pes\<^sub>a k, s\<^sub>a, x\<^sub>a),R\<^sub>a k,G\<^sub>a k);
+lemma Pes_Sound_lemma2: "\<lbrakk>\<forall>k. (\<Gamma>\<^sub>c,(pes\<^sub>c k, s\<^sub>c, x\<^sub>c),R\<^sub>c k,G\<^sub>c k) \<preceq>\<^sub>e\<^sub>s\<^sub>@\<^sub>k \<^sub>(\<^sub>\<alpha>\<^sub>;\<^sub>\<eta>\<^sub>;\<^sub>\<zeta>\<^sub>) (\<Gamma>\<^sub>a,(pes\<^sub>a k, s\<^sub>a, x\<^sub>a),R\<^sub>a k,G\<^sub>a k);
       \<forall>i j. i \<noteq> j \<longrightarrow> G\<^sub>c i \<subseteq> R\<^sub>c j \<and> G\<^sub>a i \<subseteq> R\<^sub>a j; \<Gamma>\<^sub>c \<turnstile>\<^sub>c (pes\<^sub>c, s\<^sub>c, x\<^sub>c) -pes-Cmd Pc\<sharp>k\<rightarrow> (pes\<^sub>c', s\<^sub>c', x\<^sub>c);
-      \<kappa> (x\<^sub>c k) Pc = None\<rbrakk> \<Longrightarrow> \<forall>k. (\<Gamma>\<^sub>c,(pes\<^sub>c' k, s\<^sub>c', x\<^sub>c),R\<^sub>c k,G\<^sub>c k) \<preceq>\<^sub>e\<^sub>s \<^sub>(\<^sub>\<alpha>\<^sub>;\<^sub>\<eta>\<^sub>;\<^sub>\<kappa>\<^sub>) (\<Gamma>\<^sub>a,(pes\<^sub>a k, s\<^sub>a, x\<^sub>a),R\<^sub>a k,G\<^sub>a k)"
+      \<zeta> (x\<^sub>c k) Pc = None\<rbrakk> \<Longrightarrow> \<forall>k. (\<Gamma>\<^sub>c,(pes\<^sub>c' k, s\<^sub>c', x\<^sub>c),R\<^sub>c k,G\<^sub>c k) \<preceq>\<^sub>e\<^sub>s\<^sub>@\<^sub>k \<^sub>(\<^sub>\<alpha>\<^sub>;\<^sub>\<eta>\<^sub>;\<^sub>\<zeta>\<^sub>) (\<Gamma>\<^sub>a,(pes\<^sub>a k, s\<^sub>a, x\<^sub>a),R\<^sub>a k,G\<^sub>a k)"
 proof-
-  assume a0: "\<forall>k. (\<Gamma>\<^sub>c,(pes\<^sub>c k, s\<^sub>c, x\<^sub>c),R\<^sub>c k,G\<^sub>c k) \<preceq>\<^sub>e\<^sub>s \<^sub>(\<^sub>\<alpha>\<^sub>;\<^sub>\<eta>\<^sub>;\<^sub>\<kappa>\<^sub>) (\<Gamma>\<^sub>a,(pes\<^sub>a k, s\<^sub>a, x\<^sub>a),R\<^sub>a k,G\<^sub>a k)"
+  assume a0: "\<forall>k. (\<Gamma>\<^sub>c,(pes\<^sub>c k, s\<^sub>c, x\<^sub>c),R\<^sub>c k,G\<^sub>c k) \<preceq>\<^sub>e\<^sub>s\<^sub>@\<^sub>k \<^sub>(\<^sub>\<alpha>\<^sub>;\<^sub>\<eta>\<^sub>;\<^sub>\<zeta>\<^sub>) (\<Gamma>\<^sub>a,(pes\<^sub>a k, s\<^sub>a, x\<^sub>a),R\<^sub>a k,G\<^sub>a k)"
      and a1: "\<forall>i j. i \<noteq> j \<longrightarrow> G\<^sub>c i \<subseteq> R\<^sub>c j \<and> G\<^sub>a i \<subseteq> R\<^sub>a j"
      and a2: "\<Gamma>\<^sub>c \<turnstile>\<^sub>c (pes\<^sub>c, s\<^sub>c, x\<^sub>c) -pes-Cmd Pc\<sharp>k\<rightarrow> (pes\<^sub>c', s\<^sub>c', x\<^sub>c)"
-     and a3: "\<kappa> (x\<^sub>c k) Pc = None"
+     and a3: "\<zeta> (x\<^sub>c k) Pc = None"
 
   from a2 have "\<exists>es\<^sub>c'. (\<Gamma>\<^sub>c \<turnstile>\<^sub>c (pes\<^sub>c k, s\<^sub>c, x\<^sub>c) -es-Cmd Pc\<sharp>k\<rightarrow> (pes\<^sub>c' k, s\<^sub>c', x\<^sub>c)) \<and> pes\<^sub>c' = pes\<^sub>c(k :=es\<^sub>c')"
     using Event\<^sub>c.pestran_estran by fastforce
   then obtain es\<^sub>c' where a4: "(\<Gamma>\<^sub>c \<turnstile>\<^sub>c (pes\<^sub>c k, s\<^sub>c, x\<^sub>c) -es-Cmd Pc\<sharp>k\<rightarrow> (pes\<^sub>c' k, s\<^sub>c', x\<^sub>c)) \<and> pes\<^sub>c' = pes\<^sub>c(k :=es\<^sub>c')"
     by auto
-  with a0 a3 have a5: "(s\<^sub>c, s\<^sub>c') \<in> G\<^sub>c k \<and> (\<Gamma>\<^sub>c, (es\<^sub>c', s\<^sub>c', x\<^sub>c), R\<^sub>c k, G\<^sub>c k) \<preceq>\<^sub>e\<^sub>s \<^sub>(\<^sub>\<alpha>\<^sub>;\<^sub>\<eta>\<^sub>;\<^sub>\<kappa>\<^sub>) (\<Gamma>\<^sub>a, (pes\<^sub>a k, s\<^sub>a, x\<^sub>a), R\<^sub>a k, G\<^sub>a k)"
+  with a0 a3 have a5: "(s\<^sub>c, s\<^sub>c') \<in> G\<^sub>c k \<and> (\<Gamma>\<^sub>c, (es\<^sub>c', s\<^sub>c', x\<^sub>c), R\<^sub>c k, G\<^sub>c k) \<preceq>\<^sub>e\<^sub>s\<^sub>@\<^sub>k \<^sub>(\<^sub>\<alpha>\<^sub>;\<^sub>\<eta>\<^sub>;\<^sub>\<zeta>\<^sub>) (\<Gamma>\<^sub>a, (pes\<^sub>a k, s\<^sub>a, x\<^sub>a), R\<^sub>a k, G\<^sub>a k)"
     by (metis Pes_Sound_help3 fun_upd_same)
   show ?thesis
   proof-
     {
       fix j
-      have "(\<Gamma>\<^sub>c,(pes\<^sub>c' j, s\<^sub>c', x\<^sub>c),R\<^sub>c j,G\<^sub>c j) \<preceq>\<^sub>e\<^sub>s \<^sub>(\<^sub>\<alpha>\<^sub>;\<^sub>\<eta>\<^sub>;\<^sub>\<kappa>\<^sub>) (\<Gamma>\<^sub>a,(pes\<^sub>a j, s\<^sub>a, x\<^sub>a),R\<^sub>a j,G\<^sub>a j)"
+      have "(\<Gamma>\<^sub>c,(pes\<^sub>c' j, s\<^sub>c', x\<^sub>c),R\<^sub>c j,G\<^sub>c j) \<preceq>\<^sub>e\<^sub>s\<^sub>@\<^sub>j \<^sub>(\<^sub>\<alpha>\<^sub>;\<^sub>\<eta>\<^sub>;\<^sub>\<zeta>\<^sub>) (\<Gamma>\<^sub>a,(pes\<^sub>a j, s\<^sub>a, x\<^sub>a),R\<^sub>a j,G\<^sub>a j)"
       proof(case_tac "j = k")
         assume "j = k"
         with a4 a5 show ?thesis by force
       next
         assume b0: "j \<noteq> k"
-        with a0 a2 have b1: "(\<Gamma>\<^sub>c,(pes\<^sub>c' j, s\<^sub>c, x\<^sub>c),R\<^sub>c j,G\<^sub>c j) \<preceq>\<^sub>e\<^sub>s \<^sub>(\<^sub>\<alpha>\<^sub>;\<^sub>\<eta>\<^sub>;\<^sub>\<kappa>\<^sub>) (\<Gamma>\<^sub>a,(pes\<^sub>a j, s\<^sub>a, x\<^sub>a),R\<^sub>a j,G\<^sub>a j)"
+        with a0 a2 have b1: "(\<Gamma>\<^sub>c,(pes\<^sub>c' j, s\<^sub>c, x\<^sub>c),R\<^sub>c j,G\<^sub>c j) \<preceq>\<^sub>e\<^sub>s\<^sub>@\<^sub>j \<^sub>(\<^sub>\<alpha>\<^sub>;\<^sub>\<eta>\<^sub>;\<^sub>\<zeta>\<^sub>) (\<Gamma>\<^sub>a,(pes\<^sub>a j, s\<^sub>a, x\<^sub>a),R\<^sub>a j,G\<^sub>a j)"
           using Event\<^sub>c.pestran_estran by fastforce
-        from a1 a5 b0 have b2: "(s\<^sub>c, s\<^sub>c') \<in> R\<^sub>c j \<union> Id \<and> (s\<^sub>a, s\<^sub>a) \<in> R\<^sub>a j \<union> Id" 
-          by (metis IdI UnI1 UnI2 subsetD)
-        with b1 show ?thesis by (metis Pes_Sound_help2)
+        from b1 have "(s\<^sub>c, s\<^sub>a) \<in> \<alpha>"
+          by (simp add: es_sim_init)
+        with a1 a5 b0 have b2: "((s\<^sub>c, s\<^sub>c'),(s\<^sub>a, s\<^sub>a)) \<in> (R\<^sub>c j \<union> Id, R\<^sub>a j \<union> Id)\<^sub>\<alpha>"
+          apply (simp add: related_transitions_def)
+          by (metis es_sim_init subsetD)
+        with b1 show ?thesis 
+          using Pes_Sound_help2 by fastforce
       qed
     }
     then show ?thesis by auto
   qed
 qed
 
-lemma Pes_Sound_lemma3: "\<lbrakk>\<forall>k. (\<Gamma>\<^sub>c,(pes\<^sub>c k, s\<^sub>c, x\<^sub>c),R\<^sub>c k,G\<^sub>c k) \<preceq>\<^sub>e\<^sub>s \<^sub>(\<^sub>\<alpha>\<^sub>;\<^sub>\<eta>\<^sub>;\<^sub>\<kappa>\<^sub>) (\<Gamma>\<^sub>a,(pes\<^sub>a k, s\<^sub>a, x\<^sub>a),R\<^sub>a k,G\<^sub>a k);
+lemma Pes_Sound_lemma3: "\<lbrakk>\<forall>k. (\<Gamma>\<^sub>c,(pes\<^sub>c k, s\<^sub>c, x\<^sub>c),R\<^sub>c k,G\<^sub>c k) \<preceq>\<^sub>e\<^sub>s\<^sub>@\<^sub>k \<^sub>(\<^sub>\<alpha>\<^sub>;\<^sub>\<eta>\<^sub>;\<^sub>\<zeta>\<^sub>) (\<Gamma>\<^sub>a,(pes\<^sub>a k, s\<^sub>a, x\<^sub>a),R\<^sub>a k,G\<^sub>a k);
        \<forall>i j. i \<noteq> j \<longrightarrow> G\<^sub>c i \<subseteq> R\<^sub>c j \<and> G\<^sub>a i \<subseteq> R\<^sub>a j;\<Gamma>\<^sub>c \<turnstile>\<^sub>c (pes\<^sub>c, s\<^sub>c, x\<^sub>c) -pes-Cmd Pc\<sharp>k\<rightarrow> (pes\<^sub>c', s\<^sub>c', x\<^sub>c);
-        \<kappa> (x\<^sub>c k) Pc = Some Pa\<rbrakk> \<Longrightarrow>
+        \<zeta> (x\<^sub>c k) Pc = Some Pa\<rbrakk> \<Longrightarrow>
         \<exists>pes\<^sub>a' s\<^sub>a'. (\<Gamma>\<^sub>a \<turnstile>\<^sub>a (pes\<^sub>a, s\<^sub>a, x\<^sub>a) -pes-Cmd Pa\<sharp>k\<rightarrow> (pes\<^sub>a', s\<^sub>a', x\<^sub>a)) \<and> \<eta> (x\<^sub>c k) = x\<^sub>a k \<and>
-        (\<forall>k. (\<Gamma>\<^sub>c,(pes\<^sub>c' k, s\<^sub>c', x\<^sub>c),R\<^sub>c k,G\<^sub>c k) \<preceq>\<^sub>e\<^sub>s \<^sub>(\<^sub>\<alpha>\<^sub>;\<^sub>\<eta>\<^sub>;\<^sub>\<kappa>\<^sub>) (\<Gamma>\<^sub>a,(pes\<^sub>a' k, s\<^sub>a', x\<^sub>a),R\<^sub>a k,G\<^sub>a k))"
+        (\<forall>k. (\<Gamma>\<^sub>c,(pes\<^sub>c' k, s\<^sub>c', x\<^sub>c),R\<^sub>c k,G\<^sub>c k) \<preceq>\<^sub>e\<^sub>s\<^sub>@\<^sub>k \<^sub>(\<^sub>\<alpha>\<^sub>;\<^sub>\<eta>\<^sub>;\<^sub>\<zeta>\<^sub>) (\<Gamma>\<^sub>a,(pes\<^sub>a' k, s\<^sub>a', x\<^sub>a),R\<^sub>a k,G\<^sub>a k))"
 proof-
-  assume a0: "\<forall>k. (\<Gamma>\<^sub>c,(pes\<^sub>c k, s\<^sub>c, x\<^sub>c),R\<^sub>c k,G\<^sub>c k) \<preceq>\<^sub>e\<^sub>s \<^sub>(\<^sub>\<alpha>\<^sub>;\<^sub>\<eta>\<^sub>;\<^sub>\<kappa>\<^sub>) (\<Gamma>\<^sub>a,(pes\<^sub>a k, s\<^sub>a, x\<^sub>a),R\<^sub>a k,G\<^sub>a k)"
+  assume a0: "\<forall>k. (\<Gamma>\<^sub>c,(pes\<^sub>c k, s\<^sub>c, x\<^sub>c),R\<^sub>c k,G\<^sub>c k) \<preceq>\<^sub>e\<^sub>s\<^sub>@\<^sub>k \<^sub>(\<^sub>\<alpha>\<^sub>;\<^sub>\<eta>\<^sub>;\<^sub>\<zeta>\<^sub>) (\<Gamma>\<^sub>a,(pes\<^sub>a k, s\<^sub>a, x\<^sub>a),R\<^sub>a k,G\<^sub>a k)"
      and a1: "\<forall>i j. i \<noteq> j \<longrightarrow> G\<^sub>c i \<subseteq> R\<^sub>c j \<and> G\<^sub>a i \<subseteq> R\<^sub>a j"
      and a2: "\<Gamma>\<^sub>c \<turnstile>\<^sub>c (pes\<^sub>c, s\<^sub>c, x\<^sub>c) -pes-Cmd Pc\<sharp>k\<rightarrow> (pes\<^sub>c', s\<^sub>c', x\<^sub>c)"
-     and a3: "\<kappa> (x\<^sub>c k) Pc = Some Pa"
+     and a3: "\<zeta> (x\<^sub>c k) Pc = Some Pa"
 
   from a2 have "\<exists>es\<^sub>c'. (\<Gamma>\<^sub>c \<turnstile>\<^sub>c (pes\<^sub>c k, s\<^sub>c, x\<^sub>c) -es-Cmd Pc\<sharp>k\<rightarrow> (pes\<^sub>c' k, s\<^sub>c', x\<^sub>c)) \<and> pes\<^sub>c' = pes\<^sub>c(k :=es\<^sub>c')"
     by (metis Event\<^sub>c.pestran_estran fun_upd_same)
@@ -427,11 +656,11 @@ proof-
     by auto
   with a0 a3 have "  \<eta> (x\<^sub>c k) = x\<^sub>a k \<and> (\<exists>es\<^sub>a' s\<^sub>a'. (\<Gamma>\<^sub>a \<turnstile>\<^sub>a (pes\<^sub>a k, s\<^sub>a, x\<^sub>a) -es-((Cmd Pa)\<sharp>k)\<rightarrow> (es\<^sub>a', s\<^sub>a', x\<^sub>a)) 
                      \<and> (s\<^sub>c, s\<^sub>c') \<in> G\<^sub>c k \<and> (s\<^sub>a, s\<^sub>a') \<in> G\<^sub>a k 
-                     \<and> (\<Gamma>\<^sub>c, (es\<^sub>c', s\<^sub>c', x\<^sub>c), R\<^sub>c k, G\<^sub>c k) \<preceq>\<^sub>e\<^sub>s \<^sub>(\<^sub>\<alpha>\<^sub>;\<^sub>\<eta>\<^sub>;\<^sub>\<kappa>\<^sub>) (\<Gamma>\<^sub>a, (es\<^sub>a', s\<^sub>a', x\<^sub>a), R\<^sub>a k, G\<^sub>a k))"
+                     \<and> (\<Gamma>\<^sub>c, (es\<^sub>c', s\<^sub>c', x\<^sub>c), R\<^sub>c k, G\<^sub>c k) \<preceq>\<^sub>e\<^sub>s\<^sub>@\<^sub>k \<^sub>(\<^sub>\<alpha>\<^sub>;\<^sub>\<eta>\<^sub>;\<^sub>\<zeta>\<^sub>) (\<Gamma>\<^sub>a, (es\<^sub>a', s\<^sub>a', x\<^sub>a), R\<^sub>a k, G\<^sub>a k))"
     using Pes_Sound_help4 by fastforce
   then obtain es\<^sub>a' s\<^sub>a' where a5: "(\<Gamma>\<^sub>a \<turnstile>\<^sub>a (pes\<^sub>a k, s\<^sub>a, x\<^sub>a) -es-((Cmd Pa)\<sharp>k)\<rightarrow> (es\<^sub>a', s\<^sub>a', x\<^sub>a)) 
                       \<and> (s\<^sub>c, s\<^sub>c') \<in> G\<^sub>c k \<and> (s\<^sub>a, s\<^sub>a') \<in> G\<^sub>a k \<and> \<eta> (x\<^sub>c k) = x\<^sub>a k \<and> 
-                      (\<Gamma>\<^sub>c, (es\<^sub>c', s\<^sub>c', x\<^sub>c), R\<^sub>c k, G\<^sub>c k) \<preceq>\<^sub>e\<^sub>s \<^sub>(\<^sub>\<alpha>\<^sub>;\<^sub>\<eta>\<^sub>;\<^sub>\<kappa>\<^sub>) (\<Gamma>\<^sub>a, (es\<^sub>a', s\<^sub>a', x\<^sub>a), R\<^sub>a k, G\<^sub>a k)"
+                      (\<Gamma>\<^sub>c, (es\<^sub>c', s\<^sub>c', x\<^sub>c), R\<^sub>c k, G\<^sub>c k) \<preceq>\<^sub>e\<^sub>s\<^sub>@\<^sub>k \<^sub>(\<^sub>\<alpha>\<^sub>;\<^sub>\<eta>\<^sub>;\<^sub>\<zeta>\<^sub>) (\<Gamma>\<^sub>a, (es\<^sub>a', s\<^sub>a', x\<^sub>a), R\<^sub>a k, G\<^sub>a k)"
     by auto
   then have a6: "(\<Gamma>\<^sub>a \<turnstile>\<^sub>a (pes\<^sub>a, s\<^sub>a, x\<^sub>a) -pes-((Cmd Pa)\<sharp>k)\<rightarrow> (pes\<^sub>a (k :=es\<^sub>a'), s\<^sub>a', x\<^sub>a))"
     by (simp add: Event\<^sub>a.pestran.intros)
@@ -439,16 +668,19 @@ proof-
   proof-
     {
       fix j
-      have "(\<Gamma>\<^sub>c,(pes\<^sub>c' j, s\<^sub>c', x\<^sub>c),R\<^sub>c j,G\<^sub>c j) \<preceq>\<^sub>e\<^sub>s \<^sub>(\<^sub>\<alpha>\<^sub>;\<^sub>\<eta>\<^sub>;\<^sub>\<kappa>\<^sub>) (\<Gamma>\<^sub>a,((pes\<^sub>a (k :=es\<^sub>a')) j, s\<^sub>a', x\<^sub>a),R\<^sub>a j,G\<^sub>a j)"
+      have "(\<Gamma>\<^sub>c,(pes\<^sub>c' j, s\<^sub>c', x\<^sub>c),R\<^sub>c j,G\<^sub>c j) \<preceq>\<^sub>e\<^sub>s\<^sub>@\<^sub>j \<^sub>(\<^sub>\<alpha>\<^sub>;\<^sub>\<eta>\<^sub>;\<^sub>\<zeta>\<^sub>) (\<Gamma>\<^sub>a,((pes\<^sub>a (k :=es\<^sub>a')) j, s\<^sub>a', x\<^sub>a),R\<^sub>a j,G\<^sub>a j)"
       proof(case_tac "j = k")
         assume "j = k"
         with a4 a5 show ?thesis by simp
       next
         assume b0: "j \<noteq> k"
-        with a0 a2 have b1: "(\<Gamma>\<^sub>c,(pes\<^sub>c j, s\<^sub>c, x\<^sub>c),R\<^sub>c j,G\<^sub>c j) \<preceq>\<^sub>e\<^sub>s \<^sub>(\<^sub>\<alpha>\<^sub>;\<^sub>\<eta>\<^sub>;\<^sub>\<kappa>\<^sub>) (\<Gamma>\<^sub>a,((pes\<^sub>a (k :=es\<^sub>a')) j, s\<^sub>a, x\<^sub>a),R\<^sub>a j,G\<^sub>a j)"
+        with a0 a2 have b1: "(\<Gamma>\<^sub>c,(pes\<^sub>c j, s\<^sub>c, x\<^sub>c),R\<^sub>c j,G\<^sub>c j) \<preceq>\<^sub>e\<^sub>s\<^sub>@\<^sub>j \<^sub>(\<^sub>\<alpha>\<^sub>;\<^sub>\<eta>\<^sub>;\<^sub>\<zeta>\<^sub>) (\<Gamma>\<^sub>a,((pes\<^sub>a (k :=es\<^sub>a')) j, s\<^sub>a, x\<^sub>a),R\<^sub>a j,G\<^sub>a j)"
           by simp
-        from a1 a5 b0 have b2: "(s\<^sub>c, s\<^sub>c') \<in> R\<^sub>c j \<union> Id \<and> (s\<^sub>a, s\<^sub>a') \<in> R\<^sub>a j \<union> Id"
-          by (metis in_mono sup.cobounded1)
+        from b1 have "(s\<^sub>c, s\<^sub>a) \<in> \<alpha>"
+          by (simp add: es_sim_init)
+        from a1 a5 b0 have b2: "((s\<^sub>c, s\<^sub>c'), (s\<^sub>a, s\<^sub>a')) \<in> (R\<^sub>c j \<union> Id, R\<^sub>a j \<union> Id)\<^sub>\<alpha>"
+          apply (simp add: related_transitions_def)
+          by (metis (no_types, lifting) \<open>(s\<^sub>c, s\<^sub>a) \<in> \<alpha>\<close> es_sim_init subsetD)
         with a4 b0 b1 show ?thesis
           using Pes_Sound_help2  by fastforce
       qed
@@ -457,8 +689,8 @@ proof-
   qed
 qed
 
-lemma Pes_rule : "\<lbrakk>\<forall>k. (\<Gamma>\<^sub>c, (pes\<^sub>c k, s\<^sub>c, x\<^sub>c), (R\<^sub>c k), (G\<^sub>c k)) \<preceq>\<^sub>e\<^sub>s \<^sub>(\<^sub>\<alpha>\<^sub>;\<^sub>\<eta>\<^sub>;\<^sub>\<kappa>\<^sub>) (\<Gamma>\<^sub>a, (pes\<^sub>a k, s\<^sub>a, x\<^sub>a), (R\<^sub>a k), (G\<^sub>a k));
-             \<forall>i j. i \<noteq> j \<longrightarrow> G\<^sub>c i \<subseteq> R\<^sub>c j \<and> G\<^sub>a i \<subseteq> R\<^sub>a j\<rbrakk> \<Longrightarrow> (\<Gamma>\<^sub>c, (pes\<^sub>c, s\<^sub>c, x\<^sub>c)) \<preceq>\<^sub>p\<^sub>e\<^sub>s \<^sub>(\<^sub>\<alpha>\<^sub>;\<^sub>\<eta>\<^sub>;\<^sub>\<kappa>\<^sub>) (\<Gamma>\<^sub>a, (pes\<^sub>a, s\<^sub>a, x\<^sub>a))"
+theorem Pes_rule : "\<lbrakk>\<forall>k. (\<Gamma>\<^sub>c, (pes\<^sub>c k, s\<^sub>c, x\<^sub>c), (R\<^sub>c k), (G\<^sub>c k)) \<preceq>\<^sub>e\<^sub>s\<^sub>@\<^sub>k \<^sub>(\<^sub>\<alpha>\<^sub>;\<^sub>\<eta>\<^sub>;\<^sub>\<zeta>\<^sub>) (\<Gamma>\<^sub>a, (pes\<^sub>a k, s\<^sub>a, x\<^sub>a), (R\<^sub>a k), (G\<^sub>a k));
+             \<forall>i j. i \<noteq> j \<longrightarrow> G\<^sub>c i \<subseteq> R\<^sub>c j \<and> G\<^sub>a i \<subseteq> R\<^sub>a j\<rbrakk> \<Longrightarrow> (\<Gamma>\<^sub>c, (pes\<^sub>c, s\<^sub>c, x\<^sub>c)) \<preceq>\<^sub>p\<^sub>e\<^sub>s \<^sub>(\<^sub>\<alpha>\<^sub>;\<^sub>\<eta>\<^sub>;\<^sub>\<zeta>\<^sub>) (\<Gamma>\<^sub>a, (pes\<^sub>a, s\<^sub>a, x\<^sub>a))"
   apply (coinduction arbitrary: pes\<^sub>c s\<^sub>c x\<^sub>c pes\<^sub>a s\<^sub>a x\<^sub>a, clarsimp)
   apply (rule conjI)
    apply (meson es_sim_init)
@@ -467,7 +699,7 @@ lemma Pes_rule : "\<lbrakk>\<forall>k. (\<Gamma>\<^sub>c, (pes\<^sub>c k, s\<^su
   apply (rule conjI)
    apply (metis Pes_Sound_lemma2)
   apply clarsimp
-  apply (drule_tac Pc = Pc and k = k and pes\<^sub>c' = pes\<^sub>c' and s\<^sub>c' = s\<^sub>c' and Pa = Pa in Pes_Sound_lemma3)
+  apply (drule_tac Pc = Pc  and pes\<^sub>c' = pes\<^sub>c' and s\<^sub>c' = s\<^sub>c' and Pa = Pa in Pes_Sound_lemma3)
      apply meson
     apply blast
    apply blast
@@ -502,21 +734,21 @@ locale PiCore_RGSim =
   and dome\<^sub>a :: "'s\<^sub>a \<Rightarrow> ('l\<^sub>a, 'k, 's\<^sub>a, 'prog\<^sub>a) event \<Rightarrow> 'd" +
 fixes \<alpha> :: "('s\<^sub>c \<times> 's\<^sub>a) set"
   and \<eta> :: "('l\<^sub>c,'k,'s\<^sub>c,'prog\<^sub>c) event \<Rightarrow> ('l\<^sub>a,'k,'s\<^sub>a,'prog\<^sub>a) event"
-  and \<kappa> :: "('l\<^sub>c,'k,'s\<^sub>c,'prog\<^sub>c) event \<Rightarrow> 'prog\<^sub>c \<Rightarrow> 'prog\<^sub>a option"
+  and \<zeta> :: "('l\<^sub>c,'k,'s\<^sub>c,'prog\<^sub>c) event \<Rightarrow> 'prog\<^sub>c \<Rightarrow> 'prog\<^sub>a option"
 assumes
-  init_sim : "(\<Gamma>\<^sub>c, C0\<^sub>c) \<preceq>\<^sub>p\<^sub>e\<^sub>s \<^sub>(\<^sub>\<alpha>\<^sub>;\<^sub>\<eta>\<^sub>;\<^sub>\<kappa>\<^sub>) (\<Gamma>\<^sub>a, C0\<^sub>a)" and
+  init_sim : "(\<Gamma>\<^sub>c, C0\<^sub>c) \<preceq>\<^sub>p\<^sub>e\<^sub>s \<^sub>(\<^sub>\<alpha>\<^sub>;\<^sub>\<eta>\<^sub>;\<^sub>\<zeta>\<^sub>) (\<Gamma>\<^sub>a, C0\<^sub>a)" and
   dom_sim : "\<lbrakk>(s\<^sub>c, s\<^sub>a) \<in> \<alpha>; \<eta> e\<^sub>c = e\<^sub>a \<rbrakk> \<Longrightarrow> dome\<^sub>c s\<^sub>c e\<^sub>c = dome\<^sub>a s\<^sub>a e\<^sub>a" and
   intefere_same : "interference\<^sub>c  = interference\<^sub>a" and
   sim_state_ifs : "\<lbrakk>(s\<^sub>c, s\<^sub>a) \<in> \<alpha>; (t\<^sub>c, t\<^sub>a) \<in> \<alpha>\<rbrakk> \<Longrightarrow> s\<^sub>a \<sim>\<^sub>a d \<sim>\<^sub>a t\<^sub>a = s\<^sub>c \<sim>\<^sub>c d \<sim>\<^sub>c t\<^sub>c"
 begin
 
 definition sim_s :: "('l\<^sub>c,'k,'s\<^sub>c,'prog\<^sub>c) pesconf \<Rightarrow> ('l\<^sub>a, 'k, 's\<^sub>a, 'prog\<^sub>a) pesconf \<Rightarrow> bool" ("(_ \<sim> _)" [70,70] 60)
-  where "C\<^sub>c \<sim> C\<^sub>a = (\<Gamma>\<^sub>c, C\<^sub>c) \<preceq>\<^sub>p\<^sub>e\<^sub>s \<^sub>(\<^sub>\<alpha>\<^sub>;\<^sub>\<eta>\<^sub>;\<^sub>\<kappa>\<^sub>) (\<Gamma>\<^sub>a, C\<^sub>a)"
+  where "C\<^sub>c \<sim> C\<^sub>a = (\<Gamma>\<^sub>c, C\<^sub>c) \<preceq>\<^sub>p\<^sub>e\<^sub>s \<^sub>(\<^sub>\<alpha>\<^sub>;\<^sub>\<eta>\<^sub>;\<^sub>\<zeta>\<^sub>) (\<Gamma>\<^sub>a, C\<^sub>a)"
 
 fun sim_a :: "('l\<^sub>c, 'k, 's\<^sub>c, 'prog\<^sub>c, 'd) action \<Rightarrow> ('l\<^sub>a, 'k, 's\<^sub>a, 'prog\<^sub>a, 'd) action option"
   where "sim_a \<lparr>actk = \<lparr>Act = Cmd P\<^sub>c, K = k\<rparr>, eventof = e\<^sub>c, domain = d\<rparr> = 
-         (if (\<kappa> e\<^sub>c P\<^sub>c = None) then None 
-         else Some (let e\<^sub>a = \<eta> e\<^sub>c; P\<^sub>a = the (\<kappa> e\<^sub>c P\<^sub>c) in 
+         (if (\<zeta> e\<^sub>c P\<^sub>c = None) then None 
+         else Some (let e\<^sub>a = \<eta> e\<^sub>c; P\<^sub>a = the (\<zeta> e\<^sub>c P\<^sub>c) in 
               \<lparr>actk = \<lparr>Act = Cmd P\<^sub>a, K = k\<rparr>, eventof = e\<^sub>a, domain = d\<rparr>))" |
         "sim_a \<lparr>actk = \<lparr>Act = EvtEnt e\<^sub>c, K = k\<rparr>, eventof = ec, domain = d\<rparr> = 
          Some \<lparr>actk = \<lparr>Act = EvtEnt (\<eta> e\<^sub>c), K = k\<rparr>, eventof = \<eta> e\<^sub>c, domain = d\<rparr>"
@@ -536,7 +768,7 @@ proof-
     by (metis act.exhaust action.surjective actk.surjective is_Cmd_act.simps(1) old.unit.exhaust option.distinct(1) sim_a.simps(2))
   then obtain P\<^sub>c k e\<^sub>c d where a3: "a\<^sub>c = \<lparr>actk = \<lparr>Act = Cmd P\<^sub>c, K = k\<rparr>, eventof = e\<^sub>c, domain = d\<rparr>"
     by (metis act.exhaust action.surjective actk.surjective is_Cmd_act.simps(2) old.unit.exhaust)
-  with a0 have a4: "\<kappa> e\<^sub>c P\<^sub>c = None"
+  with a0 have a4: "\<zeta> e\<^sub>c P\<^sub>c = None"
     by (metis option.discI sim_a.simps(1))
 
   obtain pes\<^sub>c s\<^sub>c x\<^sub>c pes\<^sub>c' s\<^sub>c' x\<^sub>c' where a5: "C\<^sub>c = (pes\<^sub>c ,s\<^sub>c ,x\<^sub>c) \<and> C\<^sub>c' = (pes\<^sub>c', s\<^sub>c', x\<^sub>c')" 
@@ -563,9 +795,9 @@ proof-
     assume "Act (actk a\<^sub>c) = Cmd P\<^sub>c"
     then obtain k e\<^sub>c d where b0: "a\<^sub>c = \<lparr>actk = \<lparr>Act = Cmd P\<^sub>c, K = k\<rparr>, eventof = e\<^sub>c, domain = d\<rparr>"
       by (metis action.surjective actk.surjective old.unit.exhaust)
-    with a0 have "\<exists>P\<^sub>a. \<kappa> e\<^sub>c P\<^sub>c = Some P\<^sub>a"
+    with a0 have "\<exists>P\<^sub>a. \<zeta> e\<^sub>c P\<^sub>c = Some P\<^sub>a"
       by (metis option.discI option.exhaust_sel sim_a.simps(1))
-    then obtain P\<^sub>a where b1: "\<kappa> e\<^sub>c P\<^sub>c = Some P\<^sub>a" by auto
+    then obtain P\<^sub>a where b1: "\<zeta> e\<^sub>c P\<^sub>c = Some P\<^sub>a" by auto
     with a0 b0 have b2: "a\<^sub>a = \<lparr>actk = \<lparr>Act = Cmd P\<^sub>a, K = k\<rparr>, eventof = \<eta> e\<^sub>c, domain = d\<rparr>" by auto
 
     obtain pes\<^sub>c s\<^sub>c x\<^sub>c pes\<^sub>c' s\<^sub>c' x\<^sub>c' where b3: "C\<^sub>c = (pes\<^sub>c ,s\<^sub>c ,x\<^sub>c) \<and> C\<^sub>c' = (pes\<^sub>c', s\<^sub>c', x\<^sub>c')" 
@@ -575,12 +807,12 @@ proof-
       by blast
     obtain pes\<^sub>a s\<^sub>a x\<^sub>a where b5: "C\<^sub>a = (pes\<^sub>a, s\<^sub>a, x\<^sub>a)" by (meson Sim.Event\<^sub>c.pesconf_trip)
     with a1 b1 b3 b4 have "\<exists>pes\<^sub>a' s\<^sub>a'. (\<Gamma>\<^sub>a \<turnstile>\<^sub>a (pes\<^sub>a, s\<^sub>a, x\<^sub>a) -pes-((Cmd P\<^sub>a)\<sharp>k)\<rightarrow> (pes\<^sub>a', s\<^sub>a', x\<^sub>a))
-    \<and> \<eta> (x\<^sub>c k) = (x\<^sub>a k) \<and> (\<Gamma>\<^sub>c, (pes\<^sub>c', s\<^sub>c', x\<^sub>c)) \<preceq>\<^sub>p\<^sub>e\<^sub>s \<^sub>(\<^sub>\<alpha>\<^sub>;\<^sub>\<eta>\<^sub>;\<^sub>\<kappa>\<^sub>) (\<Gamma>\<^sub>a, (pes\<^sub>a', s\<^sub>a', x\<^sub>a))"
+    \<and> \<eta> (x\<^sub>c k) = (x\<^sub>a k) \<and> (\<Gamma>\<^sub>c, (pes\<^sub>c', s\<^sub>c', x\<^sub>c)) \<preceq>\<^sub>p\<^sub>e\<^sub>s \<^sub>(\<^sub>\<alpha>\<^sub>;\<^sub>\<eta>\<^sub>;\<^sub>\<zeta>\<^sub>) (\<Gamma>\<^sub>a, (pes\<^sub>a', s\<^sub>a', x\<^sub>a))"
       apply (simp add: sim_s_def)
       apply (erule Sim.pes_sim.cases, simp)
       by (metis Sim.Event\<^sub>c.act_in_pes_notchgstate)
     then obtain pes\<^sub>a' s\<^sub>a' where b6: "(\<Gamma>\<^sub>a \<turnstile>\<^sub>a (pes\<^sub>a, s\<^sub>a, x\<^sub>a) -pes-((Cmd P\<^sub>a)\<sharp>k)\<rightarrow> (pes\<^sub>a', s\<^sub>a', x\<^sub>a))
-    \<and> \<eta> (x\<^sub>c k) = (x\<^sub>a k) \<and> (\<Gamma>\<^sub>c, (pes\<^sub>c', s\<^sub>c', x\<^sub>c)) \<preceq>\<^sub>p\<^sub>e\<^sub>s \<^sub>(\<^sub>\<alpha>\<^sub>;\<^sub>\<eta>\<^sub>;\<^sub>\<kappa>\<^sub>) (\<Gamma>\<^sub>a, (pes\<^sub>a', s\<^sub>a', x\<^sub>a))" by auto
+    \<and> \<eta> (x\<^sub>c k) = (x\<^sub>a k) \<and> (\<Gamma>\<^sub>c, (pes\<^sub>c', s\<^sub>c', x\<^sub>c)) \<preceq>\<^sub>p\<^sub>e\<^sub>s \<^sub>(\<^sub>\<alpha>\<^sub>;\<^sub>\<eta>\<^sub>;\<^sub>\<zeta>\<^sub>) (\<Gamma>\<^sub>a, (pes\<^sub>a', s\<^sub>a', x\<^sub>a))" by auto
 
     from a1 b3 b5 have "(s\<^sub>c, s\<^sub>a) \<in> \<alpha>"
       by (simp add: Sim.pes_sim_init sim_s_def)      
@@ -611,12 +843,12 @@ proof-
       by (metis Sim.Event\<^sub>c.evtent_in_pes_notchgstate)
     obtain pes\<^sub>a s\<^sub>a x\<^sub>a where b6: "C\<^sub>a = (pes\<^sub>a, s\<^sub>a, x\<^sub>a)" by (meson Sim.Event\<^sub>c.pesconf_trip)
     with a1 b3 b4 have "\<exists>e\<^sub>a pes\<^sub>a' x\<^sub>a'. (\<Gamma>\<^sub>a \<turnstile>\<^sub>a (pes\<^sub>a, s\<^sub>a, x\<^sub>a) -pes-((EvtEnt e\<^sub>a)\<sharp>k)\<rightarrow> (pes\<^sub>a', s\<^sub>a, x\<^sub>a'))
-    \<and> \<eta> e\<^sub>c = e\<^sub>a \<and> (\<Gamma>\<^sub>c, (pes\<^sub>c', s\<^sub>c, x\<^sub>c')) \<preceq>\<^sub>p\<^sub>e\<^sub>s \<^sub>(\<^sub>\<alpha>\<^sub>;\<^sub>\<eta>\<^sub>;\<^sub>\<kappa>\<^sub>) (\<Gamma>\<^sub>a, (pes\<^sub>a', s\<^sub>a, x\<^sub>a'))"
+    \<and> \<eta> e\<^sub>c = e\<^sub>a \<and> (\<Gamma>\<^sub>c, (pes\<^sub>c', s\<^sub>c, x\<^sub>c')) \<preceq>\<^sub>p\<^sub>e\<^sub>s \<^sub>(\<^sub>\<alpha>\<^sub>;\<^sub>\<eta>\<^sub>;\<^sub>\<zeta>\<^sub>) (\<Gamma>\<^sub>a, (pes\<^sub>a', s\<^sub>a, x\<^sub>a'))"
       apply (simp add: sim_s_def)
       apply (erule Sim.pes_sim.cases, simp)
       by (metis Sim.Event\<^sub>c.evtent_in_pes_notchgstate)
     then obtain pes\<^sub>a' x\<^sub>a' where b7: "(\<Gamma>\<^sub>a \<turnstile>\<^sub>a (pes\<^sub>a, s\<^sub>a, x\<^sub>a) -pes-((EvtEnt (\<eta> e\<^sub>c))\<sharp>k)\<rightarrow> (pes\<^sub>a', s\<^sub>a, x\<^sub>a'))
-     \<and> (\<Gamma>\<^sub>c, (pes\<^sub>c', s\<^sub>c, x\<^sub>c')) \<preceq>\<^sub>p\<^sub>e\<^sub>s \<^sub>(\<^sub>\<alpha>\<^sub>;\<^sub>\<eta>\<^sub>;\<^sub>\<kappa>\<^sub>) (\<Gamma>\<^sub>a, (pes\<^sub>a', s\<^sub>a, x\<^sub>a'))" by auto
+     \<and> (\<Gamma>\<^sub>c, (pes\<^sub>c', s\<^sub>c, x\<^sub>c')) \<preceq>\<^sub>p\<^sub>e\<^sub>s \<^sub>(\<^sub>\<alpha>\<^sub>;\<^sub>\<eta>\<^sub>;\<^sub>\<zeta>\<^sub>) (\<Gamma>\<^sub>a, (pes\<^sub>a', s\<^sub>a, x\<^sub>a'))" by auto
 
     then have "(s\<^sub>c, s\<^sub>a) \<in> \<alpha>"
       using Sim.pes_sim_init by blast
@@ -655,6 +887,12 @@ proof
   show "\<And>C\<^sub>c C\<^sub>a T\<^sub>c T\<^sub>a d. C\<^sub>c \<sim> C\<^sub>a \<Longrightarrow> T\<^sub>c \<sim> T\<^sub>a \<Longrightarrow> gets C\<^sub>a \<sim>\<^sub>ad\<sim>\<^sub>a gets T\<^sub>a = gets C\<^sub>c \<sim>\<^sub>cd\<sim>\<^sub>c gets T\<^sub>c "
     by (simp add: sim_ifs)
 qed
+
+theorem PiCore_abs_lr_imp: "InfoFlow\<^sub>a.local_respectC \<Longrightarrow> InfoFlow\<^sub>c.local_respectC"
+  using PiCore_abs_lr_imp by force
+
+theorem PiCore_abs_wsc_imp: "InfoFlow\<^sub>a.weak_step_consistentC \<Longrightarrow> InfoFlow\<^sub>c.weak_step_consistentC"
+  using PiCore_abs_wsc_imp by auto
 
 end
 
